<?xml version="1.0"?>
<rdf:RDF xmlns="https://w3id.org/dharc/ontology/chad-ap#"
     xml:base="https://w3id.org/dharc/ontology/chad-ap"
     xmlns:dc="http://purl.org/dc/elements/1.1/"
     xmlns:ns="http://www.w3.org/2003/06/sw-vocab-status/ns#"
     xmlns:owl="http://www.w3.org/2002/07/owl#"
     xmlns:rdf="http://www.w3.org/1999/02/22-rdf-syntax-ns#"
     xmlns:xml="http://www.w3.org/XML/1998/namespace"
     xmlns:xsd="http://www.w3.org/2001/XMLSchema#"
     xmlns:rdfs="http://www.w3.org/2000/01/rdf-schema#"
     xmlns:skos="http://www.w3.org/2004/02/skos/core#"
     xmlns:vann="http://purl.org/vocab/vann/"
     xmlns:terms="http://purl.org/dc/terms/">
    <owl:Ontology rdf:about="https://w3id.org/dharc/ontology/chad-ap">
        <owl:versionIRI rdf:resource="https://w3id.org/dharc/ontology/chad-ap/1.0.0"/>
        <dc:abstract xml:lang="en">A OWL 2 DL-based metadata application profile for describing cultural heritage digitisation data and processes in a FAIR-compliant and machine-readable format.</dc:abstract>
        <dc:contributor>Heibi, Ivan</dc:contributor>
        <dc:contributor>Moretti, Arianna</dc:contributor>
        <dc:creator>Barzaghi, Sebastian</dc:creator>
        <dc:creator>Peroni, Silvio</dc:creator>
        <dc:date rdf:datatype="http://www.w3.org/2001/XMLSchema#date">2024-04-16</dc:date>
        <dc:description xml:lang="en">

The Cultural Heritage Acquisition and Digitisation Application Profile (CHAD-AP, https://w3id.org/dharc/ontology/chad-ap) is a CIDOC CRM application profile implemented as an OWL ontology that can be logically split into two separate abstract modules: the Object Module (OM), dedicated to describing the CH objects, and the Process Module (PM), for describing the acquisition and digitisation process.

Both CHAD-AP and its [documentation](https://w3id.org/dharc/ontology/chad-ap) are living artefacts that have been drafted in the context of the [Project CHANGES](https://sites.google.com/uniroma1.it/changes/) (&quot;Cultural Heritage Active Innovation For Next-Gen Sustainable Society&quot;), an EU-funded project that  aims at increasing, at the Italian level, the curation, and management of cultural heritage artefacts in all forms, expanding the involvement of the general public, making more sustainable the exhibition potential, and including crucial social functions (accessibility, inclusiveness, critical thinking, participation, enjoyment, sustainability) into the cultural heritage environment.

Currently, CHAD-AP is able to describe the following entities:
* CH objects, described according to the Functional Requirements for Bibliographic Records (FRBR) data model, which uses several descriptive layers for its representation. In particular, CHAD-AP considers: the essence or conceptualisation of the CH object (_Work_); the intellectual content of the CH object (_Expression_); and the physical instance of the CH object (_Manifestation Singleton_);
* Activities, events, agents involved and their roles;
* Descriptive components, such as labels, types, identifiers and titles;
* Entities related to curation and conservation, like curation events, places of conservation, agent responsible for its conservation, etc.
* Concepts and other immaterial objects, such as the subjects illustrated by CH objects and the licenses or right statements assigned to them;
* Digitization processes used to capture 3D data of CH objects and to output their digital models, and software activities leveraging these digital objects as input for further processes.

The following figure contains a [Graffoo diagram](http://www.essepuntato.it/graffoo) that provides an overview of the class and properties reused in CHAD-AP.

![A Graffoo diagram of CHAD-AP](diagrams/profile-model.png)

The current version of the application profile reuses a subset of classes and properties selected from the following models:

* [CIDOC CRM](http://www.cidoc-crm.org/cidoc-crm/) is an international ISO standard that provides an ontology related to cultural heritage and museum documentation, which can be extended with additional modules for covering particular descriptions at hand;
* [CRMdig](http://www.ics.forth.gr/isl/CRMdig/) is an extension of CIDOC CRM for describing metadata related to the digital provenance of digitisation processes and digital representations;
* [FRBRoo](http://iflastandards.info/ns/fr/frbr/frbroo/) is an ontology for representing bibliographic information according to the FRBR data model within the CIDOC CRM framework;
* [AAT](http://vocab.getty.edu/page/aat/) is a structured vocabulary of terms used to describe art, architecture, decorative arts, and material culture.

A full version of CHAD-AP is available at [https://w3id.org/dharc/ontology/chad-ap](https://w3id.org/dharc/ontology/chad-ap).

The next subsections provide a quick overview of all the entities defined, some exemple of usage, and some of the queries that CHAD-AP can answer.

## Description
### Object Module (OM)
As shown in the diagram below, a Cultural Heritage (CH) object is described in CHAD-AP according to the Functional Requirements for Bibliographic Records (FRBR) data model, which uses several descriptive layers for its representation. 

![A diagram of the CHAD-AP Object Module (OM).](diagrams/profile-model.png)

In particular, the _Work_ (`frbroo:F1_Work`) represents the _essence_ or conceptualization of the CH object. It begins with a conception event (`frbroo:F27_Work_Conception`) occurring within a specific time span (`crm:E52_Time-Span`), which can be expressed as either a precisely defined period with exact starting and ending date times (`crm:P82a_begin_of_the_begin` and `crm:P82b_end_of_the_end`) or a fuzzy label if its temporal extents are not precisely known (`crm:P82_at_some_time_within`). Each work is associated with a series of titles (`crm:E35_Title`), each classified according to a particular type (`crm:E55_Type`), which can be an _original title_ (`aat:300417204`) or an _exhibition title_ (`aat:300417207`). Furthermore, a Work can be part of a larger Work (`frbroo:F15_Complex_Work`), like a series of printed volumes, which is classified under a particular type (`crm:E55_Type`).

The _Expression_ (`frbroo:F2_Expression`) is the realisation of a Work, and refers to the intellectual _content_ of the object. It is generated through a creation event (`frbroo:F28_Expression_Creation`) made of smaller activities (`crm:E7_Activity`), each conducted by one or more agents (`crm:E39_Actor`) and characterised by a specific type (`crm:E55_Type`) that defines, implicitly, the role assumed by the agent for that activity. For example, if the agent is identified as the author of the Expression, the activity type is represented as _writing_ (`aat:300054698`). Also, creation events employ various creation techniques (`crm:E55_Type`). For example, `aat:300054196` is used to express _drawing technique_. An Expression can also be associated with one or more subjects defining its contents. In CHAD-AP, a generic _concept_ is represented with the class `crm:E73_Information_Object` with the type `aat:300404126` (i.e. _subject_) explicitly specified.

Finally, the _Manifestation Singleton_ (`frbroo:F4_Manifestation_Singleton`) represents the physical instance of the CH object. It is accompanied with descriptive components like labels (expressed through the use of the property `crm:P3_has_note`), types (`crm:E55_Type`), and identifiers (`crm:E42_Identifier`). In some cases, it may be linked to a curation activity (`crm:E87_Curation_Activity`) carried out by a keeper (`crm:E39_Actor`) who manages a collection (`crm:E78_Curated_Holding`) the object belongs to, and that is located in a specific place (`crm:E53_Place`). Manifestations can consist of other Manifestations and may depict the Expression of another related object, such as a video displaying a manuscript or a tablet showing a picture of a specimen. In addition, Manifestations are associated with copyright or licensing statements (represented through the combination of `crm:E73_Information_Object` having type `aat:300435434`, i.e.  _copyright/licensing statement_), linked with the document introducing the actual license or right statements through the property `crm:P70i_is_documented_in`. Whenever possible, instances of `crm:E39_Actor` and `crm:E53_Place` are also linked with existing authority records through the property `crm:P48_has_preferred_identifier`.

### Process Module (PM)
As shown in the diagram below, CHAD-AP also describes the entities for defining a 3D digitisation workflow as a sequence of activities classified according to two main categories. 

![A diagram of the CHAD-AP Process Module (PM).](diagrams/profile-model.png)

On the one hand, we have the _acquisition activity_ (`crmdig:D2_Digitization_Process`), which involves the digitisation of a CH object (`crm:E24_Physical_Human-Made_Thing`) to produce its digital CH object (`crmdig:D9_Data_Object`). Similarly to its physical counterpart, the digital CH object can be associated with copyright statements or licenses (`crm:E73_Information_Object` with `aat:300435434` as its type). The acquisition occurs within a time span (`crm:E52_Time-Span`) with defined starting and ending date times, and engages various agents, including individuals (`crm:E21_Person`) and institutions (`crm:E74_Group`) responsible for the activity. During the acquisition, a series of techniques (`crm:E55_Type`) can be used, such as _photogrammetry_ (`aat:300053580`) or _structured light scanning_ (`aat:300391312`), along with tools (`crmdig:D8_Digital_Device`) like _digital cameras_ (`aat:300266792`) and _structured light scanners_ (`aat:300429747`).

On the other hand, we have a series of _software activities_ (`crmdig:D10_Software_Execution`), each representing a specific stage or phase of digitisation workflow. Such stage is denoted by its type (`crm:E55_Type`), such as _processing_ (`aat:300054636`), _modelling_ (`aat:300391447`), and _optimization_ (`aat:300386427`). It involves the manipulation of the digital CH object (`crmdig:D9_Data_Object`) produced previously as input and the production of a modified version of that digital CH object (`crmdig:D9_Data_Object`) as output. The activity also occurs within a defined time span (`crm:E52_Time-Span`) with precise start and end date times, engages various agents, including individuals (`crm:E21_Person`) and institutions (`crm:E74_Group`), and uses software as tools to produce its output (`crmdig:D14_Software`).

## Examples of use
CHAD-AP can be used for modelling  scenarios related to cultural heritage acquisition and digitisation processes. In the following subsections we introduce some of them, and we accompany them with exemplar instantiations. 

The prefixes that are used in all the examples provided below are defined as follows:

    @prefix aat: &lt;http://vocab.getty.edu/page/aat/&gt; .
    @prefix ex: &lt;https://w3id.org/dharc/ontology/chad-ap/data/example/&gt; .
    @prefix crm: &lt;http://www.cidoc-crm.org/cidoc-crm/&gt; .
    @prefix crmdig: &lt;http://www.ics.forth.gr/isl/CRMdig/&gt; .
    @prefix frbroo: &lt;http://iflastandards.info/ns/fr/frbr/frbroo/&gt; .
    @prefix owl: &lt;http://www.w3.org/2002/07/owl#&gt; .
    @prefix rdf: &lt;http://www.w3.org/1999/02/22-rdf-syntax-ns#&gt; .
    @prefix xml: &lt;http://www.w3.org/XML/1998/namespace&gt; .
    @prefix xsd: &lt;http://www.w3.org/2001/XMLSchema#&gt; .
    @prefix rdfs: &lt;http://www.w3.org/2000/01/rdf-schema#&gt; .

### Scenario 1
The creation event `01-exp-creation-00` created the CH object `01-exp` (&apos;Amerigo Vespucci sveglia l’America&apos;) through the technique `engraving`. The creation event consists of three smaller creation events:
* `01-exp-creation-01`, carried out by `Jan van der Straet` (`ULAN:500011304`), in the role of `illustration`;
* `01-exp-creation-02`, carried out by `Philip Galle`, `Theodor Galle` and `Jan Collaert`, in the role of `engraving process`;
* `01-exp-creation-03`, carried out by `Luigi Alamanni` (`ULAN:500714480`), in the role of `commission`.

The creation event `35-exp-creation-00` created the CH object `35-exp` (&apos;De plantis epitome utilissima&apos;) through the technique `watercolor`. The creation event consists of two smaller creation events:
* `35-exp-creation-01`, carried out by `Pietro Andrea Mattioli` (`VIAF:61549376`), in the role of `translation`;
* `35-exp-creation-02`, carried out by `Pietro Andrea Mattioli` (`VIAF:61549376`), in the role of `illustration`.

The creation event `24-exp-creation-00` created the CH object `24-exp` (&apos;Panthera onca (Linnaeus, 1758)&apos;) through the technique `taxidermy`. The creation event consists of two smaller creation events:
* `24-exp-creation-01`, carried out by `Carl Linnaeus` (`VIAF:34594730`), in the role of `discovery`;
* `24-exp-creation-02`, carried out by `Naturaliter`, in the role of `museum preparation`.

```
ex:L1-exp-creation-00 a frbroo:F28_Expression_Creation ;
    frbroo:R17_created ex:L1-exp ;
    crm:P32_used_general_technique aat:300053225 ;
    crm:P9_consists_of ex:L1-exp-creation-01 ,
        ex:L1-exp-creation-02 ,
        ex:L1-exp-creation-03 .

ex:L1-exp-creation-01 a crm:E7_Activity ;
    crm:P2_has_type aat:300054200 ;
    crm:P14_carried_out_by ex:jan-van-der-straet .

ex:L1-exp-creation-02 a crm:E7_Activity ;
    crm:P2_has_type aat:300053225 ;
    crm:P14_carried_out_by ex:philip-galle ,
        ex:theodor-galle ,
        ex:jan-collaert .

ex:L1-exp-creation-03 a crm:E7_Activity ;
    crm:P2_has_type aat:300417639 ;
    crm:P14_carried_out_by ex:luigi-alamanni .

ex:L1-exp a frbroo:F2_Expression .

ex:jan-van-der-straet a crm:E39_Actor ;
    crm:P48_has_preferred_identifier &lt;http://vocab.getty.edu/page/ulan/500011304&gt; .

ex:philip-galle a crm:E39_Actor .

ex:theodor-galle a crm:E39_Actor .

ex:jan-collaert a crm:E39_Actor .

ex:luigi-alamanni a crm:E39_Actor .

ex:35-exp-creation-00 a frbroo:F28_Expression_Creation ;
    crm:P32_used_general_technique aat:300015045 ;
    frbroo:R17_created ex:35-exp ;
    crm:P9_consists_of ex:35-exp-creation-01 ,
        ex:35-exp-creation-02 .

ex:35-exp a frbroo:F2_Expression .

ex:35-exp-creation-01 a crm:E7_Activity ;
    crm:P2_has_type aat:300069831 ;
    crm:P14_carried_out_by ex:pietro-andrea-mattioli .

ex:35-exp-creation-02 a crm:E7_Activity ;
    crm:P2_has_type aat:300054200 ;
    crm:P14_carried_out_by ex:pietro-andrea-mattioli .

ex:pietro-andrea-mattioli a crm:E39_Actor ;
    crm:P48_has_preferred_identifier &lt;http://viaf.org/viaf/61549376&gt; .

ex:24-exp-creation-00 a frbroo:F28_Expression_Creation ;
    frbroo:R17_created ex:24-exp ;
    crm:P32_used_general_technique aat:300053628 ;
    crm:P9_consists_of ex:24-exp-creation-01 ,
        ex:24-exp-creation-02 .

ex:24-exp a frbroo:F2_Expression .

ex:24-exp-creation-01 a crm:E7_Activity ;
    crm:P2_has_type aat:300404386 ;
    crm:P14_carried_out_by ex:carl-linnaeus .

ex:24-exp-creation-02 a crm:E7_Activity ;
    crm:P2_has_type aat:300077565 ;
    crm:P14_carried_out_by ex:naturaliter .

ex:carl-linnaeus a crm:E39_Actor ;
    crm:P48_has_preferred_identifier &lt;http://viaf.org/viaf/34594730&gt; .

ex:naturaliter a crm:E39_Actor .
```

#### Scenario 2
The creation event `01-exp-creation-00` created the CH object `01-man` (&apos;Amerigo Vespucci sveglia l’America&apos;). The CH object has the identifier &apos;01&apos; with type equal to `project id`. Its type is `print`. Its descriptive label is &apos;Amerigo Vespucci sveglia l’America
 Amerigo Vespucci awakens a sleeping America
 In
 Jan van del Straet (Stradano), Nova Reperta, c. 1589 – c.1593, Antwerp
 Amsterdam, Rijksmuseum&apos;

The creation event `05-exp-creation-00` created the CH object `05-exp` (&apos;De Historia Animalium lib. 9&apos;). The CH object has the identifiers:
* &apos;05&apos; with type equal to `project id`
* &apos;9&apos; with type equal to `volume number`
* &apos;A.V.GG.VII.28&apos; with type equal to `shelf mark`
Its type is `printed volume`. Its descriptive label is &apos;Aristoteles
 De Historia Animalium lib. 9 
 Venezia, Girolamo Scoto, 1545
 BUB, A.V.GG.VII.28&apos;

The creation event `45-exp-creation-00` created the CH object `45-exp` (&apos;Dryas octopetala L.&apos;). The CH object has the identifiers:
* &apos;45&apos; with type equal to `project id`
* &apos;13&apos; with type equal to `volume number`
* &apos;Erbario Aldrovandi, vol.13, carta 77&apos; with type equal to `shelf mark`
Its type is `specimen`. Its descriptive label is &apos;Dryas octopetala L.
 Camedrio alpino 
 Mountain avens 
 Erbario Aldrovandi, vol.13, carta 77
 sec. XVI 16th century
 Bologna, Orto Botanico ed Erbario, Sistema Museale di Ateneo&apos;

```
ex:L1-exp-creation-00 a frbroo:F28_Expression_Creation ;
    frbroo:R18_created ex:L1-man .

ex:L1-man a frbroo:F4_Manifestation_Singleton ;
    crm:P48_has_preferred_identifier ex:L1-identifier-00 ;
    crm:P2_has_type aat:300041273 ;
    crm:P3_has_note &quot;Amerigo Vespucci sveglia l&apos;America Amerigo Vespucci awakens a sleeping America In Jan van del Straet (Stradano), Nova Reperta, c. 1589 - c.1593, Antwerp Amsterdam, Rijksmuseum&quot;^^rdfs:Literal .

ex:L1-identifier-00 a crm:E42_Identifier ;
    crm:P190_has_symbolic_content &quot;L1&quot;^^rdfs:Literal ;
    crm:P2_has_type aat:300312355 .

ex:05-exp-creation-00 a frbroo:F28_Expression_Creation ;
    frbroo:R18_created ex:05-man .

ex:05-man a frbroo:F4_Manifestation_Singleton ;
    crm:P48_has_preferred_identifier ex:05-identifier-00 ,
        ex:05-identifier-01 ,
        ex:05-identifier-02 ;
    crm:P2_has_type aat:300265632 ;
    crm:P3_has_note &quot;Aristoteles De Historia Animalium lib. 9 Venezia, Girolamo Scoto, 1545 BUB, A.V.GG.VII.28&quot;^^rdfs:Literal .

ex:05-identifier-00 a crm:E42_Identifier ;
    crm:P190_has_symbolic_content &quot;05&quot;^^rdfs:Literal ;
    crm:P2_has_type aat:300312355 .

ex:05-identifier-01 a crm:E42_Identifier ;
    crm:P190_has_symbolic_content &quot;9&quot;^^rdfs:Literal ;
    crm:P2_has_type aat:300445021 .

ex:05-identifier-02 a crm:E42_Identifier ;
    crm:P190_has_symbolic_content &quot;A.V.GG.VII.28&quot;^^rdfs:Literal ;
    crm:P2_has_type aat:300404704 .

ex:45-exp-creation-00 a frbroo:F28_Expression_Creation ;
    frbroo:R18_created ex:45-man .

ex:45-man a frbroo:F4_Manifestation_Singleton ;
    crm:P48_has_preferred_identifier ex:45-identifier-00 ,
        ex:45-identifier-01 ,
        ex:45-identifier-02 ;
    crm:P2_has_type aat:300235576 ;
    crm:P3_has_note &quot;Dryas octopetala L. Camedrio alpino Mountain avens Erbario Aldrovandi, vol.13, carta 77 sec. XVI 16th century Bologna, Orto Botanico ed Erbario, Sistema Museale di Ateneo&quot;^^rdfs:Literal .

ex:45-identifier-00 a crm:E42_Identifier ;
    crm:P190_has_symbolic_content &quot;45&quot;^^rdfs:Literal ;
    crm:P2_has_type aat:300312355 .

ex:45-identifier-01 a crm:E42_Identifier ;
    crm:P190_has_symbolic_content &quot;13&quot;^^rdfs:Literal ;
    crm:P2_has_type aat:300445021 .

ex:45-identifier-02 a crm:E42_Identifier ;
    crm:P190_has_symbolic_content &quot;Erbario Aldrovandi, vol.13, carta 77&quot;^^rdfs:Literal ;
    crm:P2_has_type aat:300404704 .
```

#### Scenario 3
A curation event `L1-curation` - carried out by `Rijksmuseum` (located in `Amsterdam`) - curated the collection `Nova Reperta` for the CH object `L1-man`.

A curation event `1-curation` - carried out by `Sistema museale di Ateneo` (located in `Bologna`) - curated the collection `Collezione di Zoologia` for the CH object `1-man`.

A curation event `14-curation` - carried out by `Sistema museale di Ateneo` (located in `Bologna`) - curated the collection `Collezione di Anatomia comparata` for the CH object `14-man`.

```
ex:L1-curation a crm:E87_Curation_Activity ;
    crm:P147_curated ex:nova-reperta ;
    crm:P14_carried_out_by ex:rijksmuseum ;
    crm:P12_occurred_in_the_presence_of ex:L1-man .

ex:L1-man a frbroo:F4_Manifestation_Singleton ;
    crm:P74_has_current_or_former_residence ex:rijksmuseum .

ex:nova-reperta a crm:E78_Curated_Holding .

ex:rijksmuseum a crm:E39_Actor ;
    crm:P74_has_current_or_former_residence ex:amsterdam .

ex:amsterdam a crm:E53_Place .

ex:1-curation a crm:E87_Curation_Activity ;
    crm:P147_curated ex:collezione-di-zoologia ;
    crm:P14_carried_out_by ex:sistema-museale-di-ateneo ;
    crm:P12_occurred_in_the_presence_of ex:1-man .

ex:1-man a frbroo:F4_Manifestation_Singleton ;
    crm:P74_has_current_or_former_residence ex:sistema-museale-di-ateneo .

ex:collezione-di-zoologia a crm:E78_Curated_Holding .

ex:sistema-museale-di-ateneo a crm:E39_Actor ;
    crm:P74_has_current_or_former_residence ex:bologna .

ex:bologna a crm:E53_Place .

ex:14-curation a crm:E87_Curation_Activity ;
    crm:P147_curated ex:collezione-di-anatomia-comparata ;
    crm:P14_carried_out_by ex:sistema-museale-di-ateneo ;
    crm:P12_occurred_in_the_presence_of ex:14-man .

ex:14-man a frbroo:F4_Manifestation_Singleton ;
    crm:P74_has_current_or_former_residence ex:sistema-museale-di-ateneo .

ex:collezione-di-anatomia-comparata a crm:E78_Curated_Holding .

```

#### Scenario 4
A conception event `L1-work-conception` initiated the CH object `L1-work` (&apos;Amerigo Vespucci sveglia l’America&apos;) in the time interval `1589-1593`, which starts in 1589-01-01 and ends in 1593-12-31.

A conception event `1-work-conception` initiated the CH object `1-work` (&apos;Carta nautica&apos;) in the time interval `1482`, which starts in 1482-01-01 and ends in 1482-12-31.

A conception event `26-work-conception` initiated the CH object `26-work` (&apos;Chrysanthemi&apos;) in the time interval `1500-1599`, which starts in 1500-01-01 and ends in 1599-12-31.

```
ex:L1-work-conception a frbroo:F27_Work_Conception ;
    frbroo:R16_initiated ex:L1-work ;
    crm:P4_has_time-span ex:1589-1593 .            

ex:1589-1593 a crm:E52_Time-Span ;
    crm:P82a_begin_of_the_begin &quot;1589-01-01T00:00:00&quot;^^xsd:dateTime ;
    crm:P82b_end_of_the_end &quot;1593-12-31T23:59:59&quot;^^xsd:dateTime .

ex:L1-work a frbroo:F1_Work .

ex:1-work-conception a frbroo:F27_Work_Conception ;
    frbroo:R16_initiated ex:1-work ;
    crm:P4_has_time-span ex:1482 .            

ex:1482 a crm:E52_Time-Span ;
    crm:P82a_begin_of_the_begin &quot;1482-01-01T00:00:00&quot;^^xsd:dateTime ;
    crm:P82b_end_of_the_end &quot;1482-12-31T23:59:59&quot;^^xsd:dateTime .

ex:1-work a frbroo:F1_Work .

ex:26-work-conception a frbroo:F27_Work_Conception ;
    frbroo:R16_initiated ex:26-work ;
    crm:P4_has_time-span ex:1500-1599 .            

ex:1500-1599 a crm:E52_Time-Span ;
    crm:P82a_begin_of_the_begin &quot;1500-01-01T00:00:00&quot;^^xsd:dateTime ;
    crm:P82b_end_of_the_end &quot;1599-12-31T23:59:59&quot;^^xsd:dateTime .

ex:26-work a frbroo:F1_Work .
```

#### Scenario 5
The creation event `L1-exp-creation` created the work `L1-work`, the expression `L1-exp` and the manifestation `L1-man`. 
`L1-work` has two titles: the original title `L1-work-title-01` (&apos;Amerigo Vespucci sveglia l&apos;America&apos;), and the exhibition title `L1-work-title-02` (&apos;Amerigo Vespucci sveglia l&apos;America&apos;). It is member of the parent work `Nova Reperta`, which has `print series` as its type.
`L1-exp` is about the following subjects: `amerigo vespucci`, `astrolabio`, `vessillo croce del sud`, `formichiere`, `bradipo`, `tapiro`, and `gruppo di cannibali`.

The creation event `1-exp-creation` created the work `1-work`, the expression `1-exp` and the manifestation `1-man`. 
`1-work` has two titles: the original title `1-work-title-01` (&apos;Carta nautica&apos;), and the exhibition title `1-work-title-02` (&apos;Carta nautica&apos;).
`1-exp` is about the following subjects: `europa`, `africa`, `asia`, and `mar mediterraneo`.

The creation event `7-exp-creation` created the work `7-work`, the expression `7-exp` and the manifestation `7-man`. 
`7-work` has two titles: the original title `7-work-title-01` (&apos;Profilo incompleto delle coste del continente americano&apos;), and the exhibition title `7-work-title-02` (&apos;Profilo incompleto delle coste del continente americano&apos;). It is member of the parent work `Atlante Nautico`, which has `marine chart` as its type.
`7-exp` is about the following subjects: `america` and `europa`.

```
ex:L1-exp-creation a frbroo:F28_Expression_Creation ;
    frbroo:R19_created_a_realisation_of ex:L1-work ;
    frbroo:R17_created ex:L1-exp ;
    frbroo:R18_created ex:L1-man .

ex:L1-work a frbroo:F1_Work ;
    crm:P102_has_title ex:L1-work-title-01 ,
        ex:L1-work-title-02 .

ex:L1-work-title-01 a crm:E35_Title ;
    crm:P2_has_type aat:300417204 ;
    crm:P190_has_symbolic_content &quot;Amerigo Vespucci sveglia l&apos;America&quot;@it .

ex:L1-work-title-02 a crm:E35_Title ;
    crm:P2_has_type aat:300417207 ;
    crm:P190_has_symbolic_content &quot;Amerigo Vespucci sveglia l&apos;America&quot;@en .

ex:L1-exp a frbroo:F2_Expression ;
    crm:P129_is_about ex:sub-amerigo-vespucci ,
        ex:sub-astrolabio ,
        ex:sub-vessillo-croce-del-sud ,
        ex:sub-formichiere ,
        ex:sub-bradipo ,
        ex:sub-tapiro ,
        ex:sub-gruppo-di-cannibali .

ex:L1-man a frbroo:F4_Manifestation_Singleton .

ex:L1-man-license a crm:E73_Information_Object ;
    crm:P2_has_type aat:300435434 ;
    crm:P67_refers_to ex:L1-man ;
    crm:P70i_is_documented_in &lt;http://rightsstatements.org/vocab/InC/1.0/&gt; .

ex:1-man-license a crm:E73_Information_Object ;
    crm:P2_has_type aat:300435434 ;
    crm:P67_refers_to ex:1-man ;
    crm:P70i_is_documented_in &lt;http://rightsstatements.org/vocab/InC/1.0/&gt; .

ex:7-man-license a crm:E73_Information_Object ;
    crm:P2_has_type aat:300435434 ;
    crm:P67_refers_to ex:7-man ;
    crm:P70i_is_documented_in &lt;http://rightsstatements.org/vocab/InC/1.0/&gt; .

ex:PTa-man-license a crm:E73_Information_Object ;
    crm:P2_has_type aat:300435434 ;
    crm:P67_refers_to ex:PTa-man ;
    crm:P70i_is_documented_in &lt;http://rightsstatements.org/vocab/InC/1.0/&gt; .

ex:PTa-1-man-license a crm:E73_Information_Object ;
    crm:P2_has_type aat:300435434 ;
    crm:P67_refers_to ex:PTa-1-man ;
    crm:P70i_is_documented_in &lt;http://rightsstatements.org/vocab/InC/1.0/&gt; .

ex:PTa-2-man-license a crm:E73_Information_Object ;
    crm:P2_has_type aat:300435434 ;
    crm:P67_refers_to ex:PTa-2-man ;
    crm:P70i_is_documented_in &lt;http://rightsstatements.org/vocab/InC/1.0/&gt; .

ex:PTa-3-man-license a crm:E73_Information_Object ;
    crm:P2_has_type aat:300435434 ;
    crm:P67_refers_to ex:PTa-3-man ;
    crm:P70i_is_documented_in &lt;http://rightsstatements.org/vocab/InC/1.0/&gt; .

ex:nova-reperta a frbroo:F15_Complex_Work ;
    frbroo:R10_has_member ex:L1-work ;
    crm:P2_has_type aat:300189634 .

ex:sub-amerigo-vespucci a crm:E73_Information_Object ;
    crm:P2_has_type aat:300404126 .

ex:sub-astrolabio a crm:E73_Information_Object ;
    crm:P2_has_type aat:300404126 .

ex:sub-vessillo-croce-del-sud a crm:E73_Information_Object ;
    crm:P2_has_type aat:300404126 .

ex:sub-formichiere a crm:E73_Information_Object ;
    crm:P2_has_type aat:300404126 .

ex:sub-bradipo a crm:E73_Information_Object ;
    crm:P2_has_type aat:300404126 .

ex:sub-tapiro a crm:E73_Information_Object ;
    crm:P2_has_type aat:300404126 .

ex:sub-gruppo-di-cannibali a crm:E73_Information_Object ;
    crm:P2_has_type aat:300404126 .

ex:1-exp-creation a frbroo:F28_Expression_Creation ;
    frbroo:R19_created_a_realisation_of ex:1-work ;
    frbroo:R17_created ex:1-exp ;
    frbroo:R18_created ex:1-man .

ex:1-work a frbroo:F1_Work ;
    crm:P102_has_title ex:1-work-title-01 ,
        ex:1-work-title-02 .

ex:1-work-title-01 a crm:E35_Title ;
    crm:P2_has_type aat:300417204 ;
    crm:P190_has_symbolic_content &quot;Carta nautica&quot;@it .

ex:1-work-title-02 a crm:E35_Title ;
    crm:P2_has_type aat:300417207 ;
    crm:P190_has_symbolic_content &quot;Carta nautica&quot;@it .

ex:1-exp a frbroo:F2_Expression ;
    crm:P129_is_about ex:sub-europa ,
        ex:sub-africa ,
        ex:sub-asia ,
        ex:sub-mar-mediterraneo .

ex:1-man a frbroo:F4_Manifestation_Singleton .

ex:sub-europa a crm:E73_Information_Object ;
    crm:P2_has_type aat:300404126 .

ex:sub-africa a crm:E73_Information_Object ;
    crm:P2_has_type aat:300404126 .

ex:sub-asia a crm:E73_Information_Object ;
    crm:P2_has_type aat:300404126 .

ex:sub-mar-mediterraneo a crm:E73_Information_Object ;
    crm:P2_has_type aat:300404126 .

ex:7-exp-creation a frbroo:F28_Expression_Creation ;
    frbroo:R19_created_a_realisation_of ex:7-work ;
    frbroo:R17_created ex:7-exp ;
    frbroo:R18_created ex:7-man .

ex:7-work a frbroo:F1_Work ;
    crm:P102_has_title ex:7-work-title-01 ,
        ex:7-work-title-02 .

ex:7-work-title-01 a crm:E35_Title ;
    crm:P2_has_type aat:300417204 ;
    crm:P190_has_symbolic_content &quot;Profilo incompleto delle coste del continente americano&quot;@it .

ex:7-work-title-02 a crm:E35_Title ;
    crm:P2_has_type aat:300417207 ;
    crm:P190_has_symbolic_content &quot;Profilo incompleto delle coste del continente americano&quot;@it .

ex:7-exp a frbroo:F2_Expression ;
    crm:P129_is_about ex:sub-america ,
        ex:sub-europa .

ex:7-man a frbroo:F4_Manifestation_Singleton .

ex:atlante-nautico a frbroo:F15_Complex_Work ;
    frbroo:R10_has_member ex:7-work ;
    crm:P2_has_type aat:300028309 .

ex:sub-america a crm:E73_Information_Object ;
    crm:P2_has_type aat:300404126 .

ex:PTa-exp-creation a frbroo:F28_Expression_Creation ;
    frbroo:R19_created_a_realisation_of ex:PTa-work ;
    frbroo:R17_created ex:PTa-exp ;
    frbroo:R18_created ex:PTa-man .

ex:PTa-work a frbroo:F1_Work .

ex:PTa-exp a frbroo:F2_Expression .

ex:PTa-man a frbroo:F4_Manifestation_Singleton ;
    crm:P46_is_composed_of ex:PTa-1-man , 
        ex:PTa-2-man .

ex:PTa-1-exp-creation a frbroo:F28_Expression_Creation ;
    frbroo:R19_created_a_realisation_of ex:PTa-1-work ;
    frbroo:R17_created ex:PTa-1-exp ;
    frbroo:R18_created ex:PTa-1-man .

ex:PTa-1-work a frbroo:F1_Work .

ex:PTa-1-exp a frbroo:F2_Expression .

ex:PTa-1-man a frbroo:F4_Manifestation_Singleton .

ex:PTa-2-exp-creation a frbroo:F28_Expression_Creation ;
    frbroo:R19_created_a_realisation_of ex:PTa-2-work ;
    frbroo:R17_created ex:PTa-2-exp ;
    frbroo:R18_created ex:PTa-2-man .

ex:PTa-2-work a frbroo:F1_Work .

ex:PTa-2-exp a frbroo:F2_Expression .

ex:PTa-2-man a frbroo:F4_Manifestation_Singleton .

ex:PTa-3-exp-creation a frbroo:F28_Expression_Creation ;
    frbroo:R19_created_a_realisation_of ex:PTa-3-work ;
    frbroo:R17_created ex:PTa-3-exp ;
    frbroo:R18_created ex:PTa-3-man .

ex:PTa-3-work a frbroo:F1_Work .

ex:PTa-3-exp a frbroo:F2_Expression .

ex:PTa-3-man a frbroo:F4_Manifestation_Singleton ;
    crm:P62_depicts ex:PTa-man .
```

#### Scenario 6
The object `32` has been digitally acquired on the 8th of May 2023. The digitization process produced a 3D model `32-output-acq` as an output, provided with a &apos;CC BY-NC 4.0&apos; license, which will be used as an input by the software activity `32-proc`.

```
ex:32 a crm:E24_Physical_Human-Made_Thing .

ex:32-acq a crmdig:D2_Digitization_Process ;
    crmdig:L1_digitized ex:32 ;
    crmdig:L11_had_output ex:32-acq-output ;
    crm:P4_has_time-span ex:32-acq-timespan .

ex:32-proc a crmdig:D10_Software_Execution ;
    crmdig:L10_had_input ex:32-acq-output ;
    crm:P4_has_time-span ex:32-proc-timespan .

ex:32-acq-output a crmdig:D9_Data_Object .

ex:32-acq-output-license a crm:E73_Information_Object ;
    crm:P2_has_type aat:300435434 ;
    crm:P67_refers_to ex:32-acq-output ;
    crm:P70i_is_documented_in &lt;https://creativecommons.org/licenses/by-nc/4.0/&gt; .

ex:32-acq-timespan a crm:E52_Time-Span ;
    crm:P82a_begin_of_the_begin &quot;2023-05-08T00:00:00Z&quot;^^xsd:dateTime ;
    crm:P82b_end_of_the_end &quot;2023-05-08T23:59:59Z&quot;^^xsd:dateTime .

ex:32-proc-timespan a crm:E52_Time-Span ;
    crm:P82a_begin_of_the_begin &quot;2023-05-10T00:00:00Z&quot;^^xsd:dateTime ;
    crm:P82b_end_of_the_end &quot;2023-05-10T23:59:59Z&quot;^^xsd:dateTime .
```

#### Scenario 7
The digital object `15-proc-output` has been generated as an output during the processing activity carried out by the person `Federica Collina`, who belongs to the institution `UNIBO DBC`. The processing activity used the digital object `15-acq-output` (produced by the digitization process `15-acq`) as an input.

```
ex:15 a crm:E24_Physical_Human-Made_Thing .

ex:15-acq a crmdig:D2_Digitization_Process ;
    crmdig:L11_had_output ex:15-acq-output .

ex:15-proc a crmdig:D10_Software_Execution ;
    crm:P2_has_type aat:300054636 ;
    crmdig:L10_had_input ex:15-acq-output ;
    crmdig:L11_had_output ex:15-proc-output ;
    crm:P11_had_participant ex:unibo-dbc ;
    crm:P14_carried_out_by ex:federica-collina .

ex:15-acq-output a crmdig:D9_Data_Object .

ex:15-proc-output a crmdig:D9_Data_Object .

ex:federica-collina a crm:E21_Person .

ex:unibo-dbc a crm:E74_Group .
```

#### Scenario 8
The physical object `15` has been digitally acquired through the `structured light scanning` technique and the `scanner spider` tool. The digitization process produced a 3D model `15-acq-output` as an output.

```
ex:15 a crm:E24_Physical_Human-Made_Thing .

ex:15-acq a crmdig:D2_Digitization_Process ;
    crmdig:L1_digitized ex:15 ;
    crmdig:L11_had_output ex:15-acq-output ;
    crm:P32_used_general_technique aat:300391312 ;
    crm:P16_used_specific_object ex:artec-spider .

ex:15-proc a crmdig:D10_Software_Execution ;
    crm:P2_has_type aat:300054636 ;
    crmdig:L10_had_input ex:15-acq-output ;
    crmdig:L11_had_output ex:15-proc-output ;
    crmdig:L23_used_software_or_firmware ex:artec-studio-14 .

ex:15-acq-output a crmdig:D9_Data_Object .

ex:15-proc-output a crmdig:D9_Data_Object .

ex:artec-spider a crmdig:D8_Digital_Device ;
    crm:P2_has_type aat:300429747 .

ex:artec-studio-14 a crmdig:D14_Software ;
    crm:P2_has_type aat:300426696 .
```

### Competency questions
CHAD-AP can be used for answering several questions related to the acquisition and digitisation of cultural heritage objects. In the following subsections we introduce some of them, and we accompany them with exemplar SPARQL queries. 

The prefixes that are used in all the SPARQL queries provided below are defined as follows:

    PREFIX aat: &lt;http://vocab.getty.edu/page/aat/&gt;
    PREFIX crm: &lt;http://www.cidoc-crm.org/cidoc-crm/&gt;
    PREFIX crmdig: &lt;http://www.ics.forth.gr/isl/CRMdig/&gt;
    PREFIX ex: &lt;https://w3id.org/dharc/ontology/chad-ap/data/example/&gt;
    PREFIX frbroo: &lt;http://iflastandards.info/ns/fr/frbr/frbroo/&gt;  


#### Question 1
What are the CH objects whose creation involved some author?

    SELECT ?resource ?agent
    WHERE {
        ?creation_event a frbroo:F28_Expression_Creation ;
            frbroo:R17_created ?resource ;
            crm:P9_consists_of ?activity .
        ?activity crm:P2_has_type aat:300404387 ;
            crm:P14_carried_out_by ?agent .
    }

#### Question 2
What are the agents and the types of  activities they carried out to contribute to the creation of `32-exp`?

    SELECT ?agent ?type
    WHERE {
        ?creation_event a frbroo:F28_Expression_Creation ;
            frbroo:R17_created ex:32-exp ;
            crm:P9_consists_of ?activity .
        ?activity crm:P2_has_type ?type ;
            crm:P14_carried_out_by ?agent .
    }

#### Question 3
What are the agents involved in the creation of the CH objects that have been created through the drawing technique? What are the types of the activities they carried out?

    SELECT ?resource ?agent ?type
    WHERE {
        ?creation_event a frbroo:F28_Expression_Creation ;
            crm:P32_used_general_technique aat:300033973 ;
            frbroo:R17_created ?resource ;
            crm:P9_consists_of ?activity .
        ?activity crm:P2_has_type ?type ;
            crm:P14_carried_out_by ?agent .
    }

#### Question 4
What are the identifiers of the manuscript? What are their types?

    SELECT ?resource ?identifier_text ?type
    WHERE {
        ?resource a frbroo:F4_Manifestation_Singleton ;
            crm:P2_has_type aat:300028569 ;
            crm:P48_has_preferred_identifier ?identifier .
        ?identifier crm:P2_has_type ?type ;
            crm:P190_has_symbolic_content ?identifier_text.
    }

#### Question 5
What is the shelf mark of the CH object with the project ID &apos;32&apos;?

    SELECT ?identifier_text
    WHERE {
        ?resource a frbroo:F4_Manifestation_Singleton ;
        crm:P48_has_preferred_identifier ?identifier1 ,
            ?identifier2 .
        ?identifier1 crm:P2_has_type aat:300312355 ;
            crm:P190_has_symbolic_content &quot;32&quot;^^rdfs:Literal .
        ?identifier2 crm:P2_has_type aat:300404704 ;
            crm:P190_has_symbolic_content ?identifier_text.
    }

#### Question 6
What are the descriptive labels of the CH objects that either have shelf marks or are prints?

    SELECT ?resource ?label
    WHERE {
        ?resource a frbroo:F4_Manifestation_Singleton ;
            crm:P48_has_preferred_identifier ?identifier ;
            crm:P2_has_type ?type ;
            crm:P3_has_note ?label .
        ?identifier crm:P2_has_type ?id_type .
        FILTER(?type = aat:300041273 || ?id_type = aat:300404704)
    }

#### Question 7
What are the CH objects whose collections have been curated by agents located in Bologna?

    SELECT ?resource ?agent
    WHERE {
        ?curation a crm:E87_Curation_Activity ;
            crm:P14_carried_out_by ?agent ;
            crm:P12_occurred_in_the_presence_of ?resource .
        ?agent crm:P74_has_current_or_former_residence ex:bologna .
    }

#### Question 8
What are the CH objects and the time spans of their conception events?

    SELECT ?resource ?time_interval
    WHERE {
        ?conception_event a frbroo:F27_Work_Conception ;
            frbroo:R16_initiated ?resource ;
            crm:P4_has_time-span ?time_interval .
    }
    
#### Question 9
What are the titles of the work `32-work`? What are their types?
    
    SELECT ?title ?type ?content
    WHERE {
        ?creation a frbroo:F28_Expression_Creation ;
            frbroo:R19_created_a_realisation_of ex:32-work .
        ex:32-work crm:P102_has_title ?title .
        ?title crm:P2_has_type ?type ;
            crm:P190_has_symbolic_content ?content .
    }

#### Question 10
What are the parent works of the works that have either &apos;ermafrodita&apos; as their subject?
    
    SELECT ?parent ?work ?subject
    WHERE {
        ?creation a frbroo:F28_Expression_Creation ;
            frbroo:R19_created_a_realisation_of ?work ;
            frbroo:R17_created ?expression .
        ?parent a frbroo:F15_Complex_Work ;
            frbroo:R10_has_member ?work .
        ?expression a frbroo:F2_Expression ;
            crm:P129_is_about ex:sub-ermafrodita .
    }

#### Question 11
Which license statements are assigned to the manifestations?
    
    SELECT ?manifestation ?license_link
    WHERE {
        ?license crm:P67_refers_to ?manifestation ;
            crm:P2_has_type aat:300435434 ;
            crm:P70i_is_documented_in ?license_link .
    }

#### Question 12
What is the cultural object digitized and the digital object produced by the digitization process? What is the latter&apos;s license?
     
    SELECT ?input ?output ?license_link
    WHERE {
        ?activity a crmdig:D2_Digitization_Process ;
            crmdig:L1_digitized ?input ;
            crmdig:L11_had_output ?output .
        ?license crm:P2_has_type aat:300435434 ;
            crm:P67_refers_to ?output ;
            crm:P70i_is_documented_in ?license_link .
    }

#### Question 13
What are the starting and ending date times in which the digitization process and the following software activity occurred?

    SELECT ?activity ?start ?end
    WHERE {
        ?activity a crmdig:D2_Digitization_Process;
            crm:P4_has_time-span ?timespan .
        ?timespan crm:P82a_begin_of_the_begin ?start ;
            crm:P82b_end_of_the_end ?end .
    }

#### Question 14
What are the digitization process, its output, the processing activity and its output?

    SELECT ?digitization ?input ?activity ?output
    WHERE {
        ?activity a crmdig:D10_Software_Execution ;
        crm:P2_has_type aat:300054636 ;
        crmdig:L10_had_input ?input ;
        crmdig:L11_had_output ?output .
        ?digitization crmdig:L11_had_output ?input .
    }

#### Question 15
What are the people and institutions who either carried out or were participants in the processing activity?

    SELECT ?person ?institution
    WHERE {
        ?activity a crmdig:D10_Software_Execution ;
        crm:P2_has_type aat:300054636 ;
        crm:P14_carried_out_by ?person ;
        crm:P11_had_participant ?institution .
    }

#### Question 16
What are the techniques used in digitization processes?

    SELECT ?technique ?activity
    WHERE {
        ?activity a crmdig:D2_Digitization_Process ;
            crm:P32_used_general_technique ?technique .
    }

#### Question 17
What are the tools and their types used in processing activities?

    SELECT ?tool ?type
    WHERE {
        ?activity a crmdig:D10_Software_Execution ;
            crm:P2_has_type aat:300054636 ;
            crmdig:L23_used_software_or_firmware ?tool .
        ?tool a crmdig:D14_Software ;
            crm:P2_has_type ?type .
    }
</dc:description>
        <terms:bibliographicCitation xml:lang="en">Barzaghi, S. and Peroni, S. (2024). Cultural Heritage Acquisition and Digitisation Application Profile. https://w3id.org/dharc/ontology/chad-ap.</terms:bibliographicCitation>
        <terms:created rdf:datatype="http://www.w3.org/2001/XMLSchema#date">2024-04-16</terms:created>
        <terms:issued rdf:datatype="http://www.w3.org/2001/XMLSchema#date">2024-04-16</terms:issued>
        <terms:license xml:lang="en">http://creativecommons.org/licenses/by/4.0/</terms:license>
        <terms:title xml:lang="en">Cultural Heritage Acquisition and Digitisation Application Profile (CHAD-AP)</terms:title>
        <vann:preferredNamespacePrefix xml:lang="en">chad-ap</vann:preferredNamespacePrefix>
        <vann:preferredNamespaceUri xml:lang="en">https://w3id.org/dharc/ontology/chad-ap</vann:preferredNamespaceUri>
        <rdfs:comment xml:lang="en">The Cultural Heritage Acquisition and Digitisation Application Profile (CHAD-AP, https://w3id.org/dharc/ontology/chad-ap) is a CIDOC CRM application profile implemented as an OWL ontology that can be logically split into two separate abstract modules: the Object Module (OM), dedicated to describing the CH objects, and the Process Module (PM), for describing the acquisition and digitisation process.</rdfs:comment>
        <owl:versionInfo>1.0.0</owl:versionInfo>
        <ns:status xml:lang="en">work in progress</ns:status>
    </owl:Ontology>
    


    <!-- 
    ///////////////////////////////////////////////////////////////////////////////////////
    //
    // Annotation properties
    //
    ///////////////////////////////////////////////////////////////////////////////////////
     -->


    


    <!-- http://purl.org/dc/elements/1.1/abstract -->


    <owl:AnnotationProperty rdf:about="http://purl.org/dc/elements/1.1/abstract"/>
    


    <!-- http://purl.org/dc/elements/1.1/contributor -->


    <owl:AnnotationProperty rdf:about="http://purl.org/dc/elements/1.1/contributor"/>
    


    <!-- http://purl.org/dc/elements/1.1/creator -->


    <owl:AnnotationProperty rdf:about="http://purl.org/dc/elements/1.1/creator"/>
    


    <!-- http://purl.org/dc/elements/1.1/date -->


    <owl:AnnotationProperty rdf:about="http://purl.org/dc/elements/1.1/date"/>
    


    <!-- http://purl.org/dc/elements/1.1/description -->


    <owl:AnnotationProperty rdf:about="http://purl.org/dc/elements/1.1/description"/>
    


    <!-- http://purl.org/dc/elements/1.1/identifier -->


    <owl:AnnotationProperty rdf:about="http://purl.org/dc/elements/1.1/identifier"/>
    


    <!-- http://purl.org/dc/terms/bibliographicCitation -->


    <owl:AnnotationProperty rdf:about="http://purl.org/dc/terms/bibliographicCitation"/>
    


    <!-- http://purl.org/dc/terms/created -->


    <owl:AnnotationProperty rdf:about="http://purl.org/dc/terms/created"/>
    


    <!-- http://purl.org/dc/terms/issued -->


    <owl:AnnotationProperty rdf:about="http://purl.org/dc/terms/issued"/>
    


    <!-- http://purl.org/dc/terms/license -->


    <owl:AnnotationProperty rdf:about="http://purl.org/dc/terms/license"/>
    


    <!-- http://purl.org/dc/terms/title -->


    <owl:AnnotationProperty rdf:about="http://purl.org/dc/terms/title"/>
    


    <!-- http://purl.org/vocab/vann/preferredNamespacePrefix -->


    <owl:AnnotationProperty rdf:about="http://purl.org/vocab/vann/preferredNamespacePrefix"/>
    


    <!-- http://purl.org/vocab/vann/preferredNamespaceUri -->


    <owl:AnnotationProperty rdf:about="http://purl.org/vocab/vann/preferredNamespaceUri"/>
    


    <!-- http://www.w3.org/2003/06/sw-vocab-status/ns#status -->


    <owl:AnnotationProperty rdf:about="http://www.w3.org/2003/06/sw-vocab-status/ns#status"/>
    


    <!-- http://www.w3.org/2004/02/skos/core#inScheme -->


    <owl:AnnotationProperty rdf:about="http://www.w3.org/2004/02/skos/core#inScheme"/>
    


    <!-- 
    ///////////////////////////////////////////////////////////////////////////////////////
    //
    // Datatypes
    //
    ///////////////////////////////////////////////////////////////////////////////////////
     -->


    


    <!-- http://www.w3.org/2001/XMLSchema#date -->


    <rdfs:Datatype rdf:about="http://www.w3.org/2001/XMLSchema#date"/>
    


    <!-- 
    ///////////////////////////////////////////////////////////////////////////////////////
    //
    // Object Properties
    //
    ///////////////////////////////////////////////////////////////////////////////////////
     -->


    


    <!-- http://iflastandards.info/ns/fr/frbr/frbroo/R10_has_member -->


    <owl:ObjectProperty rdf:about="http://iflastandards.info/ns/fr/frbr/frbroo/R10_has_member">
        <rdfs:domain rdf:resource="http://iflastandards.info/ns/fr/frbr/frbroo/F15_Complex_Work"/>
        <rdfs:range rdf:resource="http://iflastandards.info/ns/fr/frbr/frbroo/F1_Work"/>
        <rdfs:comment xml:lang="en">This property associates a complex work with a work that forms part of it.</rdfs:comment>
        <rdfs:isDefinedBy rdf:resource="http://iflastandards.info/ns/fr/frbr/frbroo/"/>
        <rdfs:label xml:lang="en">has member</rdfs:label>
    </owl:ObjectProperty>
    


    <!-- http://iflastandards.info/ns/fr/frbr/frbroo/R10i_is_member_of -->


    <owl:ObjectProperty rdf:about="http://iflastandards.info/ns/fr/frbr/frbroo/R10i_is_member_of">
        <rdfs:domain rdf:resource="http://iflastandards.info/ns/fr/frbr/frbroo/F1_Work"/>
        <rdfs:range rdf:resource="http://iflastandards.info/ns/fr/frbr/frbroo/F15_Complex_Work"/>
        <rdfs:isDefinedBy rdf:resource="http://iflastandards.info/ns/fr/frbr/frbroo/"/>
        <rdfs:label xml:lang="en">is member of</rdfs:label>
    </owl:ObjectProperty>
    


    <!-- http://iflastandards.info/ns/fr/frbr/frbroo/R17_created -->


    <owl:ObjectProperty rdf:about="http://iflastandards.info/ns/fr/frbr/frbroo/R17_created">
        <rdfs:domain rdf:resource="http://iflastandards.info/ns/fr/frbr/frbroo/F28_Expression_Creation"/>
        <rdfs:range rdf:resource="http://iflastandards.info/ns/fr/frbr/frbroo/F2_Expression"/>
        <rdfs:comment xml:lang="en">This property associates the expression that was first externalised during a particular creation event with that particular creation event.</rdfs:comment>
        <rdfs:isDefinedBy rdf:resource="http://iflastandards.info/ns/fr/frbr/frbroo/"/>
        <rdfs:label xml:lang="en">created</rdfs:label>
    </owl:ObjectProperty>
    


    <!-- http://iflastandards.info/ns/fr/frbr/frbroo/R17i_was_created_by -->


    <owl:ObjectProperty rdf:about="http://iflastandards.info/ns/fr/frbr/frbroo/R17i_was_created_by">
        <rdfs:domain rdf:resource="http://iflastandards.info/ns/fr/frbr/frbroo/F2_Expression"/>
        <rdfs:range rdf:resource="http://iflastandards.info/ns/fr/frbr/frbroo/F28_Expression_Creation"/>
        <rdfs:isDefinedBy rdf:resource="http://iflastandards.info/ns/fr/frbr/frbroo/"/>
        <rdfs:label xml:lang="en">was created by</rdfs:label>
    </owl:ObjectProperty>
    


    <!-- http://iflastandards.info/ns/fr/frbr/frbroo/R18_created -->


    <owl:ObjectProperty rdf:about="http://iflastandards.info/ns/fr/frbr/frbroo/R18_created">
        <rdfs:domain rdf:resource="http://iflastandards.info/ns/fr/frbr/frbroo/F28_Expression_Creation"/>
        <rdfs:range rdf:resource="http://iflastandards.info/ns/fr/frbr/frbroo/F4_Manifestation_Singleton"/>
        <rdfs:comment xml:lang="en">This property associates an expression creation with the first physical objects in which the resulting expression was embodied.</rdfs:comment>
        <rdfs:isDefinedBy rdf:resource="http://iflastandards.info/ns/fr/frbr/frbroo/"/>
        <rdfs:label xml:lang="en">created</rdfs:label>
    </owl:ObjectProperty>
    


    <!-- http://iflastandards.info/ns/fr/frbr/frbroo/R18i_was_created_by -->


    <owl:ObjectProperty rdf:about="http://iflastandards.info/ns/fr/frbr/frbroo/R18i_was_created_by">
        <rdfs:domain rdf:resource="http://iflastandards.info/ns/fr/frbr/frbroo/F4_Manifestation_Singleton"/>
        <rdfs:range rdf:resource="http://iflastandards.info/ns/fr/frbr/frbroo/F28_Expression_Creation"/>
        <rdfs:isDefinedBy rdf:resource="http://iflastandards.info/ns/fr/frbr/frbroo/"/>
        <rdfs:label xml:lang="en">was created by</rdfs:label>
    </owl:ObjectProperty>
    


    <!-- http://iflastandards.info/ns/fr/frbr/frbroo/R19_created_a_realization_of -->


    <owl:ObjectProperty rdf:about="http://iflastandards.info/ns/fr/frbr/frbroo/R19_created_a_realization_of">
        <rdfs:domain rdf:resource="http://iflastandards.info/ns/fr/frbr/frbroo/F28_Expression_Creation"/>
        <rdfs:range rdf:resource="http://iflastandards.info/ns/fr/frbr/frbroo/F1_Work"/>
        <rdfs:comment xml:lang="en">This property associates an expression creation with the corresponding work.</rdfs:comment>
        <rdfs:isDefinedBy rdf:resource="http://iflastandards.info/ns/fr/frbr/frbroo/"/>
        <rdfs:label xml:lang="en">created a realization of</rdfs:label>
    </owl:ObjectProperty>
    


    <!-- http://iflastandards.info/ns/fr/frbr/frbroo/R19i_was_realised_through -->


    <owl:ObjectProperty rdf:about="http://iflastandards.info/ns/fr/frbr/frbroo/R19i_was_realised_through">
        <rdfs:domain rdf:resource="http://iflastandards.info/ns/fr/frbr/frbroo/F1_Work"/>
        <rdfs:range rdf:resource="http://iflastandards.info/ns/fr/frbr/frbroo/F28_Expression_Creation"/>
        <rdfs:isDefinedBy rdf:resource="http://iflastandards.info/ns/fr/frbr/frbroo/"/>
        <rdfs:label xml:lang="en">was realised through</rdfs:label>
    </owl:ObjectProperty>
    


    <!-- http://www.cidoc-crm.org/cidoc-crm/P102_has_title -->


    <owl:ObjectProperty rdf:about="http://www.cidoc-crm.org/cidoc-crm/P102_has_title">
        <rdfs:subPropertyOf rdf:resource="http://www.cidoc-crm.org/cidoc-crm/P1_is_identified_by"/>
        <owl:inverseOf rdf:resource="http://www.cidoc-crm.org/cidoc-crm/P102i_is_title_of"/>
        <rdfs:domain rdf:resource="http://www.cidoc-crm.org/cidoc-crm/E71_Human-Made_Thing"/>
        <rdfs:range rdf:resource="http://www.cidoc-crm.org/cidoc-crm/E35_Title"/>
        <rdfs:comment xml:lang="en">This property associates a title with the work bearing that title.</rdfs:comment>
        <rdfs:isDefinedBy rdf:resource="http://www.cidoc-crm.org/cidoc-crm/"/>
        <rdfs:label xml:lang="fr">a pour titre</rdfs:label>
        <rdfs:label xml:lang="en">has title</rdfs:label>
        <rdfs:label xml:lang="pt">tem título</rdfs:label>
        <rdfs:label xml:lang="de">trägt den Titel</rdfs:label>
        <rdfs:label xml:lang="el">έχει τίτλο</rdfs:label>
        <rdfs:label xml:lang="ru">имеет заголовок</rdfs:label>
        <rdfs:label xml:lang="zh">有题名</rdfs:label>
    </owl:ObjectProperty>
    


    <!-- http://www.cidoc-crm.org/cidoc-crm/P102i_is_title_of -->


    <owl:ObjectProperty rdf:about="http://www.cidoc-crm.org/cidoc-crm/P102i_is_title_of">
        <rdfs:subPropertyOf rdf:resource="http://www.cidoc-crm.org/cidoc-crm/P1i_identifies"/>
        <rdfs:domain rdf:resource="http://www.cidoc-crm.org/cidoc-crm/E35_Title"/>
        <rdfs:range rdf:resource="http://www.cidoc-crm.org/cidoc-crm/E71_Human-Made_Thing"/>
        <rdfs:isDefinedBy rdf:resource="http://www.cidoc-crm.org/cidoc-crm/"/>
        <rdfs:label xml:lang="fr">est le titre de</rdfs:label>
        <rdfs:label xml:lang="en">is title of</rdfs:label>
        <rdfs:label xml:lang="de">ist der Titel von</rdfs:label>
        <rdfs:label xml:lang="pt">é título de</rdfs:label>
        <rdfs:label xml:lang="el">είναι τίτλος του/της</rdfs:label>
        <rdfs:label xml:lang="ru">является заголовком для</rdfs:label>
        <rdfs:label xml:lang="zh">题名是</rdfs:label>
    </owl:ObjectProperty>
    


    <!-- http://www.cidoc-crm.org/cidoc-crm/P10_falls_within -->


    <owl:ObjectProperty rdf:about="http://www.cidoc-crm.org/cidoc-crm/P10_falls_within"/>
    


    <!-- http://www.cidoc-crm.org/cidoc-crm/P10i_contains -->


    <owl:ObjectProperty rdf:about="http://www.cidoc-crm.org/cidoc-crm/P10i_contains"/>
    


    <!-- http://www.cidoc-crm.org/cidoc-crm/P11_had_participant -->


    <owl:ObjectProperty rdf:about="http://www.cidoc-crm.org/cidoc-crm/P11_had_participant">
        <rdfs:subPropertyOf rdf:resource="http://www.cidoc-crm.org/cidoc-crm/P12_occurred_in_the_presence_of"/>
        <rdfs:domain rdf:resource="http://www.cidoc-crm.org/cidoc-crm/E5_Event"/>
        <rdfs:range rdf:resource="http://www.cidoc-crm.org/cidoc-crm/E39_Actor"/>
        <rdfs:comment xml:lang="en">This property describes the participation of one or more actors in an event.</rdfs:comment>
        <rdfs:isDefinedBy rdf:resource="http://www.cidoc-crm.org/cidoc-crm/"/>
        <rdfs:label xml:lang="fr">a eu pour actant participant</rdfs:label>
        <rdfs:label xml:lang="en">had participant</rdfs:label>
        <rdfs:label xml:lang="de">hatte Teilnehmer</rdfs:label>
        <rdfs:label xml:lang="pt">tem participante</rdfs:label>
        <rdfs:label xml:lang="el">είχε συμμέτοχο</rdfs:label>
        <rdfs:label xml:lang="ru">имел участника</rdfs:label>
        <rdfs:label xml:lang="zh">有参与者</rdfs:label>
    </owl:ObjectProperty>
    


    <!-- http://www.cidoc-crm.org/cidoc-crm/P11i_participated_in -->


    <owl:ObjectProperty rdf:about="http://www.cidoc-crm.org/cidoc-crm/P11i_participated_in">
        <rdfs:subPropertyOf rdf:resource="http://www.cidoc-crm.org/cidoc-crm/P12i_was_present_at"/>
        <owl:inverseOf rdf:resource="http://www.cidoc-crm.org/cidoc-crm/P11_had_participant"/>
        <rdfs:domain rdf:resource="http://www.cidoc-crm.org/cidoc-crm/E39_Actor"/>
        <rdfs:range rdf:resource="http://www.cidoc-crm.org/cidoc-crm/E5_Event"/>
        <rdfs:isDefinedBy rdf:resource="http://www.cidoc-crm.org/cidoc-crm/"/>
        <rdfs:label xml:lang="fr">a participé à</rdfs:label>
        <rdfs:label xml:lang="de">nahm Teil an</rdfs:label>
        <rdfs:label xml:lang="pt">participa em</rdfs:label>
        <rdfs:label xml:lang="en">participated in</rdfs:label>
        <rdfs:label xml:lang="el">συμμετείχε σε</rdfs:label>
        <rdfs:label xml:lang="ru">участвовал в</rdfs:label>
        <rdfs:label xml:lang="zh">参与</rdfs:label>
    </owl:ObjectProperty>
    


    <!-- http://www.cidoc-crm.org/cidoc-crm/P125_used_object_of_type -->


    <owl:ObjectProperty rdf:about="http://www.cidoc-crm.org/cidoc-crm/P125_used_object_of_type"/>
    


    <!-- http://www.cidoc-crm.org/cidoc-crm/P129_is_about -->


    <owl:ObjectProperty rdf:about="http://www.cidoc-crm.org/cidoc-crm/P129_is_about">
        <rdfs:subPropertyOf rdf:resource="http://www.cidoc-crm.org/cidoc-crm/P67_refers_to"/>
        <rdfs:domain rdf:resource="http://www.cidoc-crm.org/cidoc-crm/E89_Propositional_Object"/>
        <rdfs:range rdf:resource="http://www.cidoc-crm.org/cidoc-crm/E1_CRM_Entity"/>
        <rdfs:comment xml:lang="en">This property documents that an expression has as subject some entity.</rdfs:comment>
        <rdfs:isDefinedBy rdf:resource="http://www.cidoc-crm.org/cidoc-crm/"/>
        <rdfs:label xml:lang="fr">a pour sujet</rdfs:label>
        <rdfs:label xml:lang="de">handelt über</rdfs:label>
        <rdfs:label xml:lang="en">is about</rdfs:label>
        <rdfs:label xml:lang="pt">é sobre</rdfs:label>
        <rdfs:label xml:lang="el">έχει ως θέμα</rdfs:label>
        <rdfs:label xml:lang="ru">касается</rdfs:label>
        <rdfs:label xml:lang="zh">有关</rdfs:label>
    </owl:ObjectProperty>
    


    <!-- http://www.cidoc-crm.org/cidoc-crm/P129i_is_subject_of -->


    <owl:ObjectProperty rdf:about="http://www.cidoc-crm.org/cidoc-crm/P129i_is_subject_of">
        <rdfs:subPropertyOf rdf:resource="http://www.cidoc-crm.org/cidoc-crm/P67i_is_referred_to_by"/>
        <owl:inverseOf rdf:resource="http://www.cidoc-crm.org/cidoc-crm/P129_is_about"/>
        <rdfs:domain rdf:resource="http://www.cidoc-crm.org/cidoc-crm/E1_CRM_Entity"/>
        <rdfs:range rdf:resource="http://www.cidoc-crm.org/cidoc-crm/E89_Propositional_Object"/>
        <rdfs:isDefinedBy rdf:resource="http://www.cidoc-crm.org/cidoc-crm/"/>
        <rdfs:label xml:lang="fr">est le sujet de</rdfs:label>
        <rdfs:label xml:lang="en">is subject of</rdfs:label>
        <rdfs:label xml:lang="de">wird behandelt in</rdfs:label>
        <rdfs:label xml:lang="pt">é assunto de</rdfs:label>
        <rdfs:label xml:lang="el">είναι θέμα του/της</rdfs:label>
        <rdfs:label xml:lang="ru">является предметом для</rdfs:label>
        <rdfs:label xml:lang="zh">是主题</rdfs:label>
    </owl:ObjectProperty>
    


    <!-- http://www.cidoc-crm.org/cidoc-crm/P12_occurred_in_the_presence_of -->


    <owl:ObjectProperty rdf:about="http://www.cidoc-crm.org/cidoc-crm/P12_occurred_in_the_presence_of">
        <rdfs:domain rdf:resource="http://www.cidoc-crm.org/cidoc-crm/E5_Event"/>
        <rdfs:range rdf:resource="http://www.cidoc-crm.org/cidoc-crm/E77_Persistent_Item"/>
        <rdfs:comment xml:lang="en">This property describes the presence of an entity during an event, without implying any specific role.</rdfs:comment>
        <rdfs:isDefinedBy rdf:resource="http://www.cidoc-crm.org/cidoc-crm/"/>
        <rdfs:label xml:lang="fr">a eu lieu en présence de</rdfs:label>
        <rdfs:label xml:lang="de">fand statt im Beisein von</rdfs:label>
        <rdfs:label xml:lang="en">occurred in the presence of</rdfs:label>
        <rdfs:label xml:lang="pt">ocorreu na presença de</rdfs:label>
        <rdfs:label xml:lang="el">συνέβη παρουσία του/της</rdfs:label>
        <rdfs:label xml:lang="ru">появился в присутствии</rdfs:label>
        <rdfs:label xml:lang="zh">已出现</rdfs:label>
    </owl:ObjectProperty>
    


    <!-- http://www.cidoc-crm.org/cidoc-crm/P12i_was_present_at -->


    <owl:ObjectProperty rdf:about="http://www.cidoc-crm.org/cidoc-crm/P12i_was_present_at">
        <owl:inverseOf rdf:resource="http://www.cidoc-crm.org/cidoc-crm/P12_occurred_in_the_presence_of"/>
        <rdfs:domain rdf:resource="http://www.cidoc-crm.org/cidoc-crm/E77_Persistent_Item"/>
        <rdfs:range rdf:resource="http://www.cidoc-crm.org/cidoc-crm/E5_Event"/>
        <rdfs:isDefinedBy rdf:resource="http://www.cidoc-crm.org/cidoc-crm/"/>
        <rdfs:label xml:lang="fr">a été présent à</rdfs:label>
        <rdfs:label xml:lang="pt">estava presente no</rdfs:label>
        <rdfs:label xml:lang="de">war anwesend bei</rdfs:label>
        <rdfs:label xml:lang="en">was present at</rdfs:label>
        <rdfs:label xml:lang="el">ήταν παρών/παρούσα/παρόν σε</rdfs:label>
        <rdfs:label xml:lang="ru">присутствовал при</rdfs:label>
        <rdfs:label xml:lang="zh">出现在</rdfs:label>
    </owl:ObjectProperty>
    


    <!-- http://www.cidoc-crm.org/cidoc-crm/P147_curated -->


    <owl:ObjectProperty rdf:about="http://www.cidoc-crm.org/cidoc-crm/P147_curated">
        <rdfs:domain rdf:resource="http://www.cidoc-crm.org/cidoc-crm/E87_Curation_Activity"/>
        <rdfs:range rdf:resource="http://www.cidoc-crm.org/cidoc-crm/E78_Curated_Holding"/>
        <rdfs:comment xml:lang="en">This property associates a curation activity with a collection involved in such activity.</rdfs:comment>
        <rdfs:isDefinedBy rdf:resource="http://www.cidoc-crm.org/cidoc-crm/"/>
        <rdfs:label xml:lang="fr">a géré</rdfs:label>
        <rdfs:label xml:lang="de">betreute kuratorisch</rdfs:label>
        <rdfs:label xml:lang="en">curated</rdfs:label>
        <rdfs:label xml:lang="zh">管理</rdfs:label>
    </owl:ObjectProperty>
    


    <!-- http://www.cidoc-crm.org/cidoc-crm/P147i_was_curated_by -->


    <owl:ObjectProperty rdf:about="http://www.cidoc-crm.org/cidoc-crm/P147i_was_curated_by">
        <owl:inverseOf rdf:resource="http://www.cidoc-crm.org/cidoc-crm/P147_curated"/>
        <rdfs:domain rdf:resource="http://www.cidoc-crm.org/cidoc-crm/E78_Curated_Holding"/>
        <rdfs:range rdf:resource="http://www.cidoc-crm.org/cidoc-crm/E87_Curation_Activity"/>
        <rdfs:isDefinedBy rdf:resource="http://www.cidoc-crm.org/cidoc-crm/"/>
        <rdfs:label xml:lang="fr">a été géré par</rdfs:label>
        <rdfs:label xml:lang="en">was curated by</rdfs:label>
        <rdfs:label xml:lang="de">wurde kuratorisch betreut durch</rdfs:label>
        <rdfs:label xml:lang="zh">被管理</rdfs:label>
    </owl:ObjectProperty>
    


    <!-- http://www.cidoc-crm.org/cidoc-crm/P14_carried_out_by -->


    <owl:ObjectProperty rdf:about="http://www.cidoc-crm.org/cidoc-crm/P14_carried_out_by">
        <rdfs:subPropertyOf rdf:resource="http://www.cidoc-crm.org/cidoc-crm/P11_had_participant"/>
        <owl:inverseOf rdf:resource="http://www.cidoc-crm.org/cidoc-crm/P14i_performed"/>
        <rdfs:domain rdf:resource="http://www.cidoc-crm.org/cidoc-crm/E7_Activity"/>
        <rdfs:range rdf:resource="http://www.cidoc-crm.org/cidoc-crm/E39_Actor"/>
        <rdfs:comment xml:lang="en">This property describes the active, accountable participation of an actor during an activity.</rdfs:comment>
        <rdfs:isDefinedBy rdf:resource="http://www.cidoc-crm.org/cidoc-crm/"/>
        <rdfs:label xml:lang="fr">a été effectué par</rdfs:label>
        <rdfs:label xml:lang="en">carried out by</rdfs:label>
        <rdfs:label xml:lang="pt">realizada por</rdfs:label>
        <rdfs:label xml:lang="de">wurde ausgeführt von</rdfs:label>
        <rdfs:label xml:lang="el">πραγματοποιήθηκε από</rdfs:label>
        <rdfs:label xml:lang="ru">выполнялся</rdfs:label>
        <rdfs:label xml:lang="zh">执行者是</rdfs:label>
    </owl:ObjectProperty>
    


    <!-- http://www.cidoc-crm.org/cidoc-crm/P14i_performed -->


    <owl:ObjectProperty rdf:about="http://www.cidoc-crm.org/cidoc-crm/P14i_performed">
        <rdfs:subPropertyOf rdf:resource="http://www.cidoc-crm.org/cidoc-crm/P11i_participated_in"/>
        <rdfs:domain rdf:resource="http://www.cidoc-crm.org/cidoc-crm/E39_Actor"/>
        <rdfs:range rdf:resource="http://www.cidoc-crm.org/cidoc-crm/E7_Activity"/>
        <rdfs:isDefinedBy rdf:resource="http://www.cidoc-crm.org/cidoc-crm/"/>
        <rdfs:label xml:lang="fr">a effectué</rdfs:label>
        <rdfs:label xml:lang="pt">executou</rdfs:label>
        <rdfs:label xml:lang="de">führte aus</rdfs:label>
        <rdfs:label xml:lang="en">performed</rdfs:label>
        <rdfs:label xml:lang="el">πραγματοποίησε</rdfs:label>
        <rdfs:label xml:lang="ru">выполнял</rdfs:label>
        <rdfs:label xml:lang="zh">执行</rdfs:label>
    </owl:ObjectProperty>
    


    <!-- http://www.cidoc-crm.org/cidoc-crm/P15_was_influenced_by -->


    <owl:ObjectProperty rdf:about="http://www.cidoc-crm.org/cidoc-crm/P15_was_influenced_by"/>
    


    <!-- http://www.cidoc-crm.org/cidoc-crm/P15i_influenced -->


    <owl:ObjectProperty rdf:about="http://www.cidoc-crm.org/cidoc-crm/P15i_influenced"/>
    


    <!-- http://www.cidoc-crm.org/cidoc-crm/P16_used_specific_object -->


    <owl:ObjectProperty rdf:about="http://www.cidoc-crm.org/cidoc-crm/P16_used_specific_object">
        <rdfs:subPropertyOf rdf:resource="http://www.cidoc-crm.org/cidoc-crm/P12_occurred_in_the_presence_of"/>
        <rdfs:subPropertyOf rdf:resource="http://www.cidoc-crm.org/cidoc-crm/P15_was_influenced_by"/>
        <owl:inverseOf rdf:resource="http://www.cidoc-crm.org/cidoc-crm/P16i_was_used_for"/>
        <rdfs:domain rdf:resource="http://www.cidoc-crm.org/cidoc-crm/E7_Activity"/>
        <rdfs:range rdf:resource="http://www.cidoc-crm.org/cidoc-crm/E70_Thing"/>
        <rdfs:comment xml:lang="en">This property describes the use of a tool for performing an activity.</rdfs:comment>
        <rdfs:isDefinedBy rdf:resource="http://www.cidoc-crm.org/cidoc-crm/"/>
        <rdfs:label xml:lang="fr">a mobilisé l’objet spécifique</rdfs:label>
        <rdfs:label xml:lang="de">benutzte das bestimmte Objekt</rdfs:label>
        <rdfs:label xml:lang="en">used specific object</rdfs:label>
        <rdfs:label xml:lang="pt">usou objeto específico</rdfs:label>
        <rdfs:label xml:lang="el">χρησιμοποίησε αντικείμενο</rdfs:label>
        <rdfs:label xml:lang="ru">использовал особый объект</rdfs:label>
        <rdfs:label xml:lang="zh">使用特定对象</rdfs:label>
    </owl:ObjectProperty>
    


    <!-- http://www.cidoc-crm.org/cidoc-crm/P16i_was_used_for -->


    <owl:ObjectProperty rdf:about="http://www.cidoc-crm.org/cidoc-crm/P16i_was_used_for">
        <rdfs:subPropertyOf rdf:resource="http://www.cidoc-crm.org/cidoc-crm/P12i_was_present_at"/>
        <rdfs:subPropertyOf rdf:resource="http://www.cidoc-crm.org/cidoc-crm/P15i_influenced"/>
        <rdfs:domain rdf:resource="http://www.cidoc-crm.org/cidoc-crm/E70_Thing"/>
        <rdfs:range rdf:resource="http://www.cidoc-crm.org/cidoc-crm/E7_Activity"/>
        <rdfs:isDefinedBy rdf:resource="http://www.cidoc-crm.org/cidoc-crm/"/>
        <rdfs:label xml:lang="fr">a été mobilisé pour</rdfs:label>
        <rdfs:label xml:lang="pt">foi usado por</rdfs:label>
        <rdfs:label xml:lang="en">was used for</rdfs:label>
        <rdfs:label xml:lang="de">wurde benutzt für</rdfs:label>
        <rdfs:label xml:lang="el">χρησιμοποιήθηκε για</rdfs:label>
        <rdfs:label xml:lang="ru">был использован для</rdfs:label>
        <rdfs:label xml:lang="zh">用于</rdfs:label>
    </owl:ObjectProperty>
    


    <!-- http://www.cidoc-crm.org/cidoc-crm/P1_is_identified_by -->


    <owl:ObjectProperty rdf:about="http://www.cidoc-crm.org/cidoc-crm/P1_is_identified_by"/>
    


    <!-- http://www.cidoc-crm.org/cidoc-crm/P1i_identifies -->


    <owl:ObjectProperty rdf:about="http://www.cidoc-crm.org/cidoc-crm/P1i_identifies"/>
    


    <!-- http://www.cidoc-crm.org/cidoc-crm/P2_has_type -->


    <owl:ObjectProperty rdf:about="http://www.cidoc-crm.org/cidoc-crm/P2_has_type">
        <rdfs:domain rdf:resource="http://www.cidoc-crm.org/cidoc-crm/E1_CRM_Entity"/>
        <rdfs:range rdf:resource="http://www.cidoc-crm.org/cidoc-crm/E55_Type"/>
        <rdfs:comment xml:lang="en">This property allows typing of an entity through the use of an external knowledge organization system, such as a thesaurus or a controlled vocabulary.</rdfs:comment>
        <rdfs:isDefinedBy rdf:resource="http://www.cidoc-crm.org/cidoc-crm/"/>
        <rdfs:label xml:lang="fr">a pour type</rdfs:label>
        <rdfs:label xml:lang="en">has type</rdfs:label>
        <rdfs:label xml:lang="de">hat den Typus</rdfs:label>
        <rdfs:label xml:lang="pt">é do tipo</rdfs:label>
        <rdfs:label xml:lang="el">έχει τύπο</rdfs:label>
        <rdfs:label xml:lang="ru">имеет тип</rdfs:label>
        <rdfs:label xml:lang="zh">有类型</rdfs:label>
    </owl:ObjectProperty>
    


    <!-- http://www.cidoc-crm.org/cidoc-crm/P32_used_general_technique -->


    <owl:ObjectProperty rdf:about="http://www.cidoc-crm.org/cidoc-crm/P32_used_general_technique">
        <rdfs:subPropertyOf rdf:resource="http://www.cidoc-crm.org/cidoc-crm/P125_used_object_of_type"/>
        <owl:inverseOf rdf:resource="http://www.cidoc-crm.org/cidoc-crm/P32i_was_technique_of"/>
        <rdfs:domain rdf:resource="http://www.cidoc-crm.org/cidoc-crm/E7_Activity"/>
        <rdfs:range rdf:resource="http://www.cidoc-crm.org/cidoc-crm/E55_Type"/>
        <rdfs:comment xml:lang="en">This property identifies the technique or method that was employed during an activity.</rdfs:comment>
        <rdfs:isDefinedBy rdf:resource="http://www.cidoc-crm.org/cidoc-crm/"/>
        <rdfs:label xml:lang="fr">a mobilisé comme technique générale</rdfs:label>
        <rdfs:label xml:lang="de">benutzte das allgemeine Verfahren</rdfs:label>
        <rdfs:label xml:lang="en">used general technique</rdfs:label>
        <rdfs:label xml:lang="pt">usou técnica geral</rdfs:label>
        <rdfs:label xml:lang="el">χρησιμοποίησε γενική τεχνική</rdfs:label>
        <rdfs:label xml:lang="ru">использовал общую технику</rdfs:label>
        <rdfs:label xml:lang="zh">使用通用技术</rdfs:label>
    </owl:ObjectProperty>
    


    <!-- http://www.cidoc-crm.org/cidoc-crm/P32i_was_technique_of -->


    <owl:ObjectProperty rdf:about="http://www.cidoc-crm.org/cidoc-crm/P32i_was_technique_of"/>
    


    <!-- http://www.cidoc-crm.org/cidoc-crm/P39_measured -->


    <owl:ObjectProperty rdf:about="http://www.cidoc-crm.org/cidoc-crm/P39_measured"/>
    


    <!-- http://www.cidoc-crm.org/cidoc-crm/P39i_was_measured_by -->


    <owl:ObjectProperty rdf:about="http://www.cidoc-crm.org/cidoc-crm/P39i_was_measured_by"/>
    


    <!-- http://www.cidoc-crm.org/cidoc-crm/P46_is_composed_of -->


    <owl:ObjectProperty rdf:about="http://www.cidoc-crm.org/cidoc-crm/P46_is_composed_of">
        <rdfs:domain rdf:resource="http://www.cidoc-crm.org/cidoc-crm/E18_Physical_Thing"/>
        <rdfs:range rdf:resource="http://www.cidoc-crm.org/cidoc-crm/E18_Physical_Thing"/>
        <rdfs:comment xml:lang="en">This property associates a physical entity with another physical entity that forms part of it.</rdfs:comment>
        <rdfs:isDefinedBy rdf:resource="http://www.cidoc-crm.org/cidoc-crm/"/>
        <rdfs:label xml:lang="fr">est composé de</rdfs:label>
        <rdfs:label xml:lang="en">is composed of</rdfs:label>
        <rdfs:label xml:lang="de">ist zusammengesetzt aus</rdfs:label>
        <rdfs:label xml:lang="pt">é composto de</rdfs:label>
        <rdfs:label xml:lang="el">αποτελείται από</rdfs:label>
        <rdfs:label xml:lang="ru">составлен из</rdfs:label>
        <rdfs:label xml:lang="zh">组成成分是</rdfs:label>
    </owl:ObjectProperty>
    


    <!-- http://www.cidoc-crm.org/cidoc-crm/P46i_forms_part_of -->


    <owl:ObjectProperty rdf:about="http://www.cidoc-crm.org/cidoc-crm/P46i_forms_part_of">
        <owl:inverseOf rdf:resource="http://www.cidoc-crm.org/cidoc-crm/P46_is_composed_of"/>
        <rdfs:domain rdf:resource="http://www.cidoc-crm.org/cidoc-crm/E18_Physical_Thing"/>
        <rdfs:range rdf:resource="http://www.cidoc-crm.org/cidoc-crm/E18_Physical_Thing"/>
        <rdfs:isDefinedBy rdf:resource="http://www.cidoc-crm.org/cidoc-crm/"/>
        <rdfs:label xml:lang="de">bildet Teil von</rdfs:label>
        <rdfs:label xml:lang="fr">fait partie de</rdfs:label>
        <rdfs:label xml:lang="pt">faz parte de</rdfs:label>
        <rdfs:label xml:lang="en">forms part of</rdfs:label>
        <rdfs:label xml:lang="el">αποτελεί μέρος του/της</rdfs:label>
        <rdfs:label xml:lang="ru">формирует часть</rdfs:label>
        <rdfs:label xml:lang="zh">构成部分</rdfs:label>
    </owl:ObjectProperty>
    


    <!-- http://www.cidoc-crm.org/cidoc-crm/P48_has_preferred_identifier -->


    <owl:ObjectProperty rdf:about="http://www.cidoc-crm.org/cidoc-crm/P48_has_preferred_identifier">
        <rdfs:subPropertyOf rdf:resource="http://www.cidoc-crm.org/cidoc-crm/P1_is_identified_by"/>
        <rdfs:domain rdf:resource="http://www.cidoc-crm.org/cidoc-crm/E1_CRM_Entity"/>
        <rdfs:range rdf:resource="http://www.cidoc-crm.org/cidoc-crm/E42_Identifier"/>
        <rdfs:comment xml:lang="en">This property records the preferred identifier used to identify an entity.</rdfs:comment>
        <rdfs:isDefinedBy rdf:resource="http://www.cidoc-crm.org/cidoc-crm/"/>
        <rdfs:label xml:lang="fr">a pour identifiant préférentiel</rdfs:label>
        <rdfs:label xml:lang="en">has preferred identifier</rdfs:label>
        <rdfs:label xml:lang="de">hat bevorzugtes Kennzeichen</rdfs:label>
        <rdfs:label xml:lang="pt">tem identificador preferido</rdfs:label>
        <rdfs:label xml:lang="el">έχει προτιμώμενο αναγνωριστικό</rdfs:label>
        <rdfs:label xml:lang="ru">имеет предпочтительный идентификатор</rdfs:label>
        <rdfs:label xml:lang="zh">有优选标识符</rdfs:label>
    </owl:ObjectProperty>
    


    <!-- http://www.cidoc-crm.org/cidoc-crm/P48i_is_preferred_identifier_of -->


    <owl:ObjectProperty rdf:about="http://www.cidoc-crm.org/cidoc-crm/P48i_is_preferred_identifier_of">
        <rdfs:subPropertyOf rdf:resource="http://www.cidoc-crm.org/cidoc-crm/P1i_identifies"/>
        <owl:inverseOf rdf:resource="http://www.cidoc-crm.org/cidoc-crm/P48_has_preferred_identifier"/>
        <rdfs:domain rdf:resource="http://www.cidoc-crm.org/cidoc-crm/E42_Identifier"/>
        <rdfs:range rdf:resource="http://www.cidoc-crm.org/cidoc-crm/E1_CRM_Entity"/>
        <rdfs:isDefinedBy rdf:resource="http://www.cidoc-crm.org/cidoc-crm/"/>
        <rdfs:label xml:lang="fr">est l’identifiant préférentiel de</rdfs:label>
        <rdfs:label xml:lang="en">is preferred identifier of</rdfs:label>
        <rdfs:label xml:lang="de">ist bevorzugtes Kennzeichen für</rdfs:label>
        <rdfs:label xml:lang="pt">é o identificador preferido de</rdfs:label>
        <rdfs:label xml:lang="el">είναι προτιμώμενο αναγνωριστικό</rdfs:label>
        <rdfs:label xml:lang="ru">является предпочтительным идентификатором для</rdfs:label>
        <rdfs:label xml:lang="zh">是优选标识符</rdfs:label>
    </owl:ObjectProperty>
    


    <!-- http://www.cidoc-crm.org/cidoc-crm/P49_has_former_or_current_keeper -->


    <owl:ObjectProperty rdf:about="http://www.cidoc-crm.org/cidoc-crm/P49_has_former_or_current_keeper">
        <rdfs:domain rdf:resource="http://www.cidoc-crm.org/cidoc-crm/E18_Physical_Thing"/>
        <rdfs:range rdf:resource="http://www.cidoc-crm.org/cidoc-crm/E39_Actor"/>
        <rdfs:comment xml:lang="en">This property identifies an actor who has or has had custody of a physical entity at some time.</rdfs:comment>
        <rdfs:isDefinedBy rdf:resource="http://www.cidoc-crm.org/cidoc-crm/"/>
        <rdfs:label xml:lang="fr">a pour actant détenteur actuel ou antérieur</rdfs:label>
        <rdfs:label xml:lang="en">has former or current keeper</rdfs:label>
        <rdfs:label xml:lang="de">hat früheren oder derzeitigen Betreuer</rdfs:label>
        <rdfs:label xml:lang="pt">é ou foi guardada por</rdfs:label>
        <rdfs:label xml:lang="el">είναι ή ήταν στην κατοχή του</rdfs:label>
        <rdfs:label xml:lang="ru">имеет бывшего или текущего смотрителя</rdfs:label>
        <rdfs:label xml:lang="zh">有以往或当前保管者</rdfs:label>
    </owl:ObjectProperty>
    


    <!-- http://www.cidoc-crm.org/cidoc-crm/P49i_is_former_or_current_keeper_of -->


    <owl:ObjectProperty rdf:about="http://www.cidoc-crm.org/cidoc-crm/P49i_is_former_or_current_keeper_of">
        <owl:inverseOf rdf:resource="http://www.cidoc-crm.org/cidoc-crm/P49_has_former_or_current_keeper"/>
        <rdfs:domain rdf:resource="http://www.cidoc-crm.org/cidoc-crm/E39_Actor"/>
        <rdfs:range rdf:resource="http://www.cidoc-crm.org/cidoc-crm/E18_Physical_Thing"/>
        <rdfs:isDefinedBy rdf:resource="http://www.cidoc-crm.org/cidoc-crm/"/>
        <rdfs:label xml:lang="fr">est l’actant détenteur actuel ou antérieur de</rdfs:label>
        <rdfs:label xml:lang="en">is former or current keeper of</rdfs:label>
        <rdfs:label xml:lang="de">ist früherer oder derzeitiger Betreuer von</rdfs:label>
        <rdfs:label xml:lang="pt">é ou foi guardador de</rdfs:label>
        <rdfs:label xml:lang="el">κατέχει ή κατείχε</rdfs:label>
        <rdfs:label xml:lang="ru">является бывшим или текущим смотрителем для</rdfs:label>
        <rdfs:label xml:lang="zh">是以往或当前保管者</rdfs:label>
    </owl:ObjectProperty>
    


    <!-- http://www.cidoc-crm.org/cidoc-crm/P4_has_time-span -->


    <owl:ObjectProperty rdf:about="http://www.cidoc-crm.org/cidoc-crm/P4_has_time-span">
        <owl:inverseOf rdf:resource="http://www.cidoc-crm.org/cidoc-crm/P4i_is_time-span_of"/>
        <rdfs:domain rdf:resource="http://www.cidoc-crm.org/cidoc-crm/E2_Temporal_Entity"/>
        <rdfs:range rdf:resource="http://www.cidoc-crm.org/cidoc-crm/E52_Time-Span"/>
        <rdfs:comment xml:lang="en">This property associates a phenomenon with the time span during which that phenomenon was on-going.</rdfs:comment>
        <rdfs:isDefinedBy rdf:resource="http://www.cidoc-crm.org/cidoc-crm/"/>
        <rdfs:label xml:lang="fr">a pour intervalle temporel</rdfs:label>
        <rdfs:label xml:lang="en">has time-span</rdfs:label>
        <rdfs:label xml:lang="de">hat Zeitspanne</rdfs:label>
        <rdfs:label xml:lang="pt">tem período de tempo</rdfs:label>
        <rdfs:label xml:lang="el">βρισκόταν σε εξέλιξη</rdfs:label>
        <rdfs:label xml:lang="ru">имеет временной отрезок</rdfs:label>
        <rdfs:label xml:lang="zh">发生时段是</rdfs:label>
    </owl:ObjectProperty>
    


    <!-- http://www.cidoc-crm.org/cidoc-crm/P4i_is_time-span_of -->


    <owl:ObjectProperty rdf:about="http://www.cidoc-crm.org/cidoc-crm/P4i_is_time-span_of">
        <rdfs:domain rdf:resource="http://www.cidoc-crm.org/cidoc-crm/E52_Time-Span"/>
        <rdfs:range rdf:resource="http://www.cidoc-crm.org/cidoc-crm/E2_Temporal_Entity"/>
        <rdfs:isDefinedBy rdf:resource="http://www.cidoc-crm.org/cidoc-crm/"/>
        <rdfs:label xml:lang="fr">est l’intervalle temporel de</rdfs:label>
        <rdfs:label xml:lang="en">is time-span of</rdfs:label>
        <rdfs:label xml:lang="de">ist Zeitspanne von</rdfs:label>
        <rdfs:label xml:lang="pt">é o período de tempo de</rdfs:label>
        <rdfs:label xml:lang="el">είναι χρονικό διάστημα του/της</rdfs:label>
        <rdfs:label xml:lang="ru">является временным отрезком для</rdfs:label>
        <rdfs:label xml:lang="zh">是时段</rdfs:label>
    </owl:ObjectProperty>
    


    <!-- http://www.cidoc-crm.org/cidoc-crm/P62_depicts -->


    <owl:ObjectProperty rdf:about="http://www.cidoc-crm.org/cidoc-crm/P62_depicts">
        <rdfs:domain rdf:resource="http://www.cidoc-crm.org/cidoc-crm/E24_Physical_Human-Made_Thing"/>
        <rdfs:range rdf:resource="http://www.cidoc-crm.org/cidoc-crm/E1_CRM_Entity"/>
        <rdfs:comment xml:lang="en">This property identifies some entity that is depicted by a physical object.</rdfs:comment>
        <rdfs:isDefinedBy rdf:resource="http://www.cidoc-crm.org/cidoc-crm/"/>
        <rdfs:label xml:lang="de">bildet ab</rdfs:label>
        <rdfs:label xml:lang="en">depicts</rdfs:label>
        <rdfs:label xml:lang="fr">illustre</rdfs:label>
        <rdfs:label xml:lang="pt">retrata</rdfs:label>
        <rdfs:label xml:lang="el">απεικονίζει</rdfs:label>
        <rdfs:label xml:lang="ru">описывает</rdfs:label>
        <rdfs:label xml:lang="zh">描绘了</rdfs:label>
    </owl:ObjectProperty>
    


    <!-- http://www.cidoc-crm.org/cidoc-crm/P62i_is_depicted_by -->


    <owl:ObjectProperty rdf:about="http://www.cidoc-crm.org/cidoc-crm/P62i_is_depicted_by">
        <owl:inverseOf rdf:resource="http://www.cidoc-crm.org/cidoc-crm/P62_depicts"/>
        <rdfs:domain rdf:resource="http://www.cidoc-crm.org/cidoc-crm/E1_CRM_Entity"/>
        <rdfs:range rdf:resource="http://www.cidoc-crm.org/cidoc-crm/E24_Physical_Human-Made_Thing"/>
        <rdfs:isDefinedBy rdf:resource="http://www.cidoc-crm.org/cidoc-crm/"/>
        <rdfs:label xml:lang="fr">est illustré par</rdfs:label>
        <rdfs:label xml:lang="en">is depicted by</rdfs:label>
        <rdfs:label xml:lang="de">wird abgebildet durch</rdfs:label>
        <rdfs:label xml:lang="pt">é retratada por</rdfs:label>
        <rdfs:label xml:lang="el">απεικονίζεται σε</rdfs:label>
        <rdfs:label xml:lang="ru">описан посредством</rdfs:label>
        <rdfs:label xml:lang="zh">被描绘</rdfs:label>
    </owl:ObjectProperty>
    


    <!-- http://www.cidoc-crm.org/cidoc-crm/P67_refers_to -->


    <owl:ObjectProperty rdf:about="http://www.cidoc-crm.org/cidoc-crm/P67_refers_to">
        <rdfs:domain rdf:resource="http://www.cidoc-crm.org/cidoc-crm/E89_Propositional_Object"/>
        <rdfs:range rdf:resource="http://www.cidoc-crm.org/cidoc-crm/E1_CRM_Entity"/>
        <rdfs:comment xml:lang="en">This property documents that some statement refers to a cultural heritage object.</rdfs:comment>
        <rdfs:isDefinedBy rdf:resource="http://www.cidoc-crm.org/cidoc-crm/"/>
        <rdfs:label xml:lang="pt">referencia</rdfs:label>
        <rdfs:label xml:lang="en">refers to</rdfs:label>
        <rdfs:label xml:lang="fr">renvoie à</rdfs:label>
        <rdfs:label xml:lang="de">verweist auf</rdfs:label>
        <rdfs:label xml:lang="el">αναφέρεται σε</rdfs:label>
        <rdfs:label xml:lang="ru">ссылается на</rdfs:label>
        <rdfs:label xml:lang="zh">涉及</rdfs:label>
    </owl:ObjectProperty>
    


    <!-- http://www.cidoc-crm.org/cidoc-crm/P67i_is_referred_to_by -->


    <owl:ObjectProperty rdf:about="http://www.cidoc-crm.org/cidoc-crm/P67i_is_referred_to_by">
        <owl:inverseOf rdf:resource="http://www.cidoc-crm.org/cidoc-crm/P67_refers_to"/>
        <rdfs:domain rdf:resource="http://www.cidoc-crm.org/cidoc-crm/E1_CRM_Entity"/>
        <rdfs:range rdf:resource="http://www.cidoc-crm.org/cidoc-crm/E89_Propositional_Object"/>
        <rdfs:isDefinedBy rdf:resource="http://www.cidoc-crm.org/cidoc-crm/"/>
        <rdfs:label xml:lang="fr">fait l&apos;objet d&apos;un renvoi par</rdfs:label>
        <rdfs:label xml:lang="en">is referred to by</rdfs:label>
        <rdfs:label xml:lang="de">wird angeführt von</rdfs:label>
        <rdfs:label xml:lang="pt">é referenciado por</rdfs:label>
        <rdfs:label xml:lang="el">αναφέρεται από</rdfs:label>
        <rdfs:label xml:lang="ru">имеет ссылку на себя от</rdfs:label>
        <rdfs:label xml:lang="zh">被涉及</rdfs:label>
    </owl:ObjectProperty>
    


    <!-- http://www.cidoc-crm.org/cidoc-crm/P70_documents -->


    <owl:ObjectProperty rdf:about="http://www.cidoc-crm.org/cidoc-crm/P70_documents">
        <rdfs:subPropertyOf rdf:resource="http://www.cidoc-crm.org/cidoc-crm/P67_refers_to"/>
        <rdfs:domain rdf:resource="http://www.cidoc-crm.org/cidoc-crm/E31_Document"/>
        <rdfs:range rdf:resource="http://www.cidoc-crm.org/cidoc-crm/E1_CRM_Entity"/>
        <rdfs:comment xml:lang="en">This property refers to the fact that a document describes some entity.</rdfs:comment>
        <rdfs:isDefinedBy rdf:resource="http://www.cidoc-crm.org/cidoc-crm/"/>
        <rdfs:label xml:lang="de">belegt</rdfs:label>
        <rdfs:label xml:lang="pt">documenta</rdfs:label>
        <rdfs:label xml:lang="fr">documente</rdfs:label>
        <rdfs:label xml:lang="en">documents</rdfs:label>
        <rdfs:label xml:lang="el">τεκμηριώνει</rdfs:label>
        <rdfs:label xml:lang="ru">документирует</rdfs:label>
        <rdfs:label xml:lang="zh">记录了</rdfs:label>
    </owl:ObjectProperty>
    


    <!-- http://www.cidoc-crm.org/cidoc-crm/P70i_is_documented_in -->


    <owl:ObjectProperty rdf:about="http://www.cidoc-crm.org/cidoc-crm/P70i_is_documented_in">
        <rdfs:subPropertyOf rdf:resource="http://www.cidoc-crm.org/cidoc-crm/P67i_is_referred_to_by"/>
        <owl:inverseOf rdf:resource="http://www.cidoc-crm.org/cidoc-crm/P70_documents"/>
        <rdfs:domain rdf:resource="http://www.cidoc-crm.org/cidoc-crm/E1_CRM_Entity"/>
        <rdfs:range rdf:resource="http://www.cidoc-crm.org/cidoc-crm/E31_Document"/>
        <rdfs:isDefinedBy rdf:resource="http://www.cidoc-crm.org/cidoc-crm/"/>
        <rdfs:label xml:lang="fr">est documenté dans</rdfs:label>
        <rdfs:label xml:lang="en">is documented in</rdfs:label>
        <rdfs:label xml:lang="de">wird belegt in</rdfs:label>
        <rdfs:label xml:lang="pt">é documentado em</rdfs:label>
        <rdfs:label xml:lang="el">τεκμηριώνεται σε</rdfs:label>
        <rdfs:label xml:lang="ru">документирован в</rdfs:label>
        <rdfs:label xml:lang="zh">记录在</rdfs:label>
    </owl:ObjectProperty>
    


    <!-- http://www.cidoc-crm.org/cidoc-crm/P74_has_current_or_former_residence -->


    <owl:ObjectProperty rdf:about="http://www.cidoc-crm.org/cidoc-crm/P74_has_current_or_former_residence">
        <owl:inverseOf rdf:resource="http://www.cidoc-crm.org/cidoc-crm/P74i_is_current_or_former_residence_of"/>
        <rdfs:domain rdf:resource="http://www.cidoc-crm.org/cidoc-crm/E39_Actor"/>
        <rdfs:range rdf:resource="http://www.cidoc-crm.org/cidoc-crm/E53_Place"/>
        <rdfs:comment xml:lang="en">This property describes the current or former place of residence of an actor.</rdfs:comment>
        <rdfs:isDefinedBy rdf:resource="http://www.cidoc-crm.org/cidoc-crm/"/>
        <rdfs:label xml:lang="fr">a pour résidence actuelle ou antérieure</rdfs:label>
        <rdfs:label xml:lang="en">has current or former residence</rdfs:label>
        <rdfs:label xml:lang="de">hat derzeitigen oder früheren Sitz</rdfs:label>
        <rdfs:label xml:lang="pt">reside ou residiu em</rdfs:label>
        <rdfs:label xml:lang="el">έχει ή είχε κατοικία</rdfs:label>
        <rdfs:label xml:lang="ru">имеет текущее или бывшее местожительства</rdfs:label>
        <rdfs:label xml:lang="zh">有当前或曾经居住地</rdfs:label>
    </owl:ObjectProperty>
    


    <!-- http://www.cidoc-crm.org/cidoc-crm/P74i_is_current_or_former_residence_of -->


    <owl:ObjectProperty rdf:about="http://www.cidoc-crm.org/cidoc-crm/P74i_is_current_or_former_residence_of">
        <rdfs:domain rdf:resource="http://www.cidoc-crm.org/cidoc-crm/E53_Place"/>
        <rdfs:range rdf:resource="http://www.cidoc-crm.org/cidoc-crm/E39_Actor"/>
        <rdfs:isDefinedBy rdf:resource="http://www.cidoc-crm.org/cidoc-crm/"/>
        <rdfs:label xml:lang="fr">est la résidence actuelle ou antérieure de</rdfs:label>
        <rdfs:label xml:lang="en">is current or former residence of</rdfs:label>
        <rdfs:label xml:lang="de">ist derzeitiger oder früherer Sitz von</rdfs:label>
        <rdfs:label xml:lang="pt">é ou foi residência de</rdfs:label>
        <rdfs:label xml:lang="el">είναι ή ήταν κατοικία του/της</rdfs:label>
        <rdfs:label xml:lang="ru">является текущим или бывшим местом жительства для</rdfs:label>
        <rdfs:label xml:lang="zh">是当前或曾经居住地</rdfs:label>
    </owl:ObjectProperty>
    


    <!-- http://www.cidoc-crm.org/cidoc-crm/P94_has_created -->


    <owl:ObjectProperty rdf:about="http://www.cidoc-crm.org/cidoc-crm/P94_has_created"/>
    


    <!-- http://www.cidoc-crm.org/cidoc-crm/P94i_was_created_by -->


    <owl:ObjectProperty rdf:about="http://www.cidoc-crm.org/cidoc-crm/P94i_was_created_by"/>
    


    <!-- http://www.cidoc-crm.org/cidoc-crm/P9_consists_of -->


    <owl:ObjectProperty rdf:about="http://www.cidoc-crm.org/cidoc-crm/P9_consists_of">
        <rdfs:subPropertyOf rdf:resource="http://www.cidoc-crm.org/cidoc-crm/P10i_contains"/>
        <owl:inverseOf rdf:resource="http://www.cidoc-crm.org/cidoc-crm/P9i_forms_part_of"/>
        <rdfs:domain rdf:resource="http://www.cidoc-crm.org/cidoc-crm/E4_Period"/>
        <rdfs:range rdf:resource="http://www.cidoc-crm.org/cidoc-crm/E4_Period"/>
        <rdfs:comment xml:lang="en">This property associates a period of time with another period of time it contains.</rdfs:comment>
        <rdfs:isDefinedBy rdf:resource="http://www.cidoc-crm.org/cidoc-crm/"/>
        <rdfs:label xml:lang="fr">comprend</rdfs:label>
        <rdfs:label xml:lang="pt">consiste de</rdfs:label>
        <rdfs:label xml:lang="en">consists of</rdfs:label>
        <rdfs:label xml:lang="de">setzt sich zusammen aus</rdfs:label>
        <rdfs:label xml:lang="el">αποτελείται από</rdfs:label>
        <rdfs:label xml:lang="ru">состоит из</rdfs:label>
        <rdfs:label xml:lang="zh">包括</rdfs:label>
    </owl:ObjectProperty>
    


    <!-- http://www.cidoc-crm.org/cidoc-crm/P9i_forms_part_of -->


    <owl:ObjectProperty rdf:about="http://www.cidoc-crm.org/cidoc-crm/P9i_forms_part_of">
        <rdfs:subPropertyOf rdf:resource="http://www.cidoc-crm.org/cidoc-crm/P10_falls_within"/>
        <rdfs:domain rdf:resource="http://www.cidoc-crm.org/cidoc-crm/E4_Period"/>
        <rdfs:range rdf:resource="http://www.cidoc-crm.org/cidoc-crm/E4_Period"/>
        <rdfs:isDefinedBy rdf:resource="http://www.cidoc-crm.org/cidoc-crm/"/>
        <rdfs:label xml:lang="de">bildet Teil von</rdfs:label>
        <rdfs:label xml:lang="fr">fait partie de</rdfs:label>
        <rdfs:label xml:lang="pt">faz parte de</rdfs:label>
        <rdfs:label xml:lang="en">forms part of</rdfs:label>
        <rdfs:label xml:lang="el">αποτελεί μέρος του/της</rdfs:label>
        <rdfs:label xml:lang="ru">формирует часть</rdfs:label>
        <rdfs:label xml:lang="zh">组成部分</rdfs:label>
    </owl:ObjectProperty>
    


    <!-- http://www.ics.forth.gr/isl/CRMdig/L10_had_input -->


    <owl:ObjectProperty rdf:about="http://www.ics.forth.gr/isl/CRMdig/L10_had_input">
        <rdfs:subPropertyOf rdf:resource="http://www.cidoc-crm.org/cidoc-crm/P16_used_specific_object"/>
        <owl:inverseOf rdf:resource="http://www.ics.forth.gr/isl/CRMdig/L10i_was_input_of"/>
        <rdfs:domain rdf:resource="http://www.ics.forth.gr/isl/CRMdig/D7_Digital_Machine_Event"/>
        <rdfs:range rdf:resource="http://www.ics.forth.gr/isl/CRMdig/D1_Digital_Object"/>
        <rdfs:comment xml:lang="en">This property associates an activity in a digitization workflow with a digital object used as input for that activity.</rdfs:comment>
        <rdfs:isDefinedBy rdf:resource="http://www.ics.forth.gr/isl/CRMdig/"/>
        <rdfs:label xml:lang="en">has input</rdfs:label>
    </owl:ObjectProperty>
    


    <!-- http://www.ics.forth.gr/isl/CRMdig/L10i_was_input_of -->


    <owl:ObjectProperty rdf:about="http://www.ics.forth.gr/isl/CRMdig/L10i_was_input_of">
        <rdfs:subPropertyOf rdf:resource="http://www.cidoc-crm.org/cidoc-crm/P16i_was_used_for"/>
        <rdfs:domain rdf:resource="http://www.ics.forth.gr/isl/CRMdig/D1_Digital_Object"/>
        <rdfs:range rdf:resource="http://www.ics.forth.gr/isl/CRMdig/D7_Digital_Machine_Event"/>
        <rdfs:isDefinedBy rdf:resource="http://www.ics.forth.gr/isl/CRMdig/"/>
        <rdfs:label xml:lang="en">was input of</rdfs:label>
    </owl:ObjectProperty>
    


    <!-- http://www.ics.forth.gr/isl/CRMdig/L11_had_output -->


    <owl:ObjectProperty rdf:about="http://www.ics.forth.gr/isl/CRMdig/L11_had_output">
        <rdfs:subPropertyOf rdf:resource="http://www.cidoc-crm.org/cidoc-crm/P94_has_created"/>
        <rdfs:domain rdf:resource="http://www.ics.forth.gr/isl/CRMdig/D7_Digital_Machine_Event"/>
        <rdfs:range rdf:resource="http://www.ics.forth.gr/isl/CRMdig/D1_Digital_Object"/>
        <rdfs:comment xml:lang="en">This property associates an activity in a digitization workflow with a digital object produced as a result of that activity.</rdfs:comment>
        <rdfs:isDefinedBy rdf:resource="http://www.ics.forth.gr/isl/CRMdig/"/>
        <rdfs:label xml:lang="en">has output</rdfs:label>
    </owl:ObjectProperty>
    


    <!-- http://www.ics.forth.gr/isl/CRMdig/L11i_was_output_of -->


    <owl:ObjectProperty rdf:about="http://www.ics.forth.gr/isl/CRMdig/L11i_was_output_of">
        <rdfs:subPropertyOf rdf:resource="http://www.cidoc-crm.org/cidoc-crm/P94i_was_created_by"/>
        <owl:inverseOf rdf:resource="http://www.ics.forth.gr/isl/CRMdig/L11_had_output"/>
        <rdfs:domain rdf:resource="http://www.ics.forth.gr/isl/CRMdig/D1_Digital_Object"/>
        <rdfs:range rdf:resource="http://www.ics.forth.gr/isl/CRMdig/D7_Digital_Machine_Event"/>
        <rdfs:isDefinedBy rdf:resource="http://www.ics.forth.gr/isl/CRMdig/"/>
        <rdfs:label xml:lang="en">was output of</rdfs:label>
    </owl:ObjectProperty>
    


    <!-- http://www.ics.forth.gr/isl/CRMdig/L1_digitized -->


    <owl:ObjectProperty rdf:about="http://www.ics.forth.gr/isl/CRMdig/L1_digitized">
        <rdfs:subPropertyOf rdf:resource="http://www.cidoc-crm.org/cidoc-crm/P39_measured"/>
        <rdfs:domain rdf:resource="http://www.ics.forth.gr/isl/CRMdig/D2_Digitization_Process"/>
        <rdfs:range rdf:resource="http://www.cidoc-crm.org/cidoc-crm/E18_Physical_Thing"/>
        <rdfs:comment xml:lang="en">This property associates a digitization process with the cultural heritage object that is being digitized.</rdfs:comment>
        <rdfs:isDefinedBy rdf:resource="http://www.ics.forth.gr/isl/CRMdig/"/>
        <rdfs:label xml:lang="en">digitized</rdfs:label>
    </owl:ObjectProperty>
    


    <!-- http://www.ics.forth.gr/isl/CRMdig/L1i_was_digitized_by -->


    <owl:ObjectProperty rdf:about="http://www.ics.forth.gr/isl/CRMdig/L1i_was_digitized_by">
        <rdfs:subPropertyOf rdf:resource="http://www.cidoc-crm.org/cidoc-crm/P39i_was_measured_by"/>
        <owl:inverseOf rdf:resource="http://www.ics.forth.gr/isl/CRMdig/L1_digitized"/>
        <rdfs:domain rdf:resource="http://www.cidoc-crm.org/cidoc-crm/E18_Physical_Thing"/>
        <rdfs:range rdf:resource="http://www.ics.forth.gr/isl/CRMdig/D2_Digitization_Process"/>
        <rdfs:isDefinedBy rdf:resource="http://www.ics.forth.gr/isl/CRMdig/"/>
        <rdfs:label xml:lang="en">was digitized by</rdfs:label>
    </owl:ObjectProperty>
    


    <!-- http://www.ics.forth.gr/isl/CRMdig/L23_used_software_or_firmware -->


    <owl:ObjectProperty rdf:about="http://www.ics.forth.gr/isl/CRMdig/L23_used_software_or_firmware">
        <rdfs:subPropertyOf rdf:resource="http://www.cidoc-crm.org/cidoc-crm/P16_used_specific_object"/>
        <rdfs:domain rdf:resource="http://www.ics.forth.gr/isl/CRMdig/D7_Digital_Machine_Event"/>
        <rdfs:range rdf:resource="http://www.ics.forth.gr/isl/CRMdig/D14_Software"/>
        <rdfs:comment xml:lang="en">This property associates a digitization activity with the software that was used during that activity.</rdfs:comment>
        <rdfs:isDefinedBy rdf:resource="http://www.ics.forth.gr/isl/CRMdig/"/>
        <rdfs:label xml:lang="en">used software or firmware</rdfs:label>
    </owl:ObjectProperty>
    


    <!-- 
    ///////////////////////////////////////////////////////////////////////////////////////
    //
    // Data properties
    //
    ///////////////////////////////////////////////////////////////////////////////////////
     -->


    


    <!-- http://www.cidoc-crm.org/cidoc-crm/P190_has_symbolic_content -->


    <owl:DatatypeProperty rdf:about="http://www.cidoc-crm.org/cidoc-crm/P190_has_symbolic_content">
        <rdfs:subPropertyOf rdf:resource="http://www.cidoc-crm.org/cidoc-crm/P3_has_note"/>
        <rdfs:domain rdf:resource="http://www.cidoc-crm.org/cidoc-crm/E90_Symbolic_Object"/>
        <rdfs:range rdf:resource="http://www.w3.org/2000/01/rdf-schema#Literal"/>
        <rdfs:comment xml:lang="en">This property associates a symbolic object with a textual representation of its content.</rdfs:comment>
        <rdfs:isDefinedBy rdf:resource="http://www.cidoc-crm.org/cidoc-crm/"/>
        <rdfs:label xml:lang="fr">a pour contenu symbolique</rdfs:label>
        <rdfs:label xml:lang="en">has symbolic content</rdfs:label>
    </owl:DatatypeProperty>
    


    <!-- http://www.cidoc-crm.org/cidoc-crm/P3_has_note -->


    <owl:DatatypeProperty rdf:about="http://www.cidoc-crm.org/cidoc-crm/P3_has_note">
        <rdfs:domain rdf:resource="http://www.cidoc-crm.org/cidoc-crm/E1_CRM_Entity"/>
        <rdfs:range rdf:resource="http://www.w3.org/2000/01/rdf-schema#Literal"/>
        <rdfs:comment xml:lang="en">This property contains the textual description of an entity.</rdfs:comment>
        <rdfs:isDefinedBy rdf:resource="http://www.cidoc-crm.org/cidoc-crm/"/>
        <rdfs:label xml:lang="fr">a pour note</rdfs:label>
        <rdfs:label xml:lang="en">has note</rdfs:label>
        <rdfs:label xml:lang="de">hat Anmerkung</rdfs:label>
        <rdfs:label xml:lang="pt">tem nota</rdfs:label>
        <rdfs:label xml:lang="el">έχει επεξήγηση</rdfs:label>
        <rdfs:label xml:lang="ru">имеет примечание</rdfs:label>
        <rdfs:label xml:lang="zh">有注释</rdfs:label>
    </owl:DatatypeProperty>
    


    <!-- http://www.cidoc-crm.org/cidoc-crm/P82_at_some_time_within -->


    <owl:DatatypeProperty rdf:about="http://www.cidoc-crm.org/cidoc-crm/P82_at_some_time_within">
        <rdfs:domain rdf:resource="http://www.cidoc-crm.org/cidoc-crm/E52_Time-Span"/>
        <rdfs:range rdf:resource="http://www.w3.org/2000/01/rdf-schema#Literal"/>
        <rdfs:comment xml:lang="en">This property describes the maximum period of time within which a time span falls.</rdfs:comment>
        <rdfs:isDefinedBy rdf:resource="http://www.cidoc-crm.org/cidoc-crm/"/>
        <rdfs:label xml:lang="fr">a eu lieu durant</rdfs:label>
        <rdfs:label xml:lang="pt">abrange no máximo</rdfs:label>
        <rdfs:label xml:lang="en">at some time within</rdfs:label>
        <rdfs:label xml:lang="de">irgendwann innerhalb von</rdfs:label>
        <rdfs:label xml:lang="el">κάποτε εντός</rdfs:label>
        <rdfs:label xml:lang="ru">некоторое время в течение</rdfs:label>
        <rdfs:label xml:lang="zh">最长范围是</rdfs:label>
    </owl:DatatypeProperty>
    


    <!-- http://www.cidoc-crm.org/cidoc-crm/P82a_begin_of_the_begin -->


    <owl:DatatypeProperty rdf:about="http://www.cidoc-crm.org/cidoc-crm/P82a_begin_of_the_begin">
        <rdfs:subPropertyOf rdf:resource="http://www.cidoc-crm.org/cidoc-crm/P82_at_some_time_within"/>
        <rdfs:domain rdf:resource="http://www.cidoc-crm.org/cidoc-crm/E52_Time-Span"/>
        <rdfs:range rdf:resource="http://www.w3.org/2001/XMLSchema#dateTime"/>
        <rdfs:comment xml:lang="en">This property describes the precise beginning date and time of a time span.</rdfs:comment>
        <rdfs:isDefinedBy rdf:resource="http://www.cidoc-crm.org/cidoc-crm/"/>
        <rdfs:label xml:lang="de">Anfang des Anfangs</rdfs:label>
        <rdfs:label xml:lang="en">begin of the begin</rdfs:label>
        <rdfs:label xml:lang="pt">começar do início</rdfs:label>
        <rdfs:label xml:lang="fr">début du début</rdfs:label>
        <rdfs:label xml:lang="el">αρχή της αρχής</rdfs:label>
        <rdfs:label xml:lang="ru">начать с начала</rdfs:label>
    </owl:DatatypeProperty>
    


    <!-- http://www.cidoc-crm.org/cidoc-crm/P82b_end_of_the_end -->


    <owl:DatatypeProperty rdf:about="http://www.cidoc-crm.org/cidoc-crm/P82b_end_of_the_end">
        <rdfs:subPropertyOf rdf:resource="http://www.cidoc-crm.org/cidoc-crm/P82_at_some_time_within"/>
        <rdfs:domain rdf:resource="http://www.cidoc-crm.org/cidoc-crm/E52_Time-Span"/>
        <rdfs:range rdf:resource="http://www.w3.org/2001/XMLSchema#dateTime"/>
        <rdfs:comment xml:lang="en">This property describes the precise ending date and time of a time span.</rdfs:comment>
        <rdfs:isDefinedBy rdf:resource="http://www.cidoc-crm.org/cidoc-crm/"/>
        <rdfs:label xml:lang="de">Ende vom Ende</rdfs:label>
        <rdfs:label xml:lang="en">end of the end</rdfs:label>
        <rdfs:label xml:lang="pt">fim do fim</rdfs:label>
        <rdfs:label xml:lang="fr">fin de la fin</rdfs:label>
        <rdfs:label xml:lang="el">τέλος του τέλους</rdfs:label>
        <rdfs:label xml:lang="ru">конец конец</rdfs:label>
    </owl:DatatypeProperty>
    


    <!-- 
    ///////////////////////////////////////////////////////////////////////////////////////
    //
    // Classes
    //
    ///////////////////////////////////////////////////////////////////////////////////////
     -->


    


    <!-- http://iflastandards.info/ns/fr/frbr/frbroo/F15_Complex_Work -->


    <owl:Class rdf:about="http://iflastandards.info/ns/fr/frbr/frbroo/F15_Complex_Work">
        <rdfs:subClassOf rdf:resource="http://iflastandards.info/ns/fr/frbr/frbroo/F1_Work"/>
        <rdfs:comment xml:lang="en">A work that is composed of other works.</rdfs:comment>
        <rdfs:isDefinedBy rdf:resource="http://iflastandards.info/ns/fr/frbr/frbroo/"/>
        <rdfs:label xml:lang="en">Complex Work</rdfs:label>
    </owl:Class>
    


    <!-- http://iflastandards.info/ns/fr/frbr/frbroo/F1_Work -->


    <owl:Class rdf:about="http://iflastandards.info/ns/fr/frbr/frbroo/F1_Work">
        <rdfs:subClassOf rdf:resource="http://www.cidoc-crm.org/cidoc-crm/E89_Propositional_Object"/>
        <rdfs:comment xml:lang="en">The essence or conceptualization of a cultural heritage object.</rdfs:comment>
        <rdfs:isDefinedBy rdf:resource="http://iflastandards.info/ns/fr/frbr/frbroo/"/>
        <rdfs:label xml:lang="en">Work</rdfs:label>
    </owl:Class>
    


    <!-- http://iflastandards.info/ns/fr/frbr/frbroo/F27_Work_Conception -->


    <owl:Class rdf:about="http://iflastandards.info/ns/fr/frbr/frbroo/F27_Work_Conception">
        <rdfs:subClassOf rdf:resource="http://www.cidoc-crm.org/cidoc-crm/E65_Creation"/>
        <rdfs:comment xml:lang="en">An activity that represents the creation of a work.</rdfs:comment>
        <rdfs:isDefinedBy rdf:resource="http://iflastandards.info/ns/fr/frbr/frbroo/"/>
        <rdfs:label xml:lang="en">Work Conception</rdfs:label>
    </owl:Class>
    


    <!-- http://iflastandards.info/ns/fr/frbr/frbroo/F28_Expression_Creation -->


    <owl:Class rdf:about="http://iflastandards.info/ns/fr/frbr/frbroo/F28_Expression_Creation">
        <rdfs:subClassOf rdf:resource="http://www.cidoc-crm.org/cidoc-crm/E12_Production"/>
        <rdfs:subClassOf rdf:resource="http://www.cidoc-crm.org/cidoc-crm/E65_Creation"/>
        <rdfs:comment xml:lang="en">An activity that represents the creation of an expression.</rdfs:comment>
        <rdfs:isDefinedBy rdf:resource="http://iflastandards.info/ns/fr/frbr/frbroo/"/>
        <rdfs:label xml:lang="en">Expression Creation</rdfs:label>
    </owl:Class>
    


    <!-- http://iflastandards.info/ns/fr/frbr/frbroo/F2_Expression -->


    <owl:Class rdf:about="http://iflastandards.info/ns/fr/frbr/frbroo/F2_Expression">
        <rdfs:subClassOf rdf:resource="http://www.cidoc-crm.org/cidoc-crm/E73_Information_Object"/>
        <rdfs:comment xml:lang="en">The realisation of a work, referring to the intellectual content of a cultural heritage object.</rdfs:comment>
        <rdfs:isDefinedBy rdf:resource="http://iflastandards.info/ns/fr/frbr/frbroo/"/>
        <rdfs:label xml:lang="en">Expression</rdfs:label>
    </owl:Class>
    


    <!-- http://iflastandards.info/ns/fr/frbr/frbroo/F4_Manifestation_Singleton -->


    <owl:Class rdf:about="http://iflastandards.info/ns/fr/frbr/frbroo/F4_Manifestation_Singleton">
        <rdfs:subClassOf rdf:resource="http://www.cidoc-crm.org/cidoc-crm/E24_Physical_Man-Made_Thing"/>
        <rdfs:comment xml:lang="en">The physical instance of a cultural heritage object.</rdfs:comment>
        <rdfs:isDefinedBy rdf:resource="http://iflastandards.info/ns/fr/frbr/frbroo/"/>
        <rdfs:label xml:lang="en">Manifestation Singleton</rdfs:label>
    </owl:Class>
    


    <!-- http://vocab.getty.edu/aat/Concept -->


    <owl:Class rdf:about="http://vocab.getty.edu/aat/Concept"/>
    


    <!-- http://www.cidoc-crm.org/cidoc-crm/E12_Production -->


    <owl:Class rdf:about="http://www.cidoc-crm.org/cidoc-crm/E12_Production"/>
    


    <!-- http://www.cidoc-crm.org/cidoc-crm/E18_Physical_Thing -->


    <owl:Class rdf:about="http://www.cidoc-crm.org/cidoc-crm/E18_Physical_Thing"/>
    


    <!-- http://www.cidoc-crm.org/cidoc-crm/E1_CRM_Entity -->


    <owl:Class rdf:about="http://www.cidoc-crm.org/cidoc-crm/E1_CRM_Entity"/>
    


    <!-- http://www.cidoc-crm.org/cidoc-crm/E20_Biological_Object -->


    <owl:Class rdf:about="http://www.cidoc-crm.org/cidoc-crm/E20_Biological_Object"/>
    


    <!-- http://www.cidoc-crm.org/cidoc-crm/E21_Person -->


    <owl:Class rdf:about="http://www.cidoc-crm.org/cidoc-crm/E21_Person">
        <rdfs:subClassOf rdf:resource="http://www.cidoc-crm.org/cidoc-crm/E20_Biological_Object"/>
        <rdfs:subClassOf rdf:resource="http://www.cidoc-crm.org/cidoc-crm/E39_Actor"/>
        <rdfs:comment xml:lang="en">An individual person.</rdfs:comment>
        <rdfs:isDefinedBy rdf:resource="http://www.cidoc-crm.org/cidoc-crm/"/>
        <rdfs:label xml:lang="de">Person</rdfs:label>
        <rdfs:label xml:lang="en">Person</rdfs:label>
        <rdfs:label xml:lang="fr">Personne</rdfs:label>
        <rdfs:label xml:lang="pt">Pessoa</rdfs:label>
        <rdfs:label xml:lang="el">Πρόσωπο</rdfs:label>
        <rdfs:label xml:lang="ru">Личность</rdfs:label>
        <rdfs:label xml:lang="zh">人物</rdfs:label>
    </owl:Class>
    


    <!-- http://www.cidoc-crm.org/cidoc-crm/E22_Man-Made_Object -->


    <owl:Class rdf:about="http://www.cidoc-crm.org/cidoc-crm/E22_Man-Made_Object"/>
    


    <!-- http://www.cidoc-crm.org/cidoc-crm/E24_Physical_Human-Made_Thing -->


    <owl:Class rdf:about="http://www.cidoc-crm.org/cidoc-crm/E24_Physical_Human-Made_Thing">
        <rdfs:subClassOf rdf:resource="http://www.cidoc-crm.org/cidoc-crm/E18_Physical_Thing"/>
        <rdfs:subClassOf rdf:resource="http://www.cidoc-crm.org/cidoc-crm/E71_Human-Made_Thing"/>
        <rdfs:comment xml:lang="en">A persistent physical item of any size that is purposely created by human activity.</rdfs:comment>
        <rdfs:isDefinedBy rdf:resource="http://www.cidoc-crm.org/cidoc-crm/"/>
        <rdfs:label xml:lang="fr">Chose matérielle élaborée par l’humain</rdfs:label>
        <rdfs:label xml:lang="en">Physical Human-Made Thing</rdfs:label>
    </owl:Class>
    


    <!-- http://www.cidoc-crm.org/cidoc-crm/E24_Physical_Man-Made_Thing -->


    <owl:Class rdf:about="http://www.cidoc-crm.org/cidoc-crm/E24_Physical_Man-Made_Thing"/>
    


    <!-- http://www.cidoc-crm.org/cidoc-crm/E28_Conceptual_Object -->


    <owl:Class rdf:about="http://www.cidoc-crm.org/cidoc-crm/E28_Conceptual_Object"/>
    


    <!-- http://www.cidoc-crm.org/cidoc-crm/E2_Temporal_Entity -->


    <owl:Class rdf:about="http://www.cidoc-crm.org/cidoc-crm/E2_Temporal_Entity"/>
    


    <!-- http://www.cidoc-crm.org/cidoc-crm/E31_Document -->


    <owl:Class rdf:about="http://www.cidoc-crm.org/cidoc-crm/E31_Document">
        <rdfs:subClassOf rdf:resource="http://www.cidoc-crm.org/cidoc-crm/E73_Information_Object"/>
        <rdfs:comment xml:lang="en">An information object that makes propositions about reality.</rdfs:comment>
        <rdfs:isDefinedBy rdf:resource="http://www.cidoc-crm.org/cidoc-crm/"/>
        <rdfs:label xml:lang="en">Document</rdfs:label>
        <rdfs:label xml:lang="fr">Document</rdfs:label>
        <rdfs:label xml:lang="pt">Documento</rdfs:label>
        <rdfs:label xml:lang="de">Dokument</rdfs:label>
        <rdfs:label xml:lang="el">Τεκμήριο</rdfs:label>
        <rdfs:label xml:lang="ru">Документ</rdfs:label>
        <rdfs:label xml:lang="zh">文献</rdfs:label>
    </owl:Class>
    


    <!-- http://www.cidoc-crm.org/cidoc-crm/E33_Linguistic_Object -->


    <owl:Class rdf:about="http://www.cidoc-crm.org/cidoc-crm/E33_Linguistic_Object"/>
    


    <!-- http://www.cidoc-crm.org/cidoc-crm/E35_Title -->


    <owl:Class rdf:about="http://www.cidoc-crm.org/cidoc-crm/E35_Title">
        <rdfs:subClassOf rdf:resource="http://www.cidoc-crm.org/cidoc-crm/E33_Linguistic_Object"/>
        <rdfs:subClassOf rdf:resource="http://www.cidoc-crm.org/cidoc-crm/E41_Appellation"/>
        <rdfs:comment xml:lang="en">A textual string that functions as a title for a work.</rdfs:comment>
        <rdfs:isDefinedBy rdf:resource="http://www.cidoc-crm.org/cidoc-crm/"/>
        <rdfs:label xml:lang="de">Titel</rdfs:label>
        <rdfs:label xml:lang="en">Title</rdfs:label>
        <rdfs:label xml:lang="fr">Titre</rdfs:label>
        <rdfs:label xml:lang="pt">Título</rdfs:label>
        <rdfs:label xml:lang="el">Τίτλος</rdfs:label>
        <rdfs:label xml:lang="ru">Заголовок</rdfs:label>
        <rdfs:label xml:lang="zh">题名</rdfs:label>
    </owl:Class>
    


    <!-- http://www.cidoc-crm.org/cidoc-crm/E39_Actor -->


    <owl:Class rdf:about="http://www.cidoc-crm.org/cidoc-crm/E39_Actor">
        <rdfs:subClassOf rdf:resource="http://www.cidoc-crm.org/cidoc-crm/E77_Persistent_Item"/>
        <rdfs:comment xml:lang="en">An individual person or a group of people, with the potential to perform intentional and accountable actions.</rdfs:comment>
        <rdfs:isDefinedBy rdf:resource="http://www.cidoc-crm.org/cidoc-crm/"/>
        <rdfs:label xml:lang="fr">Actant</rdfs:label>
        <rdfs:label xml:lang="en">Actor</rdfs:label>
        <rdfs:label xml:lang="pt">Agente</rdfs:label>
        <rdfs:label xml:lang="de">Akteur</rdfs:label>
        <rdfs:label xml:lang="el">Δράστης</rdfs:label>
        <rdfs:label xml:lang="ru">Агент</rdfs:label>
        <rdfs:label xml:lang="zh">参与者</rdfs:label>
    </owl:Class>
    


    <!-- http://www.cidoc-crm.org/cidoc-crm/E41_Appellation -->


    <owl:Class rdf:about="http://www.cidoc-crm.org/cidoc-crm/E41_Appellation"/>
    


    <!-- http://www.cidoc-crm.org/cidoc-crm/E42_Identifier -->


    <owl:Class rdf:about="http://www.cidoc-crm.org/cidoc-crm/E42_Identifier">
        <rdfs:subClassOf rdf:resource="http://www.cidoc-crm.org/cidoc-crm/E41_Appellation"/>
        <rdfs:comment xml:lang="en">A textual string assigned to a cultural heritage object in order to identify it uniquely within a given context.</rdfs:comment>
        <rdfs:isDefinedBy rdf:resource="http://www.cidoc-crm.org/cidoc-crm/"/>
        <rdfs:label xml:lang="fr">Identifiant</rdfs:label>
        <rdfs:label xml:lang="pt">Identificador de Objeto</rdfs:label>
        <rdfs:label xml:lang="en">Identifier</rdfs:label>
        <rdfs:label xml:lang="de">Kennung</rdfs:label>
        <rdfs:label xml:lang="el">Κωδικός Αναγνώρισης</rdfs:label>
        <rdfs:label xml:lang="ru">Идентификатор Объекта</rdfs:label>
        <rdfs:label xml:lang="zh">标识符</rdfs:label>
    </owl:Class>
    


    <!-- http://www.cidoc-crm.org/cidoc-crm/E4_Period -->


    <owl:Class rdf:about="http://www.cidoc-crm.org/cidoc-crm/E4_Period"/>
    


    <!-- http://www.cidoc-crm.org/cidoc-crm/E52_Time-Span -->


    <owl:Class rdf:about="http://www.cidoc-crm.org/cidoc-crm/E52_Time-Span">
        <rdfs:subClassOf rdf:resource="http://www.cidoc-crm.org/cidoc-crm/E1_CRM_Entity"/>
        <rdfs:comment xml:lang="en">An abstract temporal extent having a beginning, an end and a duration.</rdfs:comment>
        <rdfs:isDefinedBy rdf:resource="http://www.cidoc-crm.org/cidoc-crm/"/>
        <rdfs:label xml:lang="fr">Intervalle temporel</rdfs:label>
        <rdfs:label xml:lang="pt">Período de Tempo</rdfs:label>
        <rdfs:label xml:lang="en">Time-Span</rdfs:label>
        <rdfs:label xml:lang="de">Zeitspanne</rdfs:label>
        <rdfs:label xml:lang="el">Χρονικό Διάστημα</rdfs:label>
        <rdfs:label xml:lang="ru">Интервал Времени</rdfs:label>
        <rdfs:label xml:lang="zh">时段</rdfs:label>
    </owl:Class>
    


    <!-- http://www.cidoc-crm.org/cidoc-crm/E53_Place -->


    <owl:Class rdf:about="http://www.cidoc-crm.org/cidoc-crm/E53_Place">
        <rdfs:subClassOf rdf:resource="http://www.cidoc-crm.org/cidoc-crm/E1_CRM_Entity"/>
        <rdfs:comment xml:lang="en">A geographical location.</rdfs:comment>
        <rdfs:isDefinedBy rdf:resource="http://www.cidoc-crm.org/cidoc-crm/"/>
        <rdfs:label xml:lang="fr">Lieu</rdfs:label>
        <rdfs:label xml:lang="pt">Local</rdfs:label>
        <rdfs:label xml:lang="de">Ort</rdfs:label>
        <rdfs:label xml:lang="en">Place</rdfs:label>
        <rdfs:label xml:lang="el">Τόπος</rdfs:label>
        <rdfs:label xml:lang="ru">Место</rdfs:label>
        <rdfs:label xml:lang="zh">地点</rdfs:label>
    </owl:Class>
    


    <!-- http://www.cidoc-crm.org/cidoc-crm/E54_Dimension -->


    <owl:Class rdf:about="http://www.cidoc-crm.org/cidoc-crm/E54_Dimension"/>
    


    <!-- http://www.cidoc-crm.org/cidoc-crm/E55_Type -->


    <owl:Class rdf:about="http://www.cidoc-crm.org/cidoc-crm/E55_Type">
        <rdfs:subClassOf rdf:resource="http://www.cidoc-crm.org/cidoc-crm/E28_Conceptual_Object"/>
        <rdfs:comment xml:lang="en">A categorical concept denoted by terms from thesauri and controlled vocabularies used to characterize and classify other entities.</rdfs:comment>
        <rdfs:isDefinedBy rdf:resource="http://www.cidoc-crm.org/cidoc-crm/"/>
        <rdfs:label xml:lang="pt">Tipo</rdfs:label>
        <rdfs:label xml:lang="en">Type</rdfs:label>
        <rdfs:label xml:lang="fr">Type</rdfs:label>
        <rdfs:label xml:lang="de">Typus</rdfs:label>
        <rdfs:label xml:lang="el">Τύπος</rdfs:label>
        <rdfs:label xml:lang="ru">Тип</rdfs:label>
        <rdfs:label xml:lang="zh">类型</rdfs:label>
    </owl:Class>
    


    <!-- http://www.cidoc-crm.org/cidoc-crm/E5_Event -->


    <owl:Class rdf:about="http://www.cidoc-crm.org/cidoc-crm/E5_Event"/>
    


    <!-- http://www.cidoc-crm.org/cidoc-crm/E65_Creation -->


    <owl:Class rdf:about="http://www.cidoc-crm.org/cidoc-crm/E65_Creation"/>
    


    <!-- http://www.cidoc-crm.org/cidoc-crm/E70_Thing -->


    <owl:Class rdf:about="http://www.cidoc-crm.org/cidoc-crm/E70_Thing"/>
    


    <!-- http://www.cidoc-crm.org/cidoc-crm/E71_Human-Made_Thing -->


    <owl:Class rdf:about="http://www.cidoc-crm.org/cidoc-crm/E71_Human-Made_Thing"/>
    


    <!-- http://www.cidoc-crm.org/cidoc-crm/E73_Information_Object -->


    <owl:Class rdf:about="http://www.cidoc-crm.org/cidoc-crm/E73_Information_Object">
        <rdfs:subClassOf rdf:resource="http://www.cidoc-crm.org/cidoc-crm/E89_Propositional_Object"/>
        <rdfs:subClassOf rdf:resource="http://www.cidoc-crm.org/cidoc-crm/E90_Symbolic_Object"/>
        <rdfs:comment xml:lang="en">An immaterial item that has an objectively recognizable structure and is documented as a single unit.</rdfs:comment>
        <rdfs:isDefinedBy rdf:resource="http://www.cidoc-crm.org/cidoc-crm/"/>
        <rdfs:label xml:lang="en">Information Object</rdfs:label>
        <rdfs:label xml:lang="de">Informationsgegenstand</rdfs:label>
        <rdfs:label xml:lang="fr">Objet informationnel</rdfs:label>
        <rdfs:label xml:lang="pt">Objeto de Informação</rdfs:label>
        <rdfs:label xml:lang="el">Πληροφοριακό Αντικείμενο</rdfs:label>
        <rdfs:label xml:lang="ru">Информационный Объект</rdfs:label>
        <rdfs:label xml:lang="zh">信息对象</rdfs:label>
    </owl:Class>
    


    <!-- http://www.cidoc-crm.org/cidoc-crm/E74_Group -->


    <owl:Class rdf:about="http://www.cidoc-crm.org/cidoc-crm/E74_Group">
        <rdfs:subClassOf rdf:resource="http://www.cidoc-crm.org/cidoc-crm/E39_Actor"/>
        <rdfs:comment xml:lang="en">A unified group of people.</rdfs:comment>
        <rdfs:isDefinedBy rdf:resource="http://www.cidoc-crm.org/cidoc-crm/"/>
        <rdfs:label xml:lang="en">Group</rdfs:label>
        <rdfs:label xml:lang="fr">Groupe</rdfs:label>
        <rdfs:label xml:lang="pt">Grupo</rdfs:label>
        <rdfs:label xml:lang="de">Menschliche Gruppe</rdfs:label>
        <rdfs:label xml:lang="el">Ομάδα</rdfs:label>
        <rdfs:label xml:lang="ru">Группа</rdfs:label>
        <rdfs:label xml:lang="zh">团体</rdfs:label>
    </owl:Class>
    


    <!-- http://www.cidoc-crm.org/cidoc-crm/E77_Persistent_Item -->


    <owl:Class rdf:about="http://www.cidoc-crm.org/cidoc-crm/E77_Persistent_Item"/>
    


    <!-- http://www.cidoc-crm.org/cidoc-crm/E78_Curated_Holding -->


    <owl:Class rdf:about="http://www.cidoc-crm.org/cidoc-crm/E78_Curated_Holding">
        <rdfs:subClassOf rdf:resource="http://www.cidoc-crm.org/cidoc-crm/E24_Physical_Human-Made_Thing"/>
        <rdfs:comment xml:lang="en">A collection of physical objects that is assembled and maintained by one or more actors over time for a specific purpose and audience.</rdfs:comment>
        <rdfs:isDefinedBy rdf:resource="http://www.cidoc-crm.org/cidoc-crm/"/>
        <rdfs:label xml:lang="fr">Collection</rdfs:label>
        <rdfs:label xml:lang="en">Curated Holding</rdfs:label>
    </owl:Class>
    


    <!-- http://www.cidoc-crm.org/cidoc-crm/E7_Activity -->


    <owl:Class rdf:about="http://www.cidoc-crm.org/cidoc-crm/E7_Activity">
        <rdfs:subClassOf rdf:resource="http://www.cidoc-crm.org/cidoc-crm/E5_Event"/>
        <rdfs:comment xml:lang="en">An action intentionally carried out by one or more actors.</rdfs:comment>
        <rdfs:isDefinedBy rdf:resource="http://www.cidoc-crm.org/cidoc-crm/"/>
        <rdfs:label xml:lang="en">Activity</rdfs:label>
        <rdfs:label xml:lang="fr">Activité</rdfs:label>
        <rdfs:label xml:lang="pt">Atividade</rdfs:label>
        <rdfs:label xml:lang="de">Handlung</rdfs:label>
        <rdfs:label xml:lang="el">Δράση</rdfs:label>
        <rdfs:label xml:lang="ru">Деятельность</rdfs:label>
        <rdfs:label xml:lang="zh">活动</rdfs:label>
    </owl:Class>
    


    <!-- http://www.cidoc-crm.org/cidoc-crm/E87_Curation_Activity -->


    <owl:Class rdf:about="http://www.cidoc-crm.org/cidoc-crm/E87_Curation_Activity">
        <rdfs:subClassOf rdf:resource="http://www.cidoc-crm.org/cidoc-crm/E7_Activity"/>
        <rdfs:comment xml:lang="en">An activity that results in the continuity of management and the preservation and evolution of a collection.</rdfs:comment>
        <rdfs:isDefinedBy rdf:resource="http://www.cidoc-crm.org/cidoc-crm/"/>
        <rdfs:label xml:lang="fr">Activité curatoriale</rdfs:label>
        <rdfs:label xml:lang="en">Curation Activity</rdfs:label>
        <rdfs:label xml:lang="de">Kuratorische Tätigkeit</rdfs:label>
        <rdfs:label xml:lang="zh">管理</rdfs:label>
    </owl:Class>
    


    <!-- http://www.cidoc-crm.org/cidoc-crm/E89_Propositional_Object -->


    <owl:Class rdf:about="http://www.cidoc-crm.org/cidoc-crm/E89_Propositional_Object"/>
    


    <!-- http://www.cidoc-crm.org/cidoc-crm/E90_Symbolic_Object -->


    <owl:Class rdf:about="http://www.cidoc-crm.org/cidoc-crm/E90_Symbolic_Object"/>
    


    <!-- http://www.ics.forth.gr/isl/CRMdig/D10_Software_Execution -->


    <owl:Class rdf:about="http://www.ics.forth.gr/isl/CRMdig/D10_Software_Execution">
        <rdfs:subClassOf rdf:resource="http://www.ics.forth.gr/isl/CRMdig/D7_Digital_Machine_Event"/>
        <rdfs:comment xml:lang="en">An activity in which a digital device runs a software program on a digital object.</rdfs:comment>
        <rdfs:isDefinedBy rdf:resource="http://www.ics.forth.gr/isl/CRMdig/"/>
        <rdfs:label xml:lang="en">Software Execution</rdfs:label>
    </owl:Class>
    


    <!-- http://www.ics.forth.gr/isl/CRMdig/D11_Digital_Measurement_Event -->


    <owl:Class rdf:about="http://www.ics.forth.gr/isl/CRMdig/D11_Digital_Measurement_Event"/>
    


    <!-- http://www.ics.forth.gr/isl/CRMdig/D14_Software -->


    <owl:Class rdf:about="http://www.ics.forth.gr/isl/CRMdig/D14_Software">
        <rdfs:subClassOf rdf:resource="http://www.ics.forth.gr/isl/CRMdig/D1_Digital_Object"/>
        <rdfs:comment xml:lang="en">A computer program.</rdfs:comment>
        <rdfs:isDefinedBy rdf:resource="http://www.ics.forth.gr/isl/CRMdig/"/>
        <rdfs:label xml:lang="en">Software</rdfs:label>
    </owl:Class>
    


    <!-- http://www.ics.forth.gr/isl/CRMdig/D1_Digital_Object -->


    <owl:Class rdf:about="http://www.ics.forth.gr/isl/CRMdig/D1_Digital_Object"/>
    


    <!-- http://www.ics.forth.gr/isl/CRMdig/D2_Digitization_Process -->


    <owl:Class rdf:about="http://www.ics.forth.gr/isl/CRMdig/D2_Digitization_Process">
        <rdfs:subClassOf rdf:resource="http://www.ics.forth.gr/isl/CRMdig/D11_Digital_Measurement_Event"/>
        <rdfs:comment xml:lang="en">An activity that results in the production of data objects functioning as digital representations of physical entities.</rdfs:comment>
        <rdfs:isDefinedBy rdf:resource="http://www.ics.forth.gr/isl/CRMdig/"/>
        <rdfs:label xml:lang="en">Digitization Process</rdfs:label>
    </owl:Class>
    


    <!-- http://www.ics.forth.gr/isl/CRMdig/D7_Digital_Machine_Event -->


    <owl:Class rdf:about="http://www.ics.forth.gr/isl/CRMdig/D7_Digital_Machine_Event"/>
    


    <!-- http://www.ics.forth.gr/isl/CRMdig/D8_Digital_Device -->


    <owl:Class rdf:about="http://www.ics.forth.gr/isl/CRMdig/D8_Digital_Device">
        <rdfs:subClassOf rdf:resource="http://www.cidoc-crm.org/cidoc-crm/E22_Man-Made_Object"/>
        <rdfs:comment xml:lang="en">A technical tool that is used to process or produce digital objects.</rdfs:comment>
        <rdfs:isDefinedBy rdf:resource="http://www.ics.forth.gr/isl/CRMdig/"/>
        <rdfs:label xml:lang="en">Digital Device</rdfs:label>
    </owl:Class>
    


    <!-- http://www.ics.forth.gr/isl/CRMdig/D9_Data_Object -->


    <owl:Class rdf:about="http://www.ics.forth.gr/isl/CRMdig/D9_Data_Object">
        <rdfs:subClassOf rdf:resource="http://www.cidoc-crm.org/cidoc-crm/E54_Dimension"/>
        <rdfs:subClassOf rdf:resource="http://www.ics.forth.gr/isl/CRMdig/D1_Digital_Object"/>
        <rdfs:comment xml:lang="en">A digital object that is the direct result of an activity in a digitization workflow.</rdfs:comment>
        <rdfs:isDefinedBy rdf:resource="http://www.ics.forth.gr/isl/CRMdig/"/>
        <rdfs:label xml:lang="en">Data Object</rdfs:label>
    </owl:Class>
    


    <!-- 
    ///////////////////////////////////////////////////////////////////////////////////////
    //
    // Individuals
    //
    ///////////////////////////////////////////////////////////////////////////////////////
     -->


    


    <!-- http://vocab.getty.edu/aat/300011172 -->


    <owl:NamedIndividual rdf:about="http://vocab.getty.edu/aat/300011172">
        <rdf:type rdf:resource="http://vocab.getty.edu/aat/Concept"/>
        <dc:identifier>300011172</dc:identifier>
        <rdfs:comment xml:lang="en">Works comprising precious or semiprecious stones or other materials such as amber or pearl, cut, polished, or otherwise dressed for ornamental purposes to be used in jewelry, seals, or amulets.</rdfs:comment>
        <rdfs:isDefinedBy rdf:resource="http://vocab.getty.edu/aat/"/>
        <rdfs:label xml:lang="en">gems (worked stones)</rdfs:label>
        <skos:inScheme rdf:resource="http://vocab.getty.edu/aat/"/>
    </owl:NamedIndividual>
    


    <!-- http://vocab.getty.edu/aat/300022488 -->


    <owl:NamedIndividual rdf:about="http://vocab.getty.edu/aat/300022488">
        <rdf:type rdf:resource="http://vocab.getty.edu/aat/Concept"/>
        <dc:identifier>300022488</dc:identifier>
        <rdfs:comment xml:lang="en">Instruments for drawing circles and measuring the distance between two points.</rdfs:comment>
        <rdfs:isDefinedBy rdf:resource="http://vocab.getty.edu/aat/"/>
        <rdfs:label xml:lang="en">compasses (drawing instruments)</rdfs:label>
        <skos:inScheme rdf:resource="http://vocab.getty.edu/aat/"/>
    </owl:NamedIndividual>
    


    <!-- http://vocab.getty.edu/aat/300024594 -->


    <owl:NamedIndividual rdf:about="http://vocab.getty.edu/aat/300024594">
        <rdf:type rdf:resource="http://vocab.getty.edu/aat/Concept"/>
        <dc:identifier>300024594</dc:identifier>
        <rdfs:comment xml:lang="en">Optical instruments consisting of a lens or combination of lenses that allow the viewing of objects that are too small to be seen with the naked, unaided eye.</rdfs:comment>
        <rdfs:isDefinedBy rdf:resource="http://vocab.getty.edu/aat/"/>
        <rdfs:label xml:lang="en">microscopes</rdfs:label>
        <skos:inScheme rdf:resource="http://vocab.getty.edu/aat/"/>
    </owl:NamedIndividual>
    


    <!-- http://vocab.getty.edu/aat/300024814 -->


    <owl:NamedIndividual rdf:about="http://vocab.getty.edu/aat/300024814">
        <rdf:type rdf:resource="http://vocab.getty.edu/aat/Concept"/>
        <dc:identifier>300024814</dc:identifier>
        <rdfs:comment xml:lang="en">Hollow forms in which castings or pressings are made; used with many materials, including clay, metal, glass, and paper.</rdfs:comment>
        <rdfs:isDefinedBy rdf:resource="http://vocab.getty.edu/aat/"/>
        <rdfs:label xml:lang="en">molds (shaping equipment)</rdfs:label>
        <skos:inScheme rdf:resource="http://vocab.getty.edu/aat/"/>
    </owl:NamedIndividual>
    


    <!-- http://vocab.getty.edu/aat/300024928 -->


    <owl:NamedIndividual rdf:about="http://vocab.getty.edu/aat/300024928">
        <rdf:type rdf:resource="http://vocab.getty.edu/aat/Concept"/>
        <dc:identifier>300024928</dc:identifier>
        <rdfs:comment xml:lang="en">Tool handles, such as those of axes, hatchets, or hammers.</rdfs:comment>
        <rdfs:isDefinedBy rdf:resource="http://vocab.getty.edu/aat/"/>
        <rdfs:label xml:lang="en">helves</rdfs:label>
        <skos:inScheme rdf:resource="http://vocab.getty.edu/aat/"/>
    </owl:NamedIndividual>
    


    <!-- http://vocab.getty.edu/aat/300027349 -->


    <owl:NamedIndividual rdf:about="http://vocab.getty.edu/aat/300027349">
        <rdf:type rdf:resource="http://vocab.getty.edu/aat/Concept"/>
        <dc:identifier>300027349</dc:identifier>
        <rdfs:comment xml:lang="en">A conceptual grouping of visual arts works, literary works, or performance art created in succession by the same author, artist, or studio and intended by the creator(s) to be seen together.</rdfs:comment>
        <rdfs:isDefinedBy rdf:resource="http://vocab.getty.edu/aat/"/>
        <rdfs:label xml:lang="en">series (object groupings)</rdfs:label>
        <skos:inScheme rdf:resource="http://vocab.getty.edu/aat/"/>
    </owl:NamedIndividual>
    


    <!-- http://vocab.getty.edu/aat/300028051 -->


    <owl:NamedIndividual rdf:about="http://vocab.getty.edu/aat/300028051">
        <rdf:type rdf:resource="http://vocab.getty.edu/aat/Concept"/>
        <dc:identifier>300028051</dc:identifier>
        <rdfs:comment xml:lang="en">Items comprising a collection of leaves of paper, parchment, wood, stiffened textile, ivory, metal tablets, or other flat material, that are blank, written on, or printed, and are strung or bound together.</rdfs:comment>
        <rdfs:isDefinedBy rdf:resource="http://vocab.getty.edu/aat/"/>
        <rdfs:label xml:lang="en">books</rdfs:label>
        <skos:inScheme rdf:resource="http://vocab.getty.edu/aat/"/>
    </owl:NamedIndividual>
    


    <!-- http://vocab.getty.edu/aat/300028094 -->


    <owl:NamedIndividual rdf:about="http://vocab.getty.edu/aat/300028094">
        <rdf:type rdf:resource="http://vocab.getty.edu/aat/Concept"/>
        <dc:identifier>300028094</dc:identifier>
        <rdfs:comment xml:lang="en">Refers to graphic or photogrammetric representations of the Earth&apos;s surface or a part of it, including physical features and political boundaries.</rdfs:comment>
        <rdfs:isDefinedBy rdf:resource="http://vocab.getty.edu/aat/"/>
        <rdfs:label xml:lang="en">maps (documents)</rdfs:label>
        <skos:inScheme rdf:resource="http://vocab.getty.edu/aat/"/>
    </owl:NamedIndividual>
    


    <!-- http://vocab.getty.edu/aat/300028309 -->


    <owl:NamedIndividual rdf:about="http://vocab.getty.edu/aat/300028309">
        <rdf:type rdf:resource="http://vocab.getty.edu/aat/Concept"/>
        <dc:identifier>300028309</dc:identifier>
        <rdfs:comment xml:lang="en">Maps designed and used primarily for plotting courses and traveling on water in a ship or other vessel or in an aircraft or spacecraft.</rdfs:comment>
        <rdfs:isDefinedBy rdf:resource="http://vocab.getty.edu/aat/"/>
        <rdfs:label xml:lang="en">navigation charts</rdfs:label>
        <skos:inScheme rdf:resource="http://vocab.getty.edu/aat/"/>
    </owl:NamedIndividual>
    


    <!-- http://vocab.getty.edu/aat/300028569 -->


    <owl:NamedIndividual rdf:about="http://vocab.getty.edu/aat/300028569">
        <rdf:type rdf:resource="http://vocab.getty.edu/aat/Concept"/>
        <dc:identifier>300028569</dc:identifier>
        <rdfs:comment xml:lang="en">Handwritten documents, particularly books and other documents created before the invention of the printing press.</rdfs:comment>
        <rdfs:isDefinedBy rdf:resource="http://vocab.getty.edu/aat/"/>
        <rdfs:label xml:lang="en">manuscripts (documents)</rdfs:label>
        <skos:inScheme rdf:resource="http://vocab.getty.edu/aat/"/>
    </owl:NamedIndividual>
    


    <!-- http://vocab.getty.edu/aat/300028682 -->


    <owl:NamedIndividual rdf:about="http://vocab.getty.edu/aat/300028682">
        <rdf:type rdf:resource="http://vocab.getty.edu/aat/Concept"/>
        <dc:identifier>300028682</dc:identifier>
        <rdfs:comment xml:lang="en">Manifestations of motion pictures, stored electronically, in any media or digitized format.</rdfs:comment>
        <rdfs:isDefinedBy rdf:resource="http://vocab.getty.edu/aat/"/>
        <rdfs:label xml:lang="en">video recordings (physical artifacts)</rdfs:label>
        <skos:inScheme rdf:resource="http://vocab.getty.edu/aat/"/>
    </owl:NamedIndividual>
    


    <!-- http://vocab.getty.edu/aat/300033618 -->


    <owl:NamedIndividual rdf:about="http://vocab.getty.edu/aat/300033618">
        <rdf:type rdf:resource="http://vocab.getty.edu/aat/Concept"/>
        <dc:identifier>300033618</dc:identifier>
        <rdfs:comment xml:lang="en">Unique works in which images are formed primarily by the direct application of pigments suspended in oil, water, egg yolk, molten wax, or other liquid, arranged in masses of color, onto a general surface.</rdfs:comment>
        <rdfs:isDefinedBy rdf:resource="http://vocab.getty.edu/aat/"/>
        <rdfs:label xml:lang="en">paintings (visual works)</rdfs:label>
        <skos:inScheme rdf:resource="http://vocab.getty.edu/aat/"/>
    </owl:NamedIndividual>
    


    <!-- http://vocab.getty.edu/aat/300033799 -->


    <owl:NamedIndividual rdf:about="http://vocab.getty.edu/aat/300033799">
        <rdf:type rdf:resource="http://vocab.getty.edu/aat/Concept"/>
        <dc:identifier>300033799</dc:identifier>
        <rdfs:comment xml:lang="en">Creative works in the medium of oil paint.</rdfs:comment>
        <rdfs:isDefinedBy rdf:resource="http://vocab.getty.edu/aat/"/>
        <rdfs:label xml:lang="en">oil paintings (visual works)</rdfs:label>
        <skos:inScheme rdf:resource="http://vocab.getty.edu/aat/"/>
    </owl:NamedIndividual>
    


    <!-- http://vocab.getty.edu/aat/300037592 -->


    <owl:NamedIndividual rdf:about="http://vocab.getty.edu/aat/300037592">
        <rdf:type rdf:resource="http://vocab.getty.edu/aat/Concept"/>
        <dc:identifier>300037592</dc:identifier>
        <rdfs:comment xml:lang="en">Lighting devices having a vessel to contain fuel used as a source of illumination, such as grease or oil.</rdfs:comment>
        <rdfs:isDefinedBy rdf:resource="http://vocab.getty.edu/aat/"/>
        <rdfs:label xml:lang="en">lamps (lighting devices)</rdfs:label>
        <skos:inScheme rdf:resource="http://vocab.getty.edu/aat/"/>
    </owl:NamedIndividual>
    


    <!-- http://vocab.getty.edu/aat/300041273 -->


    <owl:NamedIndividual rdf:about="http://vocab.getty.edu/aat/300041273">
        <rdf:type rdf:resource="http://vocab.getty.edu/aat/Concept"/>
        <dc:identifier>300041273</dc:identifier>
        <rdfs:comment xml:lang="en">Pictorial works produced by transferring images by means of a matrix such as a plate, block, or screen, using any of various printing processes.</rdfs:comment>
        <rdfs:isDefinedBy rdf:resource="http://vocab.getty.edu/aat/"/>
        <rdfs:label xml:lang="en">prints (visual works)</rdfs:label>
        <skos:inScheme rdf:resource="http://vocab.getty.edu/aat/"/>
    </owl:NamedIndividual>
    


    <!-- http://vocab.getty.edu/aat/300041340 -->


    <owl:NamedIndividual rdf:about="http://vocab.getty.edu/aat/300041340">
        <rdf:type rdf:resource="http://vocab.getty.edu/aat/Concept"/>
        <dc:identifier>300041340</dc:identifier>
        <rdfs:comment xml:lang="en">Prints on paper incorporating impressions of a reverse design created on a printing plate, usually copper, into which the design has been incised (engraved) using burins or gravers.</rdfs:comment>
        <rdfs:isDefinedBy rdf:resource="http://vocab.getty.edu/aat/"/>
        <rdfs:label xml:lang="en">engravings (prints)</rdfs:label>
        <skos:inScheme rdf:resource="http://vocab.getty.edu/aat/"/>
    </owl:NamedIndividual>
    


    <!-- http://vocab.getty.edu/aat/300041405 -->


    <owl:NamedIndividual rdf:about="http://vocab.getty.edu/aat/300041405">
        <rdf:type rdf:resource="http://vocab.getty.edu/aat/Concept"/>
        <dc:identifier>300041405</dc:identifier>
        <rdfs:comment xml:lang="en">Prints made using the process of woodcut, which is a relief process in which the design is cut into and printed from the plank side of a wood block.</rdfs:comment>
        <rdfs:isDefinedBy rdf:resource="http://vocab.getty.edu/aat/"/>
        <rdfs:label xml:lang="en">woodcuts (prints)</rdfs:label>
        <skos:inScheme rdf:resource="http://vocab.getty.edu/aat/"/>
    </owl:NamedIndividual>
    


    <!-- http://vocab.getty.edu/aat/300041933 -->


    <owl:NamedIndividual rdf:about="http://vocab.getty.edu/aat/300041933">
        <rdf:type rdf:resource="http://vocab.getty.edu/aat/Concept"/>
        <dc:identifier>300041933</dc:identifier>
        <rdfs:comment xml:lang="en">Shaken idiophones made in a variety of forms worldwide, in which one or more objects strike against each other or against the inside or outside of another object.</rdfs:comment>
        <rdfs:isDefinedBy rdf:resource="http://vocab.getty.edu/aat/"/>
        <rdfs:label xml:lang="en">rattles (indirectly struck idiophones)</rdfs:label>
        <skos:inScheme rdf:resource="http://vocab.getty.edu/aat/"/>
    </owl:NamedIndividual>
    


    <!-- http://vocab.getty.edu/aat/300045627 -->


    <owl:NamedIndividual rdf:about="http://vocab.getty.edu/aat/300045627">
        <rdf:type rdf:resource="http://vocab.getty.edu/aat/Concept"/>
        <dc:identifier>300045627</dc:identifier>
        <rdfs:comment xml:lang="en">Vessels having a neck and mouth considerably narrower than the body, used for packaging and containing liquid and dry preparations.</rdfs:comment>
        <rdfs:isDefinedBy rdf:resource="http://vocab.getty.edu/aat/"/>
        <rdfs:label xml:lang="en">bottles</rdfs:label>
        <skos:inScheme rdf:resource="http://vocab.getty.edu/aat/"/>
    </owl:NamedIndividual>
    


    <!-- http://vocab.getty.edu/aat/300046001 -->


    <owl:NamedIndividual rdf:about="http://vocab.getty.edu/aat/300046001">
        <rdf:type rdf:resource="http://vocab.getty.edu/aat/Concept"/>
        <dc:identifier>300046001</dc:identifier>
        <rdfs:comment xml:lang="en">Ornaments worn around the neck, usually in the form of chains or strands of beads, pearls, stones, or decorative or precious materials, and often including a suspended ornamental pendant.</rdfs:comment>
        <rdfs:isDefinedBy rdf:resource="http://vocab.getty.edu/aat/"/>
        <rdfs:label xml:lang="en">necklaces</rdfs:label>
        <skos:inScheme rdf:resource="http://vocab.getty.edu/aat/"/>
    </owl:NamedIndividual>
    


    <!-- http://vocab.getty.edu/aat/300046025 -->


    <owl:NamedIndividual rdf:about="http://vocab.getty.edu/aat/300046025">
        <rdf:type rdf:resource="http://vocab.getty.edu/aat/Concept"/>
        <dc:identifier>300046025</dc:identifier>
        <rdfs:comment xml:lang="en">Small pieces of metal, usually gold, silver, or bronze and bearing a relief design on one or both sides and having a commemorative purpose.</rdfs:comment>
        <rdfs:isDefinedBy rdf:resource="http://vocab.getty.edu/aat/"/>
        <rdfs:label xml:lang="en">medals</rdfs:label>
        <skos:inScheme rdf:resource="http://vocab.getty.edu/aat/"/>
    </owl:NamedIndividual>
    


    <!-- http://vocab.getty.edu/aat/300047600 -->


    <owl:NamedIndividual rdf:about="http://vocab.getty.edu/aat/300047600">
        <rdf:type rdf:resource="http://vocab.getty.edu/aat/Concept"/>
        <dc:identifier>300047600</dc:identifier>
        <rdfs:comment xml:lang="en">Sculpture in the round, usually but not always depicting humans, animals, mythical beings, or small figure groups.</rdfs:comment>
        <rdfs:isDefinedBy rdf:resource="http://vocab.getty.edu/aat/"/>
        <rdfs:label xml:lang="en">statues</rdfs:label>
        <skos:inScheme rdf:resource="http://vocab.getty.edu/aat/"/>
    </owl:NamedIndividual>
    


    <!-- http://vocab.getty.edu/aat/300047753 -->


    <owl:NamedIndividual rdf:about="http://vocab.getty.edu/aat/300047753">
        <rdf:type rdf:resource="http://vocab.getty.edu/aat/Concept"/>
        <dc:identifier>300047753</dc:identifier>
        <rdfs:comment xml:lang="en">Refers to scaled or lifesize representations of objects, structures, beings, or other subjects, usually three-dimensional.</rdfs:comment>
        <rdfs:isDefinedBy rdf:resource="http://vocab.getty.edu/aat/"/>
        <rdfs:label xml:lang="en">models (representations)</rdfs:label>
        <skos:inScheme rdf:resource="http://vocab.getty.edu/aat/"/>
    </owl:NamedIndividual>
    


    <!-- http://vocab.getty.edu/aat/300047762 -->


    <owl:NamedIndividual rdf:about="http://vocab.getty.edu/aat/300047762">
        <rdf:type rdf:resource="http://vocab.getty.edu/aat/Concept"/>
        <dc:identifier>300047762</dc:identifier>
        <rdfs:comment xml:lang="en">Works in which three-dimensional objects, often figural sculpture, in the foreground blend with a realistic painted background.</rdfs:comment>
        <rdfs:isDefinedBy rdf:resource="http://vocab.getty.edu/aat/"/>
        <rdfs:label xml:lang="en">dioramas</rdfs:label>
        <skos:inScheme rdf:resource="http://vocab.getty.edu/aat/"/>
    </owl:NamedIndividual>
    


    <!-- http://vocab.getty.edu/aat/300051658 -->


    <owl:NamedIndividual rdf:about="http://vocab.getty.edu/aat/300051658">
        <rdf:type rdf:resource="http://vocab.getty.edu/aat/Concept"/>
        <dc:identifier>300051658</dc:identifier>
        <rdfs:comment xml:lang="en">Long-bladed weapons with a hilt and usually a hand guard, used primarily for cutting or thrusting.</rdfs:comment>
        <rdfs:isDefinedBy rdf:resource="http://vocab.getty.edu/aat/"/>
        <rdfs:label xml:lang="en">swords</rdfs:label>
        <skos:inScheme rdf:resource="http://vocab.getty.edu/aat/"/>
    </owl:NamedIndividual>
    


    <!-- http://vocab.getty.edu/aat/300053225 -->


    <owl:NamedIndividual rdf:about="http://vocab.getty.edu/aat/300053225">
        <rdf:type rdf:resource="http://vocab.getty.edu/aat/Concept"/>
        <dc:identifier>300053225</dc:identifier>
        <rdfs:comment xml:lang="en">The intaglio process in which the design is incised into a printing plate, usually a flat copper plate, with the aid of a graver or burin.</rdfs:comment>
        <rdfs:isDefinedBy rdf:resource="http://vocab.getty.edu/aat/"/>
        <rdfs:label xml:lang="en">engraving (printing process)</rdfs:label>
        <skos:inScheme rdf:resource="http://vocab.getty.edu/aat/"/>
    </owl:NamedIndividual>
    


    <!-- http://vocab.getty.edu/aat/300053357 -->


    <owl:NamedIndividual rdf:about="http://vocab.getty.edu/aat/300053357">
        <rdf:type rdf:resource="http://vocab.getty.edu/aat/Concept"/>
        <dc:identifier>300053357</dc:identifier>
        <rdfs:comment xml:lang="en">Mural painting technique in which dry pigments are ground with water then brushed onto wet or partially dry lime plaster.</rdfs:comment>
        <rdfs:isDefinedBy rdf:resource="http://vocab.getty.edu/aat/"/>
        <rdfs:label xml:lang="en">fresco painting (technique)</rdfs:label>
        <skos:inScheme rdf:resource="http://vocab.getty.edu/aat/"/>
    </owl:NamedIndividual>
    


    <!-- http://vocab.getty.edu/aat/300053363 -->


    <owl:NamedIndividual rdf:about="http://vocab.getty.edu/aat/300053363">
        <rdf:type rdf:resource="http://vocab.getty.edu/aat/Concept"/>
        <dc:identifier>300053363</dc:identifier>
        <rdfs:comment xml:lang="en">Watercolor painting done in transparent washes of color as distinguished from the opaque method using gouache.</rdfs:comment>
        <rdfs:isDefinedBy rdf:resource="http://vocab.getty.edu/aat/"/>
        <rdfs:label xml:lang="en">aquarelle (technique)</rdfs:label>
        <skos:inScheme rdf:resource="http://vocab.getty.edu/aat/"/>
    </owl:NamedIndividual>
    


    <!-- http://vocab.getty.edu/aat/300053580 -->


    <owl:NamedIndividual rdf:about="http://vocab.getty.edu/aat/300053580">
        <rdf:type rdf:resource="http://vocab.getty.edu/aat/Concept"/>
        <dc:identifier>300053580</dc:identifier>
        <rdfs:comment xml:lang="en">Refers to the technique of making measurements by using photography. It usually refers to this technique as applied to mapmaking, measuring site elements, and surveying.</rdfs:comment>
        <rdfs:isDefinedBy rdf:resource="http://vocab.getty.edu/aat/"/>
        <rdfs:label xml:lang="en">photogrammetry</rdfs:label>
        <skos:inScheme rdf:resource="http://vocab.getty.edu/aat/"/>
    </owl:NamedIndividual>
    


    <!-- http://vocab.getty.edu/aat/300053628 -->


    <owl:NamedIndividual rdf:about="http://vocab.getty.edu/aat/300053628">
        <rdf:type rdf:resource="http://vocab.getty.edu/aat/Concept"/>
        <dc:identifier>300053628</dc:identifier>
        <rdfs:comment xml:lang="en">Preparing lifelike representations of animals by stuffing the skin or molding it around a model of the specimen.</rdfs:comment>
        <rdfs:isDefinedBy rdf:resource="http://vocab.getty.edu/aat/"/>
        <rdfs:label xml:lang="en">taxidermy</rdfs:label>
        <skos:inScheme rdf:resource="http://vocab.getty.edu/aat/"/>
    </owl:NamedIndividual>
    


    <!-- http://vocab.getty.edu/aat/300053758 -->


    <owl:NamedIndividual rdf:about="http://vocab.getty.edu/aat/300053758">
        <rdf:type rdf:resource="http://vocab.getty.edu/aat/Concept"/>
        <dc:identifier>300053758</dc:identifier>
        <rdfs:comment xml:lang="en">Making free or nearly free of liquids.</rdfs:comment>
        <rdfs:isDefinedBy rdf:resource="http://vocab.getty.edu/aat/"/>
        <rdfs:label xml:lang="en">drying</rdfs:label>
        <skos:inScheme rdf:resource="http://vocab.getty.edu/aat/"/>
    </owl:NamedIndividual>
    


    <!-- http://vocab.getty.edu/aat/300053852 -->


    <owl:NamedIndividual rdf:about="http://vocab.getty.edu/aat/300053852">
        <rdf:type rdf:resource="http://vocab.getty.edu/aat/Concept"/>
        <dc:identifier>300053852</dc:identifier>
        <rdfs:comment xml:lang="en">Decorative wood process in which the design or pattern is made by assembling small pieces of veneer in various shapes.</rdfs:comment>
        <rdfs:isDefinedBy rdf:resource="http://vocab.getty.edu/aat/"/>
        <rdfs:label xml:lang="en">intarsia (process)</rdfs:label>
        <skos:inScheme rdf:resource="http://vocab.getty.edu/aat/"/>
    </owl:NamedIndividual>
    


    <!-- http://vocab.getty.edu/aat/300054196 -->


    <owl:NamedIndividual rdf:about="http://vocab.getty.edu/aat/300054196">
        <rdf:type rdf:resource="http://vocab.getty.edu/aat/Concept"/>
        <dc:identifier>300054196</dc:identifier>
        <rdfs:comment xml:lang="en">Producing visible forms primarily by delineation, usually by the direct application of material or instrument to the surface of the support.</rdfs:comment>
        <rdfs:isDefinedBy rdf:resource="http://vocab.getty.edu/aat/"/>
        <rdfs:label xml:lang="en">drawing (image-making)</rdfs:label>
        <skos:inScheme rdf:resource="http://vocab.getty.edu/aat/"/>
    </owl:NamedIndividual>
    


    <!-- http://vocab.getty.edu/aat/300054200 -->


    <owl:NamedIndividual rdf:about="http://vocab.getty.edu/aat/300054200">
        <rdf:type rdf:resource="http://vocab.getty.edu/aat/Concept"/>
        <dc:identifier>300054200</dc:identifier>
        <rdfs:comment xml:lang="en">The art or process of providing drawings or other pictures intended to elucidate a description, story, or other written material, usually in a book or periodical.</rdfs:comment>
        <rdfs:isDefinedBy rdf:resource="http://vocab.getty.edu/aat/"/>
        <rdfs:label xml:lang="en">illustration (process)</rdfs:label>
        <skos:inScheme rdf:resource="http://vocab.getty.edu/aat/"/>
    </owl:NamedIndividual>
    


    <!-- http://vocab.getty.edu/aat/300054636 -->


    <owl:NamedIndividual rdf:about="http://vocab.getty.edu/aat/300054636">
        <rdf:type rdf:resource="http://vocab.getty.edu/aat/Concept"/>
        <dc:identifier>300054636</dc:identifier>
        <rdfs:comment xml:lang="en">Creating and manipulating data in machine-readable form by means of computers, including inputting, storage, conversion, editing, and printing.</rdfs:comment>
        <rdfs:isDefinedBy rdf:resource="http://vocab.getty.edu/aat/"/>
        <rdfs:label xml:lang="en">data processing</rdfs:label>
        <skos:inScheme rdf:resource="http://vocab.getty.edu/aat/"/>
    </owl:NamedIndividual>
    


    <!-- http://vocab.getty.edu/aat/300054638 -->


    <owl:NamedIndividual rdf:about="http://vocab.getty.edu/aat/300054638">
        <rdf:type rdf:resource="http://vocab.getty.edu/aat/Concept"/>
        <dc:identifier>300054638</dc:identifier>
        <rdfs:comment xml:lang="en">The process or function of gathering and recording information, especially to record facts or characteristics or to establish evidence or testimony.</rdfs:comment>
        <rdfs:isDefinedBy rdf:resource="http://vocab.getty.edu/aat/"/>
        <rdfs:label xml:lang="en">documentation (activity)</rdfs:label>
        <skos:inScheme rdf:resource="http://vocab.getty.edu/aat/"/>
    </owl:NamedIndividual>
    


    <!-- http://vocab.getty.edu/aat/300054686 -->


    <owl:NamedIndividual rdf:about="http://vocab.getty.edu/aat/300054686">
        <rdf:type rdf:resource="http://vocab.getty.edu/aat/Concept"/>
        <dc:identifier>300054686</dc:identifier>
        <rdfs:comment xml:lang="en">The actions, functions, or event of issuing printed, taped, or otherwise reproduced records of knowledge or visual works in any medium for sale or distribution to the public.</rdfs:comment>
        <rdfs:isDefinedBy rdf:resource="http://vocab.getty.edu/aat/"/>
        <rdfs:label xml:lang="en">publishing</rdfs:label>
        <skos:inScheme rdf:resource="http://vocab.getty.edu/aat/"/>
    </owl:NamedIndividual>
    


    <!-- http://vocab.getty.edu/aat/300054698 -->


    <owl:NamedIndividual rdf:about="http://vocab.getty.edu/aat/300054698">
        <rdf:type rdf:resource="http://vocab.getty.edu/aat/Concept"/>
        <dc:identifier>300054698</dc:identifier>
        <rdfs:comment xml:lang="en">Forming or producing letters to record the ideas which characters and words express or to communicate the ideas by visible signs.</rdfs:comment>
        <rdfs:isDefinedBy rdf:resource="http://vocab.getty.edu/aat/"/>
        <rdfs:label xml:lang="en">writing (processes)</rdfs:label>
        <skos:inScheme rdf:resource="http://vocab.getty.edu/aat/"/>
    </owl:NamedIndividual>
    


    <!-- http://vocab.getty.edu/aat/300055021 -->


    <owl:NamedIndividual rdf:about="http://vocab.getty.edu/aat/300055021">
        <rdf:type rdf:resource="http://vocab.getty.edu/aat/Concept"/>
        <dc:identifier>300055021</dc:identifier>
        <rdfs:comment xml:lang="en">Books printed before 1501.</rdfs:comment>
        <rdfs:isDefinedBy rdf:resource="http://vocab.getty.edu/aat/"/>
        <rdfs:label xml:lang="en">incunabula (books)</rdfs:label>
        <skos:inScheme rdf:resource="http://vocab.getty.edu/aat/"/>
    </owl:NamedIndividual>
    


    <!-- http://vocab.getty.edu/aat/300063663 -->


    <owl:NamedIndividual rdf:about="http://vocab.getty.edu/aat/300063663">
        <rdf:type rdf:resource="http://vocab.getty.edu/aat/Concept"/>
        <dc:identifier>300063663</dc:identifier>
        <rdfs:comment xml:lang="en">Japanese sword guards, usually made of metal and serving to protect the hand from sliding forward on to the blade.</rdfs:comment>
        <rdfs:isDefinedBy rdf:resource="http://vocab.getty.edu/aat/"/>
        <rdfs:label xml:lang="en">tsuba</rdfs:label>
        <skos:inScheme rdf:resource="http://vocab.getty.edu/aat/"/>
    </owl:NamedIndividual>
    


    <!-- http://vocab.getty.edu/aat/300069831 -->


    <owl:NamedIndividual rdf:about="http://vocab.getty.edu/aat/300069831">
        <rdf:type rdf:resource="http://vocab.getty.edu/aat/Concept"/>
        <dc:identifier>300069831</dc:identifier>
        <rdfs:comment xml:lang="en">The activity of comprehending, analyzing, and expressing written or spoken material in a different language from the original.</rdfs:comment>
        <rdfs:isDefinedBy rdf:resource="http://vocab.getty.edu/aat/"/>
        <rdfs:label xml:lang="en">translation (function)</rdfs:label>
        <skos:inScheme rdf:resource="http://vocab.getty.edu/aat/"/>
    </owl:NamedIndividual>
    


    <!-- http://vocab.getty.edu/aat/300077565 -->


    <owl:NamedIndividual rdf:about="http://vocab.getty.edu/aat/300077565">
        <rdf:type rdf:resource="http://vocab.getty.edu/aat/Concept"/>
        <dc:identifier>300077565</dc:identifier>
        <rdfs:comment xml:lang="en">The action or process of making something ready for use or service or of getting ready for some occasion, test, or duty.</rdfs:comment>
        <rdfs:isDefinedBy rdf:resource="http://vocab.getty.edu/aat/"/>
        <rdfs:label xml:lang="en">preparing</rdfs:label>
        <skos:inScheme rdf:resource="http://vocab.getty.edu/aat/"/>
    </owl:NamedIndividual>
    


    <!-- http://vocab.getty.edu/aat/300117127 -->


    <owl:NamedIndividual rdf:about="http://vocab.getty.edu/aat/300117127">
        <rdf:type rdf:resource="http://vocab.getty.edu/aat/Concept"/>
        <dc:identifier>300117127</dc:identifier>
        <rdfs:comment xml:lang="en">Generally, objects or other things made or modified by humans, typically manually portable products of human workmanship, such as tools, utensils, objects for personal adornment, or art.</rdfs:comment>
        <rdfs:isDefinedBy rdf:resource="http://vocab.getty.edu/aat/"/>
        <rdfs:label xml:lang="en">artifacts (object genre)</rdfs:label>
        <skos:inScheme rdf:resource="http://vocab.getty.edu/aat/"/>
    </owl:NamedIndividual>
    


    <!-- http://vocab.getty.edu/aat/300122241 -->


    <owl:NamedIndividual rdf:about="http://vocab.getty.edu/aat/300122241">
        <rdf:type rdf:resource="http://vocab.getty.edu/aat/Concept"/>
        <dc:identifier>300122241</dc:identifier>
        <rdfs:comment xml:lang="en">Articles or physical resources used to array, dress up, rig out, equip, or otherwise provide with what is requisite for efficient action by a person or animal or for a thing.</rdfs:comment>
        <rdfs:isDefinedBy rdf:resource="http://vocab.getty.edu/aat/"/>
        <rdfs:label xml:lang="en">equipment</rdfs:label>
        <skos:inScheme rdf:resource="http://vocab.getty.edu/aat/"/>
    </owl:NamedIndividual>
    


    <!-- http://vocab.getty.edu/aat/300132254 -->


    <owl:NamedIndividual rdf:about="http://vocab.getty.edu/aat/300132254">
        <rdf:type rdf:resource="http://vocab.getty.edu/aat/Concept"/>
        <dc:identifier>300132254</dc:identifier>
        <rdfs:comment xml:lang="en">Vessels of varying shape and size but which are usually taller than they are wide, varying greatly in actual form and use.</rdfs:comment>
        <rdfs:isDefinedBy rdf:resource="http://vocab.getty.edu/aat/"/>
        <rdfs:label xml:lang="en">vases</rdfs:label>
        <skos:inScheme rdf:resource="http://vocab.getty.edu/aat/"/>
    </owl:NamedIndividual>
    


    <!-- http://vocab.getty.edu/aat/300137376 -->


    <owl:NamedIndividual rdf:about="http://vocab.getty.edu/aat/300137376">
        <rdf:type rdf:resource="http://vocab.getty.edu/aat/Concept"/>
        <dc:identifier>300137376</dc:identifier>
        <rdfs:comment xml:lang="en">Medieval marine charts, used before compasses, and for Medieval navigation manuals, illustrated with charts and showing the location of ports and other navigational information.</rdfs:comment>
        <rdfs:isDefinedBy rdf:resource="http://vocab.getty.edu/aat/"/>
        <rdfs:label xml:lang="en">portolanos</rdfs:label>
        <skos:inScheme rdf:resource="http://vocab.getty.edu/aat/"/>
    </owl:NamedIndividual>
    


    <!-- http://vocab.getty.edu/aat/300138684 -->


    <owl:NamedIndividual rdf:about="http://vocab.getty.edu/aat/300138684">
        <rdf:type rdf:resource="http://vocab.getty.edu/aat/Concept"/>
        <dc:identifier>300138684</dc:identifier>
        <rdfs:comment xml:lang="en">A method of decorating surfaces with patterns or pictures composed of small, regularly-shaped pieces of colored durable material, such as stone or glass.</rdfs:comment>
        <rdfs:isDefinedBy rdf:resource="http://vocab.getty.edu/aat/"/>
        <rdfs:label xml:lang="en">mosaic (process)</rdfs:label>
        <skos:inScheme rdf:resource="http://vocab.getty.edu/aat/"/>
    </owl:NamedIndividual>
    


    <!-- http://vocab.getty.edu/aat/300138758 -->


    <owl:NamedIndividual rdf:about="http://vocab.getty.edu/aat/300138758">
        <rdf:type rdf:resource="http://vocab.getty.edu/aat/Concept"/>
        <dc:identifier>300138758</dc:identifier>
        <rdfs:comment xml:lang="en">Refers to coverings for all or part of the face, usually with openings for the eyes and sometimes the mouth.</rdfs:comment>
        <rdfs:isDefinedBy rdf:resource="http://vocab.getty.edu/aat/"/>
        <rdfs:label xml:lang="en">masks (costume)</rdfs:label>
        <skos:inScheme rdf:resource="http://vocab.getty.edu/aat/"/>
    </owl:NamedIndividual>
    


    <!-- http://vocab.getty.edu/aat/300155365 -->


    <owl:NamedIndividual rdf:about="http://vocab.getty.edu/aat/300155365">
        <rdf:type rdf:resource="http://vocab.getty.edu/aat/Concept"/>
        <dc:identifier>300155365</dc:identifier>
        <rdfs:comment xml:lang="en">Publishing text or images in electronic machine-readable formats.</rdfs:comment>
        <rdfs:isDefinedBy rdf:resource="http://vocab.getty.edu/aat/"/>
        <rdfs:label xml:lang="en">electronic publishing</rdfs:label>
        <skos:inScheme rdf:resource="http://vocab.getty.edu/aat/"/>
    </owl:NamedIndividual>
    


    <!-- http://vocab.getty.edu/aat/300178926 -->


    <owl:NamedIndividual rdf:about="http://vocab.getty.edu/aat/300178926">
        <rdf:type rdf:resource="http://vocab.getty.edu/aat/Concept"/>
        <dc:identifier>300178926</dc:identifier>
        <rdfs:comment xml:lang="en">Printing from raised and inked type, distinguished from lithographic or intaglio printing, particularly in the context of book and other text printing.</rdfs:comment>
        <rdfs:isDefinedBy rdf:resource="http://vocab.getty.edu/aat/"/>
        <rdfs:label xml:lang="en">letterpress printing</rdfs:label>
        <skos:inScheme rdf:resource="http://vocab.getty.edu/aat/"/>
    </owl:NamedIndividual>
    


    <!-- http://vocab.getty.edu/aat/300184300 -->


    <owl:NamedIndividual rdf:about="http://vocab.getty.edu/aat/300184300">
        <rdf:type rdf:resource="http://vocab.getty.edu/aat/Concept"/>
        <dc:identifier>300184300</dc:identifier>
        <rdfs:comment xml:lang="en">Refers to series of visual works depicting events and unified by a common topic, not necessarily a sequence in a single story line.</rdfs:comment>
        <rdfs:isDefinedBy rdf:resource="http://vocab.getty.edu/aat/"/>
        <rdfs:label xml:lang="en">narrative cycles</rdfs:label>
        <skos:inScheme rdf:resource="http://vocab.getty.edu/aat/"/>
    </owl:NamedIndividual>
    


    <!-- http://vocab.getty.edu/aat/300189634 -->


    <owl:NamedIndividual rdf:about="http://vocab.getty.edu/aat/300189634">
        <rdf:type rdf:resource="http://vocab.getty.edu/aat/Concept"/>
        <dc:identifier>300189634</dc:identifier>
        <rdfs:comment xml:lang="en">Groups of prints related in theme or technique and usually issued together.</rdfs:comment>
        <rdfs:isDefinedBy rdf:resource="http://vocab.getty.edu/aat/"/>
        <rdfs:label xml:lang="en">suites (print groupings)</rdfs:label>
        <skos:inScheme rdf:resource="http://vocab.getty.edu/aat/"/>
    </owl:NamedIndividual>
    


    <!-- http://vocab.getty.edu/aat/300191086 -->


    <owl:NamedIndividual rdf:about="http://vocab.getty.edu/aat/300191086">
        <rdf:type rdf:resource="http://vocab.getty.edu/aat/Concept"/>
        <dc:identifier>300191086</dc:identifier>
        <rdfs:comment xml:lang="en">Works of art, architecture, and any objects that occupy space, are perceived by the sense of sight, and are created or arranged, rather than naturally occurring.</rdfs:comment>
        <rdfs:isDefinedBy rdf:resource="http://vocab.getty.edu/aat/"/>
        <rdfs:label xml:lang="en">visual works (works)</rdfs:label>
        <skos:inScheme rdf:resource="http://vocab.getty.edu/aat/"/>
    </owl:NamedIndividual>
    


    <!-- http://vocab.getty.edu/aat/300224200 -->


    <owl:NamedIndividual rdf:about="http://vocab.getty.edu/aat/300224200">
        <rdf:type rdf:resource="http://vocab.getty.edu/aat/Concept"/>
        <dc:identifier>300224200</dc:identifier>
        <rdfs:comment xml:lang="en">Ancient manuscripts generally taking the form of the modern book: bound leaves of paper or parchment with information inscribed on both faces, attached at a center fold.</rdfs:comment>
        <rdfs:isDefinedBy rdf:resource="http://vocab.getty.edu/aat/"/>
        <rdfs:label xml:lang="en">codices (bound manuscripts)</rdfs:label>
        <skos:inScheme rdf:resource="http://vocab.getty.edu/aat/"/>
    </owl:NamedIndividual>
    


    <!-- http://vocab.getty.edu/aat/300226836 -->


    <owl:NamedIndividual rdf:about="http://vocab.getty.edu/aat/300226836">
        <rdf:type rdf:resource="http://vocab.getty.edu/aat/Concept"/>
        <dc:identifier>300226836</dc:identifier>
        <rdfs:comment xml:lang="en">Sets or ensembles of visual works.</rdfs:comment>
        <rdfs:isDefinedBy rdf:resource="http://vocab.getty.edu/aat/"/>
        <rdfs:label xml:lang="en">visual works groupings</rdfs:label>
        <skos:inScheme rdf:resource="http://vocab.getty.edu/aat/"/>
    </owl:NamedIndividual>
    


    <!-- http://vocab.getty.edu/aat/300235576 -->


    <owl:NamedIndividual rdf:about="http://vocab.getty.edu/aat/300235576">
        <rdf:type rdf:resource="http://vocab.getty.edu/aat/Concept"/>
        <dc:identifier>300235576</dc:identifier>
        <rdfs:comment xml:lang="en">A specimen is an individual instance that represents a class. A good specimen shows the character of the thing or material, useful for close study and permitting exact identification.</rdfs:comment>
        <rdfs:isDefinedBy rdf:resource="http://vocab.getty.edu/aat/"/>
        <rdfs:label xml:lang="en">specimens</rdfs:label>
        <skos:inScheme rdf:resource="http://vocab.getty.edu/aat/"/>
    </owl:NamedIndividual>
    


    <!-- http://vocab.getty.edu/aat/300252927 -->


    <owl:NamedIndividual rdf:about="http://vocab.getty.edu/aat/300252927">
        <rdf:type rdf:resource="http://vocab.getty.edu/aat/Concept"/>
        <dc:identifier>300252927</dc:identifier>
        <rdfs:comment xml:lang="en">The forming of letters and words by hand rather than by printing; may be used to designate a particular and distinctive form, style, or method of writing by hand.</rdfs:comment>
        <rdfs:isDefinedBy rdf:resource="http://vocab.getty.edu/aat/"/>
        <rdfs:label xml:lang="en">handwriting</rdfs:label>
        <skos:inScheme rdf:resource="http://vocab.getty.edu/aat/"/>
    </owl:NamedIndividual>
    


    <!-- http://vocab.getty.edu/aat/300264383 -->


    <owl:NamedIndividual rdf:about="http://vocab.getty.edu/aat/300264383">
        <rdf:type rdf:resource="http://vocab.getty.edu/aat/Concept"/>
        <dc:identifier>300264383</dc:identifier>
        <rdfs:comment xml:lang="en">Refers to the process or branch of fine art concerned with creating sculpture, which are three-dimensional works.</rdfs:comment>
        <rdfs:isDefinedBy rdf:resource="http://vocab.getty.edu/aat/"/>
        <rdfs:label xml:lang="en">sculpting</rdfs:label>
        <skos:inScheme rdf:resource="http://vocab.getty.edu/aat/"/>
    </owl:NamedIndividual>
    


    <!-- http://vocab.getty.edu/aat/300265248 -->


    <owl:NamedIndividual rdf:about="http://vocab.getty.edu/aat/300265248">
        <rdf:type rdf:resource="http://vocab.getty.edu/aat/Concept"/>
        <dc:identifier>300265248</dc:identifier>
        <rdfs:comment xml:lang="en">Any technique for forming or shaping wax into sculptural shapes, either for casting purposes or as a final work.</rdfs:comment>
        <rdfs:isDefinedBy rdf:resource="http://vocab.getty.edu/aat/"/>
        <rdfs:label xml:lang="en">wax-modeling</rdfs:label>
        <skos:inScheme rdf:resource="http://vocab.getty.edu/aat/"/>
    </owl:NamedIndividual>
    


    <!-- http://vocab.getty.edu/aat/300265483 -->


    <owl:NamedIndividual rdf:about="http://vocab.getty.edu/aat/300265483">
        <rdf:type rdf:resource="http://vocab.getty.edu/aat/Concept"/>
        <dc:identifier>300265483</dc:identifier>
        <rdfs:comment xml:lang="en">Handwritten manuscripts that have been decorated with gold or silver, brilliant colors, designs, or miniature pictures.</rdfs:comment>
        <rdfs:isDefinedBy rdf:resource="http://vocab.getty.edu/aat/"/>
        <rdfs:label xml:lang="en">illuminated manuscripts</rdfs:label>
        <skos:inScheme rdf:resource="http://vocab.getty.edu/aat/"/>
    </owl:NamedIndividual>
    


    <!-- http://vocab.getty.edu/aat/300265632 -->


    <owl:NamedIndividual rdf:about="http://vocab.getty.edu/aat/300265632">
        <rdf:type rdf:resource="http://vocab.getty.edu/aat/Concept"/>
        <dc:identifier>300265632</dc:identifier>
        <rdfs:comment xml:lang="en">Objects comprising sheets of paper, vellum, papyrus, or another material that are bound together. Volumes may include printed books, manuscripts, sketchbooks, or albums.</rdfs:comment>
        <rdfs:isDefinedBy rdf:resource="http://vocab.getty.edu/aat/"/>
        <rdfs:label xml:lang="en">volumes (documents by form)</rdfs:label>
        <skos:inScheme rdf:resource="http://vocab.getty.edu/aat/"/>
    </owl:NamedIndividual>
    


    <!-- http://vocab.getty.edu/aat/300266792 -->


    <owl:NamedIndividual rdf:about="http://vocab.getty.edu/aat/300266792">
        <rdf:type rdf:resource="http://vocab.getty.edu/aat/Concept"/>
        <dc:identifier>300266792</dc:identifier>
        <rdfs:comment xml:lang="en">Cameras capable of acquiring still or motion pictures via an electronic sensor and storing them as digital information on a memory device.</rdfs:comment>
        <rdfs:isDefinedBy rdf:resource="http://vocab.getty.edu/aat/"/>
        <rdfs:label xml:lang="en">digital cameras</rdfs:label>
        <skos:inScheme rdf:resource="http://vocab.getty.edu/aat/"/>
    </owl:NamedIndividual>
    


    <!-- http://vocab.getty.edu/aat/300312355 -->


    <owl:NamedIndividual rdf:about="http://vocab.getty.edu/aat/300312355">
        <rdf:type rdf:resource="http://vocab.getty.edu/aat/Concept"/>
        <dc:identifier>300312355</dc:identifier>
        <rdfs:comment xml:lang="en">Numeric, alphanumeric, or other identifying codes assigned when an art object, book, or other item enters the collection of a museum, library, or other repository.</rdfs:comment>
        <rdfs:isDefinedBy rdf:resource="http://vocab.getty.edu/aat/"/>
        <rdfs:label xml:lang="en">accession numbers</rdfs:label>
        <skos:inScheme rdf:resource="http://vocab.getty.edu/aat/"/>
    </owl:NamedIndividual>
    


    <!-- http://vocab.getty.edu/aat/300343820 -->


    <owl:NamedIndividual rdf:about="http://vocab.getty.edu/aat/300343820">
        <rdf:type rdf:resource="http://vocab.getty.edu/aat/Concept"/>
        <dc:identifier>300343820</dc:identifier>
        <rdfs:comment xml:lang="en">The process and technique of creating two-dimensional decoration on pottery by using paint made of metallic oxides or other pigments held in suspension in slip or another medium.</rdfs:comment>
        <rdfs:isDefinedBy rdf:resource="http://vocab.getty.edu/aat/"/>
        <rdfs:label xml:lang="en">vase painting (image-making)</rdfs:label>
        <skos:inScheme rdf:resource="http://vocab.getty.edu/aat/"/>
    </owl:NamedIndividual>
    


    <!-- http://vocab.getty.edu/aat/300386427 -->


    <owl:NamedIndividual rdf:about="http://vocab.getty.edu/aat/300386427">
        <rdf:type rdf:resource="http://vocab.getty.edu/aat/Concept"/>
        <dc:identifier>300386427</dc:identifier>
        <rdfs:comment xml:lang="en">Reduction of data needed for storage or transmission. Data is reduced in volume by means of encoding information to require fewer bits to be stored than the original.</rdfs:comment>
        <rdfs:isDefinedBy rdf:resource="http://vocab.getty.edu/aat/"/>
        <rdfs:label xml:lang="en">data compression</rdfs:label>
        <skos:inScheme rdf:resource="http://vocab.getty.edu/aat/"/>
    </owl:NamedIndividual>
    


    <!-- http://vocab.getty.edu/aat/300391312 -->


    <owl:NamedIndividual rdf:about="http://vocab.getty.edu/aat/300391312">
        <rdf:type rdf:resource="http://vocab.getty.edu/aat/Concept"/>
        <dc:identifier>300391312</dc:identifier>
        <rdfs:comment xml:lang="en">Scanning technique that involves a pattern of lines projected onto a 3-D object and the subsequent mathematical measurement of the deformations caused by the geometry of the object.</rdfs:comment>
        <rdfs:isDefinedBy rdf:resource="http://vocab.getty.edu/aat/"/>
        <rdfs:label xml:lang="en">structured light scanning</rdfs:label>
        <skos:inScheme rdf:resource="http://vocab.getty.edu/aat/"/>
    </owl:NamedIndividual>
    


    <!-- http://vocab.getty.edu/aat/300391447 -->


    <owl:NamedIndividual rdf:about="http://vocab.getty.edu/aat/300391447">
        <rdf:type rdf:resource="http://vocab.getty.edu/aat/Concept"/>
        <dc:identifier>300391447</dc:identifier>
        <rdfs:comment xml:lang="en">Computer software technique for rendering virtual models of surfaces in three-dimensions.</rdfs:comment>
        <rdfs:isDefinedBy rdf:resource="http://vocab.getty.edu/aat/"/>
        <rdfs:label xml:lang="en">digital surface modeling</rdfs:label>
        <skos:inScheme rdf:resource="http://vocab.getty.edu/aat/"/>
    </owl:NamedIndividual>
    


    <!-- http://vocab.getty.edu/aat/300403970 -->


    <owl:NamedIndividual rdf:about="http://vocab.getty.edu/aat/300403970">
        <rdf:type rdf:resource="http://vocab.getty.edu/aat/Concept"/>
        <dc:identifier>300403970</dc:identifier>
        <rdfs:comment xml:lang="en">Manuscript volumes comprising two or more works, whether referring to only the content combined or to the combination of physically separate leafs or gatherings that are sewn or tipped in</rdfs:comment>
        <rdfs:isDefinedBy rdf:resource="http://vocab.getty.edu/aat/"/>
        <rdfs:label xml:lang="en">compilation manuscripts</rdfs:label>
        <skos:inScheme rdf:resource="http://vocab.getty.edu/aat/"/>
    </owl:NamedIndividual>
    


    <!-- http://vocab.getty.edu/aat/300404386 -->


    <owl:NamedIndividual rdf:about="http://vocab.getty.edu/aat/300404386">
        <rdf:type rdf:resource="http://vocab.getty.edu/aat/Concept"/>
        <dc:identifier>300404386</dc:identifier>
        <rdfs:comment xml:lang="en">Events or activities of finding out or becoming aware of something that had been lost, forgotten, or previously unknown. Includes the finding of archaeological objects, lost buildings, places.</rdfs:comment>
        <rdfs:isDefinedBy rdf:resource="http://vocab.getty.edu/aat/"/>
        <rdfs:label xml:lang="en">discoveries</rdfs:label>
        <skos:inScheme rdf:resource="http://vocab.getty.edu/aat/"/>
    </owl:NamedIndividual>
    


    <!-- http://vocab.getty.edu/aat/300404704 -->


    <owl:NamedIndividual rdf:about="http://vocab.getty.edu/aat/300404704">
        <rdf:type rdf:resource="http://vocab.getty.edu/aat/Concept"/>
        <dc:identifier>300404704</dc:identifier>
        <rdfs:comment xml:lang="en">Identifying numeric or alpha codes found, usually on the spine, of a manuscript, book or other volume, giving the location where the item can be found in the library.</rdfs:comment>
        <rdfs:isDefinedBy rdf:resource="http://vocab.getty.edu/aat/"/>
        <rdfs:label xml:lang="en">shelf marks</rdfs:label>
        <skos:inScheme rdf:resource="http://vocab.getty.edu/aat/"/>
    </owl:NamedIndividual>
    


    <!-- http://vocab.getty.edu/aat/300417204 -->


    <owl:NamedIndividual rdf:about="http://vocab.getty.edu/aat/300417204">
        <rdf:type rdf:resource="http://vocab.getty.edu/aat/Concept"/>
        <dc:identifier>300417204</dc:identifier>
        <rdfs:comment xml:lang="en">Titles or names that were originally assigned to a work or assigned soon after its creation. It may refer to a former title or to a title that has been translated.</rdfs:comment>
        <rdfs:isDefinedBy rdf:resource="http://vocab.getty.edu/aat/"/>
        <rdfs:label xml:lang="en">original titles</rdfs:label>
        <skos:inScheme rdf:resource="http://vocab.getty.edu/aat/"/>
    </owl:NamedIndividual>
    


    <!-- http://vocab.getty.edu/aat/300417207 -->


    <owl:NamedIndividual rdf:about="http://vocab.getty.edu/aat/300417207">
        <rdf:type rdf:resource="http://vocab.getty.edu/aat/Concept"/>
        <dc:identifier>300417207</dc:identifier>
        <rdfs:comment xml:lang="en">For art cataloging, titles or names by which the work has been known in exhibitions, particularly when different from titles by which the work is normally known.</rdfs:comment>
        <rdfs:isDefinedBy rdf:resource="http://vocab.getty.edu/aat/"/>
        <rdfs:label xml:lang="en">exhibition titles (work titles)</rdfs:label>
        <skos:inScheme rdf:resource="http://vocab.getty.edu/aat/"/>
    </owl:NamedIndividual>
    


    <!-- http://vocab.getty.edu/aat/300417260 -->


    <owl:NamedIndividual rdf:about="http://vocab.getty.edu/aat/300417260">
        <rdf:type rdf:resource="http://vocab.getty.edu/aat/Concept"/>
        <dc:identifier>300417260</dc:identifier>
        <rdfs:comment xml:lang="en">The process or function of copying material or data to a computer drive, the cloud, or otherwise to a safe, more permanent location.</rdfs:comment>
        <rdfs:isDefinedBy rdf:resource="http://vocab.getty.edu/aat/"/>
        <rdfs:label xml:lang="en">saving (information handling)</rdfs:label>
        <skos:inScheme rdf:resource="http://vocab.getty.edu/aat/"/>
    </owl:NamedIndividual>
    


    <!-- http://vocab.getty.edu/aat/300417639 -->


    <owl:NamedIndividual rdf:about="http://vocab.getty.edu/aat/300417639">
        <rdf:type rdf:resource="http://vocab.getty.edu/aat/Concept"/>
        <dc:identifier>300417639</dc:identifier>
        <rdfs:comment xml:lang="en">Method of acquiring property by request from the creator or producer.</rdfs:comment>
        <rdfs:isDefinedBy rdf:resource="http://vocab.getty.edu/aat/"/>
        <rdfs:label xml:lang="en">commission (method of acquisition)</rdfs:label>
        <skos:inScheme rdf:resource="http://vocab.getty.edu/aat/"/>
    </owl:NamedIndividual>
    


    <!-- http://vocab.getty.edu/aat/300420536 -->


    <owl:NamedIndividual rdf:about="http://vocab.getty.edu/aat/300420536">
        <rdf:type rdf:resource="http://vocab.getty.edu/aat/Concept"/>
        <dc:identifier>300420536</dc:identifier>
        <rdfs:comment xml:lang="en">A category of handheld tools or weapons characterized by a sharp-edged blade attached to a handle, typically made of wood or metal.</rdfs:comment>
        <rdfs:isDefinedBy rdf:resource="http://vocab.getty.edu/aat/"/>
        <rdfs:label xml:lang="en">axe weapons</rdfs:label>
        <skos:inScheme rdf:resource="http://vocab.getty.edu/aat/"/>
    </owl:NamedIndividual>
    


    <!-- http://vocab.getty.edu/aat/300422994 -->


    <owl:NamedIndividual rdf:about="http://vocab.getty.edu/aat/300422994">
        <rdf:type rdf:resource="http://vocab.getty.edu/aat/Concept"/>
        <dc:identifier>300422994</dc:identifier>
        <rdfs:comment xml:lang="en">A small decorative item, often made of metal or other materials, that is attached to a necklace or bracelet.</rdfs:comment>
        <rdfs:isDefinedBy rdf:resource="http://vocab.getty.edu/aat/"/>
        <rdfs:label xml:lang="en">charm pendant</rdfs:label>
        <skos:inScheme rdf:resource="http://vocab.getty.edu/aat/"/>
    </owl:NamedIndividual>
    


    <!-- http://vocab.getty.edu/aat/300425064 -->


    <owl:NamedIndividual rdf:about="http://vocab.getty.edu/aat/300425064">
        <rdf:type rdf:resource="http://vocab.getty.edu/aat/Concept"/>
        <dc:identifier>300425064</dc:identifier>
        <rdfs:comment xml:lang="en">Machines for the production of electrical discharge at high voltage.</rdfs:comment>
        <rdfs:isDefinedBy rdf:resource="http://vocab.getty.edu/aat/"/>
        <rdfs:label xml:lang="en">electrostatic generators</rdfs:label>
        <skos:inScheme rdf:resource="http://vocab.getty.edu/aat/"/>
    </owl:NamedIndividual>
    


    <!-- http://vocab.getty.edu/aat/300426696 -->


    <owl:NamedIndividual rdf:about="http://vocab.getty.edu/aat/300426696">
        <rdf:type rdf:resource="http://vocab.getty.edu/aat/Concept"/>
        <dc:identifier>300426696</dc:identifier>
        <rdfs:comment xml:lang="en">Software used to create computer graphics, or edit and otherwise manipulate existing graphics.</rdfs:comment>
        <rdfs:isDefinedBy rdf:resource="http://vocab.getty.edu/aat/"/>
        <rdfs:label xml:lang="en">graphics software</rdfs:label>
        <skos:inScheme rdf:resource="http://vocab.getty.edu/aat/"/>
    </owl:NamedIndividual>
    


    <!-- http://vocab.getty.edu/aat/300428379 -->


    <owl:NamedIndividual rdf:about="http://vocab.getty.edu/aat/300428379">
        <rdf:type rdf:resource="http://vocab.getty.edu/aat/Concept"/>
        <dc:identifier>300428379</dc:identifier>
        <rdfs:comment xml:lang="en">Japanese decorative sword guards, and accessories such as handle decorations and skewers used to keep the sword in its scabbard.</rdfs:comment>
        <rdfs:isDefinedBy rdf:resource="http://vocab.getty.edu/aat/"/>
        <rdfs:label xml:lang="en">tsuba kōzuka kogai sets</rdfs:label>
        <skos:inScheme rdf:resource="http://vocab.getty.edu/aat/"/>
    </owl:NamedIndividual>
    


    <!-- http://vocab.getty.edu/aat/300429747 -->


    <owl:NamedIndividual rdf:about="http://vocab.getty.edu/aat/300429747">
        <rdf:type rdf:resource="http://vocab.getty.edu/aat/Concept"/>
        <dc:identifier>300429747</dc:identifier>
        <rdfs:comment xml:lang="en">A device that captures images or text documents and converts them into digital data that can be processed by a computer. These scanners use optical technology to scan physical documents or images and create digital representations of them.</rdfs:comment>
        <rdfs:isDefinedBy rdf:resource="http://vocab.getty.edu/aat/"/>
        <rdfs:label xml:lang="en">optical scanner</rdfs:label>
        <skos:inScheme rdf:resource="http://vocab.getty.edu/aat/"/>
    </owl:NamedIndividual>
    


    <!-- http://vocab.getty.edu/aat/300433476 -->


    <owl:NamedIndividual rdf:about="http://vocab.getty.edu/aat/300433476">
        <rdf:type rdf:resource="http://vocab.getty.edu/aat/Concept"/>
        <dc:identifier>300433476</dc:identifier>
        <rdfs:comment xml:lang="en">Instruments used to discharge a capacitor, which is a device capable of storing energy within an electrostatic field.</rdfs:comment>
        <rdfs:isDefinedBy rdf:resource="http://vocab.getty.edu/aat/"/>
        <rdfs:label xml:lang="en">spark arresters</rdfs:label>
        <skos:inScheme rdf:resource="http://vocab.getty.edu/aat/"/>
    </owl:NamedIndividual>
    


    <!-- http://vocab.getty.edu/aat/300435434 -->


    <owl:NamedIndividual rdf:about="http://vocab.getty.edu/aat/300435434">
        <rdf:type rdf:resource="http://vocab.getty.edu/aat/Concept"/>
        <dc:identifier>300435434</dc:identifier>
        <rdfs:comment xml:lang="en">A formal statement of the copyright or licensing of a work, and/or any restrictions placed on it.</rdfs:comment>
        <rdfs:isDefinedBy rdf:resource="http://vocab.getty.edu/aat/"/>
        <rdfs:label xml:lang="en">copyright/licensing statement</rdfs:label>
        <skos:inScheme rdf:resource="http://vocab.getty.edu/aat/"/>
    </owl:NamedIndividual>
    


    <!-- http://vocab.getty.edu/aat/300440768 -->


    <owl:NamedIndividual rdf:about="http://vocab.getty.edu/aat/300440768">
        <rdf:type rdf:resource="http://vocab.getty.edu/aat/Concept"/>
        <dc:identifier>300440768</dc:identifier>
        <rdfs:comment xml:lang="en">Systematically arranged collections of pressed plant specimens that have been gathered in situ, then dried and pressed onto sheets of archival paper so that major morphological characteristics are preserved.</rdfs:comment>
        <rdfs:isDefinedBy rdf:resource="http://vocab.getty.edu/aat/"/>
        <rdfs:label xml:lang="en">herbaria (documents)</rdfs:label>
        <skos:inScheme rdf:resource="http://vocab.getty.edu/aat/"/>
    </owl:NamedIndividual>
    


    <!-- http://vocab.getty.edu/aat/300445021 -->


    <owl:NamedIndividual rdf:about="http://vocab.getty.edu/aat/300445021">
        <rdf:type rdf:resource="http://vocab.getty.edu/aat/Concept"/>
        <dc:identifier>300445021</dc:identifier>
        <rdfs:comment xml:lang="en">Numbers used to identify an individual publication within a classification or location in a library.</rdfs:comment>
        <rdfs:isDefinedBy rdf:resource="http://vocab.getty.edu/aat/"/>
        <rdfs:label xml:lang="en">book numbers</rdfs:label>
        <skos:inScheme rdf:resource="http://vocab.getty.edu/aat/"/>
    </owl:NamedIndividual>
</rdf:RDF>



<!-- Generated by the OWL API (version 5.1.18) https://github.com/owlcs/owlapi/ -->


