@prefix : <https://w3id.org/dharc/ontology/chad-ap#> .
@prefix owl: <http://www.w3.org/2002/07/owl#> .
@prefix rdf: <http://www.w3.org/1999/02/22-rdf-syntax-ns#> .
@prefix xml: <http://www.w3.org/XML/1998/namespace> .
@prefix xsd: <http://www.w3.org/2001/XMLSchema#> .
@prefix rdfs: <http://www.w3.org/2000/01/rdf-schema#> .
@base <https://w3id.org/dharc/ontology/chad-ap#> .

<https://w3id.org/dharc/ontology/chad-ap> rdf:type owl:Ontology ;
    owl:versionIRI <https://w3id.org/dharc/ontology/chad-ap/1.0.0> ;
    <http://purl.org/dc/elements/1.1/abstract> "A OWL 2 DL-based metadata application profile for describing cultural heritage digitisation data and processes in a FAIR-compliant and machine-readable format."@en ;
    <http://purl.org/dc/elements/1.1/contributor> "Heibi, Ivan" ,
        "Moretti, Arianna" ;
    <http://purl.org/dc/elements/1.1/creator> "Barzaghi, Sebastian" ,
        "Peroni, Silvio" ;
    <http://purl.org/dc/elements/1.1/date> "2024-04-16"^^xsd:date ;
    <http://purl.org/dc/elements/1.1/description> """

        ## Description

        The Cultural Heritage Acquisition and Digitisation Application Profile (CHAD-AP, https://w3id.org/dharc/ontology/chad-ap) is a CIDOC CRM application profile implemented as an OWL ontology that can be logically split into two separate abstract modules: the _Object Module_ (OM), dedicated to describing the CHOs, and the _Process Module_ (PM), for describing the acquisition and digitisation process.

        Both CHAD-AP and its [documentation](https://w3id.org/dharc/ontology/chad-ap) are living artefacts that have been drafted in the context of the [Project CHANGES](https://sites.google.com/uniroma1.it/changes/) ("Cultural Heritage Active Innovation For Next-Gen Sustainable Society"), an EU-funded project that aims at increasing, at the Italian level, the curation, and management of cultural heritage artefacts in all forms, expanding the involvement of the general public, making more sustainable the exhibition potential, and including crucial social functions (accessibility, inclusiveness, critical thinking, participation, enjoyment, sustainability) into the cultural heritage environment.

        Currently, CHAD-AP is able to describe the following entities:
        * CHOs, described according to the Functional Requirements for Bibliographic Records (FRBR) data model, which uses several descriptive layers for its representation. In particular, CHAD-AP considers: the essence or conceptualisation of the CHO (_Work_); the intellectual content of the CHO (_Expression_); the embodiment of the CHO in terms of its format (_Manifestation_); and the physical exemplar of the CHO (_Item_);
        * Activities, events, agents involved and their roles;
        * Descriptive components, such as labels, types, identifiers and titles;
        * Entities related to curation and conservation, like curation events, places of conservation, agent responsible for its conservation, etc.
        * Concepts and other immaterial objects, such as the subjects illustrated by CHOs and the licenses or right statements assigned to them;
        * Digitization processes used to capture 3D data of CHOs and to output their digital models, and software activities leveraging these DCHOs as input for further processes.

        The current version of the application profile reuses a subset of classes and properties selected from the following models:

        * [CIDOC CRM](http://www.cidoc-crm.org/cidoc-crm/) is an international ISO standard that provides an ontology related to cultural heritage and museum documentation, which can be extended with additional modules for covering particular descriptions at hand;
        * [CRMdig](http://www.ics.forth.gr/isl/CRMdig/) is an extension of CIDOC CRM for describing metadata related to the digital provenance of digitisation processes and digital representations;
        * [LRMoo](http://iflastandards.info/ns/lrm/lrmoo/) is an ontology for representing bibliographic information according to the LRM data model within the CIDOC CRM framework;
        * [AAT](http://vocab.getty.edu/page/aat/) is a structured vocabulary of terms used to describe art, architecture, decorative arts, and material culture.

        A full version of CHAD-AP is available at [https://w3id.org/dharc/ontology/chad-ap](https://w3id.org/dharc/ontology/chad-ap).

        The next subsections provide a quick overview of all the entities defined, some exemple of usage, and some of the queries that CHAD-AP can answer.

        ### Object Module (OM)
        As shown in the diagram below, a Cultural Heritage Object (CHO) is described in CHAD-AP according to the Functional Requirements for Bibliographic Records (FRBR) data model, which uses several descriptive layers for its representation. 

        ![A diagram of the CHAD-AP Object Module (OM).](diagrams/object-model.png)

        In particular, the _Work_ (`lrmoo:F1_Work`) represents the _essence_ or conceptualization of the CHO. Each work is associated with a series of titles (`crm:E35_Title`), each classified according to a particular type (`crm:E55_Type`), which can be an _original title_ (`aat:300417204`) or an _exhibition title_ (`aat:300417207`). Furthermore, a Work can be part of a larger Work, like a series of printed volumes, which is classified under a particular type (`crm:E55_Type`).

        The _Expression_ (`lrmoo:F2_Expression`) is the realisation of a Work, and refers to the intellectual _content_ of the object. Both the Expression and the Work are generated through a creation event (`lrmoo:F28_Expression_Creation`) occurring within a specific time span (`crm:E52_Time-Span`), which can be expressed as either a precisely defined period with exact starting and ending date times (`crm:P82a_begin_of_the_begin` and `crm:P82b_end_of_the_end`) or a fuzzy label if its temporal extents are not precisely known (`crm:P82_at_some_time_within`). A creation event is made of smaller activities (`crm:E7_Activity`), each conducted by one or more agents (`crm:E39_Actor`) and characterised by a specific type (`crm:E55_Type`) that defines, implicitly, the role assumed by the agent for that activity. For example, if the agent is identified as the author of the Expression, the activity type is represented as _writing_ (`aat:300054698`). Also, creation events employ various creation techniques (`crm:E55_Type`). For example, `aat:300054196` is used to express _drawing technique_. An Expression can also be associated with one or more subjects defining its contents. In CHAD-AP, a generic _concept_ is represented with the class `crm:E73_Information_Object` with the type `aat:300404126` (i.e. _subject_) explicitly specified.

        The _Manifestation_ (`lrmoo:F3_Manifestation`) represents the embodiment of the CHO's content in a physical format. It is characterised by having a type (`crm:E55_Type`). In addition, Manifestations are associated with copyright or licensing statements (represented through the combination of `crm:E73_Information_Object` having type `aat:300435434`, i.e.  _copyright/licensing statement_), linked with the document introducing the actual license or right statements through the property `crm:P70i_is_documented_in`.

        Finally, the _Item_ (`lrmoo:F5_Item`) represents the physical, localised exemplar of the CHO. It is accompanied with descriptive components like labels (expressed through the use of the property `crm:P3_has_note`) and identifiers (`crm:E42_Identifier`, each with its own content and type). Items can depict the content (`lrmoo:F2_Expression`) of another CHO. Sometimes, an Item may be linked to a curation activity (represented through the combination of `crm:E7_Activity` with type `aat:300054277`, i.e. _curating_) carried out by a keeper (`crm:E39_Actor`) who manages a collection (`crm:E24_Physical_Human-Made_Thing` with type `aat:300025976`, i.e. _collections_) to which the object belongs, located in a specific place (`crm:E53_Place`). An Item can also be composed of (`crm:P46_is_composed_of`) other Items.

        Whenever possible, instances of `crm:E39_Actor` and `crm:E53_Place` are also linked with existing authority records through the property `crm:P1_is_identified_by`.

        ### Process Module (PM)
        As shown in the diagram below, CHAD-AP also describes the entities for defining a 3D digitisation workflow as a sequence of activities classified according to two main categories. 

        ![A diagram of the CHAD-AP Process Module (PM).](diagrams/process-model.png)

        On the one hand, we have the _acquisition activity_ (`crmdig:D2_Digitization_Process`), which involves the digitisation of a CHO (`crm:E24_Physical_Human-Made_Thing`) to produce a Digital CHO (DCHO) (`crmdig:D9_Data_Object`). Similarly to its physical counterpart, the DCHO can be associated with copyright statements or licenses (`crm:E73_Information_Object` with `aat:300435434` as its type). The acquisition occurs within a time span (`crm:E52_Time-Span`) with defined starting and ending date times, and engages various agents, including individuals (`crm:E21_Person`) and institutions (`crm:E74_Group`) responsible for the activity. During the acquisition, a series of techniques (`crm:E55_Type`) can be used, such as _photogrammetry_ (`aat:300053580`) or _structured light scanning_ (`aat:300391312`), along with tools (`crmdig:D8_Digital_Device`) like _digital cameras_ (`aat:300266792`) and _structured light scanners_ (`aat:300429747`).

        On the other hand, we have a series of _software activities_ (`crmdig:D10_Software_Execution`), each representing a specific stage or phase of digitisation workflow. Such stage is denoted by its type (`crm:E55_Type`), such as _processing_ (`aat:300054636`), _modelling_ (`aat:300391447`), and _optimization_ (`aat:300386427`). It involves the manipulation of the DCHO (`crmdig:D9_Data_Object`) produced previously as input and the production of a modified version of that DCHO (`crmdig:D9_Data_Object`) as output. The activity also occurs within a defined time span (`crm:E52_Time-Span`) with precise start and end date times, engages various agents, including individuals (`crm:E21_Person`) and institutions (`crm:E74_Group`), and uses software as tools to produce its output (`crmdig:D14_Software`).

        ## Examples of use
        CHAD-AP can be used for modelling  scenarios related to cultural heritage acquisition and digitisation processes. In the following subsections we introduce some of them, and we accompany them with exemplar instantiations. 

        The prefixes that are used in all the examples provided below are defined as follows:

            @prefix aat: <http://vocab.getty.edu/page/aat/> .
            @prefix ex: <https://w3id.org/dharc/ontology/chad-ap/data/example/> .
            @prefix crm: <http://www.cidoc-crm.org/cidoc-crm/> .
            @prefix crmdig: <http://www.ics.forth.gr/isl/CRMdig/> .
            @prefix lrmoo: <http://iflastandards.info/ns/lrm/lrmoo/> .
            @prefix owl: <http://www.w3.org/2002/07/owl#> .
            @prefix rdf: <http://www.w3.org/1999/02/22-rdf-syntax-ns#> .
            @prefix xml: <http://www.w3.org/XML/1998/namespace> .
            @prefix xsd: <http://www.w3.org/2001/XMLSchema#> .
            @prefix rdfs: <http://www.w3.org/2000/01/rdf-schema#> .

        ### Scenario 
        The creation event `32-expression-creation` created the work `32-work` and its expression `32-expression` within a time span ranging from 1500 to 1599. The creation event is carried out through the `drawing` technique and consists of an activity `32-expression-creation-01`, carried out by `ulisse-aldrovandi` (ULAN:`500342675`) as a creator of the work.

        `32-work` has two titles: `32-work-title-01` with type `original-title` ("Essere umano ermafrodita"), and `32-work-title-02` with type `exhibition-title` ("Essere umano ermafrodita" and "Human hermaphrodite"). It is member of another work `tavole-di-animali-work`, whose manifestation has `print-volume` as its type. It is realised in `32-expression`.

        `32-expression` is about the concept `ermafrodita`. It is embodied in the manifestation `L1-manifestation`.

        `32-manifestation` has `manuscript` as its type. It is referred to by a license statement `32-manifestation-license` documented in the external document "http://rightsstatements.org/vocab/InC/1.0/". It is exemplified by `32-item`.

        `32-item` is identified by three identifiers: `32-item-identifier-01` ("32") with type `collection-id`; `32-item-identifier-02` ("5") with type `volume-number`; and `32-item-identifier-03` ("Ms. Aldrovandi, Tavole di animali, vol. 5, carta 86") with type `shelf-mark`. The item is used in a curation activity `32-item-curation` carried out by `bub`. Its description reads: "Essere umano ermafrodita Human hermaphrodite (Monstrum humanum hermaphroditicum) sec. XVI 16th century BUB, Ms. Aldrovandi, Tavole di animali, vol. 5, carta 86".

        ```
        ex:32-expression-creation a lrmoo:F28_Expression_Creation ;
            crm:P9_consists_of ex:32-expression-creation-activity-01 ;
            crm:P32_used_general_technique aat:300054196 ;
            lrmoo:R19_created_a_realisation_of ex:32-work ;
            lrmoo:R17_created ex:32-expression ;
            crm:P4_has_time-span ex:1500-1599 .

        ex:32-expression-creation-activity-01 a crm:E7_Activity ;
            crm:P2_has_type aat:300404387 ;
            crm:P14_carried_out_by ex:ulisse-aldrovandi .

        ex:ulisse-aldrovandi a crm:E39_Actor ;
            crm:P70i_is_documented_in <http://vocab.getty.edu/page/ulan/500342675> .

        ex:1500-1599 a crm:E52_Time-Span ;
            crm:P82a_begin_of_the_begin "1500-01-01T00:00:00Z"^^xsd:dateTime ;
            crm:P82b_end_of_the_end "1599-12-31T23:59:59Z"^^xsd:dateTime .

        ex:32-work a lrmoo:F1_Work ;
            crm:P102_has_title ex:32-work-title-01 ,
                ex:32-work-title-02 ;
            lrmoo:R3_is_realised_in ex:32-expression .

        ex:32-work-title-01 a crm:E35_Title ;
            crm:P2_has_type aat:300417204 ;
            crm:P190_has_symbolic_content "Essere umano ermafrodita"@it .

        ex:32-work-title-02 a crm:E35_Title ;
            crm:P2_has_type aat:300417207 ;
            crm:P190_has_symbolic_content "Essere umano ermafrodita"@it ,
                "Human hermaphrodite"@en .
                        
        ex:32-expression a lrmoo:F2_Expression ;
            crm:P129_is_about ex:ermafrodita ;
            lrmoo:R4i_is_embodied_in ex:32-manifestation .

        ex:32-manifestation a lrmoo:F3_Manifestation ;
            crm:P2_has_type aat:300028569 ;
            lrmoo:R7i_is_exemplified_by ex:32-item .

        ex:32-manifestation-license a crm:E73_Information_Object ;
            crm:P2_has_type aat:300435434 ;
            crm:P67_refers_to ex:32-manifestation ;
            crm:P70i_is_documented_in <http://rightsstatements.org/vocab/InC/1.0/> .

        ex:tavole-di-animali-work a lrmoo:F1_Work ;
            lrmoo:R10_has_member ex:32-work ;
            lrmoo:R3_is_realised_in ex:tavole-di-animali-expression .

        ex:tavole-di-animali-expression a lrmoo:F2_Expression ;
            lrmoo:R4i_is_embodied_in ex:tavole-di-animali-manifestation .

        ex:tavole-di-animali-manifestation a lrmoo:F3_Manifestation ;
            crm:P2_has_type aat:300265632 ;
            lrmoo:R7i_is_exemplified_by ex:tavole-di-animali-item .

        ex:tavole-di-animali-item a lrmoo:F5_Item .

        ex:ermafrodita a crm:E73_Information_Object ;
            crm:P2_has_type aat:300404126 .

        ex:32-item a lrmoo:F5_Item ;
            crm:P1_is_identified_by ex:32-item-identifier-01 ,
                ex:32-item-identifier-02 ,
                ex:32-item-identifier-03 ;
            crm:P3_has_note '''
                Essere umano ermafrodita 
                Human hermaphrodite (Monstrum humanum hermaphroditicum) 
                sec. XVI 
                16th century 
                BUB, 
                Ms. Aldrovandi, Tavole di animali, vol. 5, carta 86
            '''^^rdfs:Literal .

        ex:32-item-identifier-01 a crm:E42_Identifier ;
            crm:P2_has_type aat:300312355 ;
            crm:P190_has_symbolic_content "32"^^rdfs:Literal .

        ex:32-item-identifier-02 a crm:E42_Identifier ;
            crm:P2_has_type aat:300445021 ;
            crm:P190_has_symbolic_content "5"^^rdfs:Literal .

        ex:32-item-identifier-03 a crm:E42_Identifier ;
            crm:P2_has_type aat:300404704 ;
            crm:P190_has_symbolic_content "Ms. Aldrovandi, Tavole di animali, vol. 5, carta 86"^^rdfs:Literal .

        ex:32-item-curation a crm:E7_Activity ;
            crm:P2_has_type aat:300054277 ;
            crm:P16_used_specific_object ex:32-item ;
            crm:P14_carried_out_by ex:bub .

        ex:bub a crm:E39_Actor .
        ```

        On `2023-05-08`, `alice-bordignon` acquired digital data of `32-item` on behalf of `unibo-ficlit`, leveraging `photogrammetry` and using the `panasonic-dmc-lx100` camera, resulting in a digital model `32-model-00`.

        Subsequently, on `2023-05-10`, Alice processed `32-model-00` on behalf of `unibo-ficlit` using the `3df-zephyr` software, creating a processed digital model `32-model-01`.

        From `2023-05-17` to `2023-05-18`, Alice further modeled `32-model-01` on behalf of `unibo-ficlit` using the `blender` software, resulting in a refined digital model `32-model-02`.

        From `2023-05-18` to `2023-05-19`, Alice optimized `32-model-02` on behalf of `unibo-ficlit` using the `instantmeshes` and `3df-zephyr` software, resulting in an optimized digital model `32-model-03`.

        Finally, on `2023-05-19`, Alice exported `32-model-03` on behalf of `unibo-ficlit` using the `blender` software, resulting in the final exported model `32-model-04` as an output.

        Each digital model is licensed under a CC BY-NC 4.0 license.

        ```
        ex:unibo-ficlit a crm:E74_Group .

        ex:panasonic-dmc-lx100 a crmdig:D8_Digital_Device ;
            crm:P2_has_type aat:300266792 .

        ex:32-acquisition a crmdig:D2_Digitization_Process ;
            crmdig:L1_digitized ex:32-item ;
            crmdig:L11_had_output ex:32-model-00 ;
            crm:P4_has_time-span ex:32-acquisition-timespan ;
            crm:P11_had_participant ex:unibo-ficlit ;
            crm:P14_carried_out_by ex:alice-bordignon ;
            crm:P32_used_general_technique aat:300391312 ;
            crm:P16_used_specific_object ex:panasonic-dmc-lx100 .

        ex:3df-zephyr a crmdig:D14_Software ;
            crm:P2_has_type aat:300426696 .

        ex:32-processing a crmdig:D10_Software_Execution ;
            crm:P2_has_type aat:300054636 ;
            crmdig:L10_had_input ex:32-model-00 ;
            crmdig:L11_had_output ex:32-model-01 ;
            crm:P4_has_time-span ex:32-processing-timespan ;
            crm:P11_had_participant ex:unibo-ficlit ;
            crm:P14_carried_out_by ex:alice-bordignon ;
            crmdig:L23_used_software_or_firmware ex:3df-zephyr .

        ex:blender a crmdig:D14_Software ;
            crm:P2_has_type aat:300426696 .

        ex:32-modeling a crmdig:D10_Software_Execution ;
            crm:P2_has_type aat:300391447 ;
            crmdig:L10_had_input ex:32-model-01 ;
            crmdig:L11_had_output ex:32-model-02 ;
            crm:P4_has_time-span ex:32-modeling-timespan ;
            crm:P11_had_participant ex:unibo-ficlit ;
            crm:P14_carried_out_by ex:alice-bordignon ;
            crmdig:L23_used_software_or_firmware ex:blender .

        ex:instantmeshes a crmdig:D14_Software ;
            crm:P2_has_type aat:300426696 .

        ex:32-optimisation a crmdig:D10_Software_Execution ;
            crm:P2_has_type aat:300386427 ;
            crmdig:L10_had_input ex:32-model-02 ;
            crmdig:L11_had_output ex:32-model-03 ;
            crm:P4_has_time-span ex:32-optimisation-timespan ;
            crm:P11_had_participant ex:unibo-ficlit ;
            crm:P14_carried_out_by ex:alice-bordignon ;
            crmdig:L23_used_software_or_firmware ex:instantmeshes, ex:3df-zephyr .

        ex:32-export a crmdig:D10_Software_Execution ;
            crm:P2_has_type aat:300417260 ;
            crmdig:L10_had_input ex:32-model-03 ;
            crmdig:L11_had_output ex:32-model-04 ;
            crm:P4_has_time-span ex:32-export-timespan ;
            crm:P11_had_participant ex:unibo-ficlit ;
            crm:P14_carried_out_by ex:alice-bordignon ;
            crmdig:L23_used_software_or_firmware ex:blender .

        ex:32-model-00 a crmdig:D9_Data_Object .

        ex:32-model-01 a crmdig:D9_Data_Object .

        ex:32-model-02 a crmdig:D9_Data_Object .

        ex:32-model-03 a crmdig:D9_Data_Object .

        ex:32-model-04 a crmdig:D9_Data_Object .

        ex:32-model-00-license a crm:E73_Information_Object ;
            crm:P2_has_type aat:300435434 ;
            crm:P67_refers_to ex:32-model-00 ;
            crm:P70i_is_documented_in <https://creativecommons.org/licenses/by-nc/4.0/> .

        ex:32-model-01-license a crm:E73_Information_Object ;
            crm:P2_has_type aat:300435434 ;
            crm:P67_refers_to ex:32-model-01 ;
            crm:P70i_is_documented_in <https://creativecommons.org/licenses/by-nc/4.0/> .

        ex:32-model-02-license a crm:E73_Information_Object ;
            crm:P2_has_type aat:300435434 ;
            crm:P67_refers_to ex:32-model-02 ;
            crm:P70i_is_documented_in <https://creativecommons.org/licenses/by-nc/4.0/> .

        ex:32-model-03-license a crm:E73_Information_Object ;
            crm:P2_has_type aat:300435434 ;
            crm:P67_refers_to ex:32-model-03 ;
            crm:P70i_is_documented_in <https://creativecommons.org/licenses/by-nc/4.0/> .

        ex:32-model-04-license a crm:E73_Information_Object ;
            crm:P2_has_type aat:300435434 ;
            crm:P67_refers_to ex:32-model-04 ;
            crm:P70i_is_documented_in <https://creativecommons.org/licenses/by-nc/4.0/> .

        ex:32-acquisition-timespan a crm:E52_Time-Span ;
            crm:P82a_begin_of_the_begin "2023-05-08T00:00:00Z"^^xsd:dateTime ;
            crm:P82b_end_of_the_end "2023-05-08T23:59:59Z"^^xsd:dateTime .

        ex:32-processing-timespan a crm:E52_Time-Span ;
            crm:P82a_begin_of_the_begin "2023-05-10T00:00:00Z"^^xsd:dateTime ;
            crm:P82b_end_of_the_end "2023-05-10T23:59:59Z"^^xsd:dateTime .

        ex:32-modeling-timespan a crm:E52_Time-Span ;
            crm:P82a_begin_of_the_begin "2023-05-17T00:00:00Z"^^xsd:dateTime ;
            crm:P82b_end_of_the_end "2023-05-18T23:59:59Z"^^xsd:dateTime .

        ex:32-optimisation-timespan a crm:E52_Time-Span ;
            crm:P82a_begin_of_the_begin "2023-05-18T00:00:00Z"^^xsd:dateTime ;
            crm:P82b_end_of_the_end "2023-05-19T23:59:59Z"^^xsd:dateTime .

        ex:32-export-timespan a crm:E52_Time-Span ;
            crm:P82a_begin_of_the_begin "2023-05-19T00:00:00Z"^^xsd:dateTime ;
            crm:P82b_end_of_the_end "2023-05-19T23:59:59Z"^^xsd:dateTime .
        ```

        ### Competency questions
        CHAD-AP can be used for answering several questions related to the acquisition and digitisation of cultural heritage objects. In the following subsections we introduce some of them, and we accompany them with exemplar SPARQL queries. 

        The prefixes that are used in all the SPARQL queries provided below are defined as follows:

            PREFIX aat: <http://vocab.getty.edu/page/aat/>
            PREFIX crm: <http://www.cidoc-crm.org/cidoc-crm/>
            PREFIX crmdig: <http://www.ics.forth.gr/isl/CRMdig/>
            PREFIX ex: <https://w3id.org/dharc/ontology/chad-ap/data/example/>
            PREFIX lrmoo: <http://iflastandards.info/ns/fr/frbr/lrmoo/>  

        #### Question 1
        What are the CHOs whose creation involved some author?

            SELECT ?resource ?agent
            WHERE {
                ?creation_event a lrmoo:F28_Expression_Creation ;
                    lrmoo:R17_created ?resource ;
                    crm:P9_consists_of ?activity .
                ?activity crm:P2_has_type aat:300054698 ;
                    crm:P14_carried_out_by ?agent .
            }

        #### Question 2
        What are the agents and the types of  activities they carried out to contribute to the creation of `32-expression`?

            SELECT ?agent ?type
            WHERE {
                ?creation_event a lrmoo:F28_Expression_Creation ;
                    lrmoo:R17_created ex:32-expression ;
                    crm:P9_consists_of ?activity .
                ?activity crm:P2_has_type ?type ;
                    crm:P14_carried_out_by ?agent .
            }

        #### Question 3
        What are the agents involved in the creation of the CHOs that have been created through the drawing technique? What are the types of the activities they carried out?

            SELECT ?resource ?agent ?type
            WHERE {
                ?creation_event a lrmoo:F28_Expression_Creation ;
                    crm:P32_used_general_technique aat:300054196 ;
                    lrmoo:R17_created ?resource ;
                    crm:P9_consists_of ?activity .
                ?activity crm:P2_has_type ?type ;
                    crm:P14_carried_out_by ?agent .
            }

        #### Question 4
        What are the identifiers of a manuscript? What are their types?

            SELECT ?resource ?identifier_text ?type
            WHERE {
                ?resource a lrmoo:F5_Item ;
                    crm:P2_has_type aat:300028569 ;
                    crm:P1_is_identified_by ?identifier .
                ?identifier crm:P2_has_type ?type ;
                    crm:P190_has_symbolic_content ?identifier_text.
            }

        #### Question 5
        What is the shelf mark of the CHO with the project ID '32'?

            SELECT ?identifier_text
            WHERE {
                ?resource a lrmoo:F5_Item ;
                crm:P1_is_identified_by ?identifier1 ,
                    ?identifier2 .
                ?identifier1 crm:P2_has_type aat:300312355 ;
                    crm:P190_has_symbolic_content "32"^^rdfs:Literal .
                ?identifier2 crm:P2_has_type aat:300404704 ;
                    crm:P190_has_symbolic_content ?identifier_text.
            }

        #### Question 6
        What are the descriptive labels of the CHOs that either have shelf marks or are prints?

            SELECT ?resource ?label
            WHERE {
                ?manifestation a lrmoo:F3_Manifestation ;
                    lrmoo:R7i_is_exemplified_by ?resource ;
                    crm:P2_has_type ?type .
                ?resource a lrmoo:F5_Item ;
                    crm:P1_is_identified_by ?identifier ;
                    crm:P3_has_note ?label .
                ?identifier crm:P2_has_type ?id_type .
                FILTER(?type = aat:300041273 || ?id_type = aat:300404704)
            }

        #### Question 7
        What are the CHOs whose collections have been curated by agents located in Bologna?

            SELECT ?resource ?agent
            WHERE {
                ?curation a crm:E7_Activity ;
                    crm:P2_has_type aat:300054277 ;
                    crm:P14_carried_out_by ?agent ;
                    crm:P16_used_specific_object ?resource .
                ?agent crm:P74_has_current_or_former_residence ex:bologna .
            }

        #### Question 8
        What are the CHOs and the time spans of their creation events?

            SELECT ?resource ?time_interval
            WHERE {
                ?creation_event a lrmoo:F28_Expression_Creation ;
                    lrmoo:R19_created_a_realisation_of ?resource ;
                    crm:P4_has_time-span ?time_interval .
            }
            
        #### Question 9
        What are the titles of the work `32-work`? What are their types?
            
            SELECT ?title ?type ?content
            WHERE {
                ?creation a lrmoo:F28_Expression_Creation ;
                    lrmoo:R19_created_a_realisation_of ex:32-work .
                ex:32-work crm:P102_has_title ?title .
                ?title crm:P2_has_type ?type ;
                    crm:P190_has_symbolic_content ?content .
            }

        #### Question 10
        What are the parent works of the works that have 'ermafrodita' as their subject?
            
            SELECT ?parent ?work ?subject
            WHERE {
                ?creation a lrmoo:F28_Expression_Creation ;
                    lrmoo:R19_created_a_realisation_of ?work ;
                    lrmoo:R17_created ?expression .
                ?parent a lrmoo:F1_Work ;
                    lrmoo:R10_has_member ?work .
                ?expression a lrmoo:F2_Expression ;
                    crm:P129_is_about ex:ermafrodita .
            }

        #### Question 11
        Which license statements are assigned to the manifestations?
            
            SELECT ?manifestation ?license_link
            WHERE {
                ?license crm:P67_refers_to ?manifestation ;
                    crm:P2_has_type aat:300435434 ;
                    crm:P70i_is_documented_in ?license_link .
            }

        #### Question 12
        What is the CHO digitized and the DCHO produced by an acquisition activity? What is the latter's license?
            
            SELECT ?input ?output ?license_link
            WHERE {
                ?activity a crmdig:D2_Digitization_Process ;
                    crmdig:L1_digitized ?input ;
                    crmdig:L11_had_output ?output .
                ?license crm:P2_has_type aat:300435434 ;
                    crm:P67_refers_to ?output ;
                    crm:P70i_is_documented_in ?license_link .
            }

        #### Question 13
        What are the starting and ending date times in which the acquisition activity occurred?

            SELECT ?activity ?start ?end
            WHERE {
                ?activity a crmdig:D2_Digitization_Process;
                    crm:P4_has_time-span ?timespan .
                ?timespan crm:P82a_begin_of_the_begin ?start ;
                    crm:P82b_end_of_the_end ?end .
            }

        #### Question 14
        What are the acquisition activities, its output, the processing activity and its output?

            SELECT ?digitization ?input ?activity ?output
            WHERE {
                ?activity a crmdig:D10_Software_Execution ;
                    crm:P2_has_type aat:300054636 ;
                    crmdig:L10_had_input ?input ;
                    crmdig:L11_had_output ?output .
                ?digitization crmdig:L11_had_output ?input .
            }

        #### Question 15
        What are the people and institutions who either carried out or were participants in the processing activity?

            SELECT ?person ?institution
            WHERE {
                ?activity a crmdig:D10_Software_Execution ;
                    crm:P2_has_type aat:300054636 ;
                    crm:P14_carried_out_by ?person ;
                    crm:P11_had_participant ?institution .
            }

        #### Question 16
        What are the techniques used in acquisition activities?

            SELECT ?technique ?activity
            WHERE {
                ?activity a crmdig:D2_Digitization_Process ;
                    crm:P32_used_general_technique ?technique .
            }

        #### Question 17
        What are the tools and their types used in processing activities?

            SELECT ?tool ?type
            WHERE {
                ?activity a crmdig:D10_Software_Execution ;
                    crm:P2_has_type aat:300054636 ;
                    crmdig:L23_used_software_or_firmware ?tool .
                ?tool a crmdig:D14_Software ;
                    crm:P2_has_type ?type .
            }

        """@en ;
    <http://purl.org/dc/terms/bibliographicCitation> "Barzaghi, S. and Peroni, S. (2024). Cultural Heritage Acquisition and Digitisation Application Profile. https://w3id.org/dharc/ontology/chad-ap."@en ;
    <http://purl.org/dc/terms/created> "2024-04-16"^^xsd:date ;
    <http://purl.org/dc/terms/issued> "2024-04-16"^^xsd:date ;
    <http://purl.org/dc/terms/modified> "2024-06-01"^^xsd:date ;
    <http://purl.org/dc/terms/license> "http://creativecommons.org/licenses/by/4.0/"@en ;
    <http://purl.org/dc/terms/title> "Cultural Heritage Acquisition and Digitisation Application Profile (CHAD-AP)"@en ;
    <http://purl.org/vocab/vann/preferredNamespacePrefix> "chad-ap"@en ;
    <http://purl.org/vocab/vann/preferredNamespaceUri> "https://w3id.org/dharc/ontology/chad-ap"@en ;
    rdfs:comment "The Cultural Heritage Acquisition and Digitisation Application Profile (CHAD-AP, https://w3id.org/dharc/ontology/chad-ap) is a CIDOC CRM application profile implemented as an OWL ontology that can be logically split into two separate abstract modules: the Object Module (OM), dedicated to describing the CH objects, and the Process Module (PM), for describing the acquisition and digitisation process."@en ;
    owl:versionInfo "2.0.0" ;
    <http://www.w3.org/2003/06/sw-vocab-status/ns#status> "work in progress"@en .

#################################################################
#    Annotation properties
#################################################################

###  http://purl.org/dc/elements/1.1/abstract
<http://purl.org/dc/elements/1.1/abstract> rdf:type owl:AnnotationProperty .


###  http://purl.org/dc/elements/1.1/contributor
<http://purl.org/dc/elements/1.1/contributor> rdf:type owl:AnnotationProperty .


###  http://purl.org/dc/elements/1.1/creator
<http://purl.org/dc/elements/1.1/creator> rdf:type owl:AnnotationProperty .


###  http://purl.org/dc/elements/1.1/date
<http://purl.org/dc/elements/1.1/date> rdf:type owl:AnnotationProperty .


###  http://purl.org/dc/elements/1.1/description
<http://purl.org/dc/elements/1.1/description> rdf:type owl:AnnotationProperty .


###  http://purl.org/dc/elements/1.1/identifier
<http://purl.org/dc/elements/1.1/identifier> rdf:type owl:AnnotationProperty .


###  http://purl.org/dc/terms/bibliographicCitation
<http://purl.org/dc/terms/bibliographicCitation> rdf:type owl:AnnotationProperty .


###  http://purl.org/dc/terms/created
<http://purl.org/dc/terms/created> rdf:type owl:AnnotationProperty .


###  http://purl.org/dc/terms/issued
<http://purl.org/dc/terms/issued> rdf:type owl:AnnotationProperty .


###  http://purl.org/dc/terms/license
<http://purl.org/dc/terms/license> rdf:type owl:AnnotationProperty .


###  http://purl.org/dc/terms/title
<http://purl.org/dc/terms/title> rdf:type owl:AnnotationProperty .


###  http://purl.org/vocab/vann/preferredNamespacePrefix
<http://purl.org/vocab/vann/preferredNamespacePrefix> rdf:type owl:AnnotationProperty .


###  http://purl.org/vocab/vann/preferredNamespaceUri
<http://purl.org/vocab/vann/preferredNamespaceUri> rdf:type owl:AnnotationProperty .


###  http://www.w3.org/2003/06/sw-vocab-status/ns#status
<http://www.w3.org/2003/06/sw-vocab-status/ns#status> rdf:type owl:AnnotationProperty .


###  http://www.w3.org/2004/02/skos/core#inScheme
<http://www.w3.org/2004/02/skos/core#inScheme> rdf:type owl:AnnotationProperty .


#################################################################
#    Datatypes
#################################################################

###  http://www.w3.org/2001/XMLSchema#date
xsd:date rdf:type rdfs:Datatype .


#################################################################
#    Object Properties
#################################################################

###  http://iflastandards.info/ns/lrm/lrmoo/R10_has_member
<http://iflastandards.info/ns/lrm/lrmoo/R10_has_member> rdf:type owl:ObjectProperty ;
    rdfs:label "has member"@en ;
    rdfs:comment "This property associates a complex work with a work that forms part of it."@en ;
    rdfs:domain lrmoo:F1_Work ;
    rdfs:range crm:E28_Conceptual_Object ;
    owl:inverseOf lrmoo:R10i_is_member_of ;
    <http://purl.org/vocab/vann/example> """

        ### Example of a complex work made up by another work.
        
        :parent-work a lrmoo:F1_Work ;
            lrmoo:R10_has_member :another-work .
        
        :another-work a lrmoo:F1_Work .

    """@en ;
    <http://www.w3.org/2003/06/sw-vocab-status/ns#term_status> <http://purl.org/linked-data/registry#statusStable> ;
    <http://www.linkedmodel.org/schema/vaem#rationale> "This property is used to represent works composed of other works."@en ;
    rdfs:isDefinedBy <http://iflastandards.info/ns/lrm/lrmoo/> .


###  http://iflastandards.info/ns/lrm/lrmoo/R10i_is_member_of
<http://iflastandards.info/ns/lrm/lrmoo/R10i_is_member_of> rdf:type owl:ObjectProperty ;
    rdfs:label "is member of"@en ;
    rdfs:domain crm:E28_Conceptual_Object ;
    rdfs:range lrmoo:F1_Work ;
    owl:inverseOf lrmoo:R10_has_member ;
    rdfs:isDefinedBy <http://iflastandards.info/ns/lrm/lrmoo/> .


lrmoo:R3_is_realised_in 
    a owl:ObjectProperty ;
    rdfs:label "is realised in"@en ;
    rdfs:comment "This property associates an expression with a work."@en ;
    rdfs:domain lrmoo:F1_Work ;
    rdfs:range lrmoo:F2_Expression ;
    owl:inverseOf lrmoo:R3i_realises ;
    <http://purl.org/vocab/vann/example> """

        ### Example of a work realised in an expression.
        
        :work a lrmoo:F1_Work ;
            lrmoo:R3_is_realised_in :expression .
        
        :expression a lrmoo:F2_Expression .

    """@en ;
    <http://www.w3.org/2003/06/sw-vocab-status/ns#term_status> <http://purl.org/linked-data/registry#statusStable> ;
    <http://www.linkedmodel.org/schema/vaem#rationale> "This property is used to model the relation between the Work and the Expression LRM entities."@en ;
    rdfs:isDefinedBy <http://iflastandards.info/ns/lrm/lrmoo/> .

lrmoo:R3i_realises 
    a owl:ObjectProperty ;
    rdfs:label "realises"@en ;
    rdfs:domain lrmoo:F2_Expression ;
    rdfs:range lrmoo:F1_Work ;
    owl:inverseOf lrmoo:R3_is_realised_in ;
    rdfs:isDefinedBy <http://iflastandards.info/ns/lrm/lrmoo/> .

lrmoo:R4_embodies 
    a owl:ObjectProperty ;
    rdfs:label "embodies"@en ;
    rdfs:comment "This property associates a Manifestation with one or more expressions which are rendered by this manifestation."@en ;
    rdfs:domain lrmoo:F3_Manifestation ;
    rdfs:range lrmoo:F2_Expression ;
    owl:inverseOf lrmoo:R4i_is_embodied_in ;
    rdfs:subPropertyOf crm:P165_incorporates ;
    <http://purl.org/vocab/vann/example> """

        ### Example of a Manifestation embodying an Expression.
        
        :manifestation a lrmoo:F3_Manifestation ;
            lrmoo:R4_embodies :expression .
        
        :expression a lrmoo:F2_Expression .

    """@en ;
    <http://www.w3.org/2003/06/sw-vocab-status/ns#term_status> <http://purl.org/linked-data/registry#statusStable> ;
    <http://www.linkedmodel.org/schema/vaem#rationale> "This property is used to model the relation between the Manifestation and the Expression LRM entities."@en ;
    rdfs:isDefinedBy <http://iflastandards.info/ns/lrm/lrmoo/> .

lrmoo:R4i_is_embodied_by 
    a owl:ObjectProperty ;
    rdfs:label "is embodied in"@en ;
    rdfs:domain lrmoo:F2_Expression ;
    rdfs:range lrmoo:F3_Manifestation ;
    owl:inverseOf lrmoo:R4_embodies ;
    rdfs:subPropertyOf crm:P165i_is_incorporated_in ;
    rdfs:isDefinedBy <http://iflastandards.info/ns/lrm/lrmoo/> .

lrmoo:R7_exemplifies
    a owl:ObjectProperty ;
    rdfs:label "exemplifies"@en ;
    rdfs:comment "This property associates a manifestation with an item that is one of its exemplars or its only exemplar."@en ;
    rdfs:domain lrmoo:F5_Item ;
    rdfs:range lrmoo:F3_Manifestation ;
    owl:inverseOf lrmoo:R7i_is_exemplified_by ;
    rdfs:subPropertyOf crm:P128_carries ;
    <http://purl.org/vocab/vann/example> """

        ### Example of a item exemplifying a manifestation.
        
        :item a lrmoo:F5_Item ;
            lrmoo:R7_exemplifies :manifestation .
        
        :manifestation a lrmoo:F3_Manifestation .

    """@en ;
    <http://www.w3.org/2003/06/sw-vocab-status/ns#term_status> <http://purl.org/linked-data/registry#statusStable> ;
    <http://www.linkedmodel.org/schema/vaem#rationale> "This property is used to represent the relation between the Item and Manifestation LRM entities."@en ;
    rdfs:isDefinedBy <http://iflastandards.info/ns/lrm/lrmoo/> .

lrmoo:R7i_is_exemplified_by
    a owl:ObjectProperty ;
    rdfs:label "is exemplified by"@en ;
    rdfs:domain lrmoo:F3_Manifestation ;
    rdfs:range lrmoo:F5_Item ;
    owl:inverseOf lrmoo:R7_exemplifies ;
    rdfs:subPropertyOf crm:P128i_is_carried_by ;
    rdfs:isDefinedBy <http://iflastandards.info/ns/lrm/lrmoo/> .

###  http://iflastandards.info/ns/lrm/lrmoo/R17_created
<http://iflastandards.info/ns/lrm/lrmoo/R17_created> rdf:type owl:ObjectProperty ;
    rdfs:label "created"@en ;
    rdfs:comment "This property associates the expression that was first externalised during a particular creation event with that particular creation event."@en ;
    rdfs:domain lrmoo:F28_Expression_Creation ;
    rdfs:range lrmoo:F2_Expression ;
    owl:inverseOf lrmoo:R17i_was_created_by ;
    rdfs:subPropertyOf crm:P94_has_created ;
    <http://purl.org/vocab/vann/example> """

        ### Example of an expression being created in a creation event.
        
        :expression-creation a lrmoo:F28_Expression_Creation ;
            lrmoo:R17_created :expression .
        
        :expression a lrmoo:F2_Expression .

    """@en ;
    <http://www.w3.org/2003/06/sw-vocab-status/ns#term_status> <http://purl.org/linked-data/registry#statusStable> ;
    <http://www.linkedmodel.org/schema/vaem#rationale> "This property is used to represent the creation of an LRM Expression entity."@en ;
    rdfs:isDefinedBy <http://iflastandards.info/ns/lrm/lrmoo/> .


###  http://iflastandards.info/ns/lrm/lrmoo/R17i_was_created_by
<http://iflastandards.info/ns/lrm/lrmoo/R17i_was_created_by> rdf:type owl:ObjectProperty ;
    rdfs:label "was created by"@en ;
    rdfs:domain lrmoo:F2_Expression ;
    rdfs:range lrmoo:F28_Expression_Creation ;
    owl:inverseOf lrmoo:R17_created ;
    rdfs:subPropertyOf crm:P94i_was_created_by ;
    rdfs:isDefinedBy <http://iflastandards.info/ns/lrm/lrmoo/> .


###  http://iflastandards.info/ns/lrm/lrmoo/R19_created_a_realisation_of
<http://iflastandards.info/ns/lrm/lrmoo/R19_created_a_realisation_of> rdf:type owl:ObjectProperty ;
    rdfs:label "created a realisation of"@en ;
    rdfs:comment "This property associates an expression creation with the corresponding work."@en ;
    rdfs:domain lrmoo:F28_Expression_Creation ;
    rdfs:range lrmoo:F1_Work ;
    owl:inverseOf lrmoo:R19i_was_realised_through ;
    rdfs:subPropertyOf crm:P16_used_specific_object ;
    <http://purl.org/vocab/vann/example> """

        ### Example of a work being created during a creation event.
        
        :expression-creation a lrmoo:F28_Expression_Creation ;
            lrmoo:R19_created_a_realisation_of :work .
        
        :work a lrmoo:F1_Work .

    """@en ;
    <http://www.w3.org/2003/06/sw-vocab-status/ns#term_status> <http://purl.org/linked-data/registry#statusStable> ;
    <http://www.linkedmodel.org/schema/vaem#rationale> "This property is used to represent the creation of an LRM Work entity."@en ;
    rdfs:isDefinedBy <http://iflastandards.info/ns/lrm/lrmoo/> .


###  http://iflastandards.info/ns/lrm/lrmoo/R19i_was_realised_through
<http://iflastandards.info/ns/lrm/lrmoo/R19i_was_realised_through> rdf:type owl:ObjectProperty ;
    rdfs:label "was realised through"@en ;
    rdfs:domain lrmoo:F1_Work ;
    rdfs:range lrmoo:F28_Expression_Creation ;
    owl:inverseOf lrmoo:R19_created_a_realisation_of ;
    rdfs:subPropertyOf crm:P16i_was_used_for ;
    rdfs:isDefinedBy <http://iflastandards.info/ns/lrm/lrmoo/> .


###  http://www.cidoc-crm.org/cidoc-crm/P102_has_title
<http://www.cidoc-crm.org/cidoc-crm/P102_has_title> rdf:type owl:ObjectProperty ;
    rdfs:subPropertyOf <http://www.cidoc-crm.org/cidoc-crm/P1_is_identified_by> ;
    owl:inverseOf <http://www.cidoc-crm.org/cidoc-crm/P102i_is_title_of> ;
    rdfs:domain <http://www.cidoc-crm.org/cidoc-crm/E71_Human-Made_Thing> ;
    rdfs:range <http://www.cidoc-crm.org/cidoc-crm/E35_Title> ;
    rdfs:comment "This property associates a title with the work bearing that title."@en ;
    rdfs:isDefinedBy <http://www.cidoc-crm.org/cidoc-crm/> ;
    <http://purl.org/vocab/vann/example> """

        ### Example of a work bearing a title.
        
        :work a lrmoo:F1_Work ;
            crm:P102_has_title :title .
        
        :title a crm:E35_Title .

    """@en ;
    <http://www.w3.org/2003/06/sw-vocab-status/ns#term_status> <http://purl.org/linked-data/registry#statusStable> ;
    <http://www.linkedmodel.org/schema/vaem#rationale> "This property is used to represent the fact that a CHO at the Work level has a title."@en ;
    rdfs:label "a pour titre"@fr ,
        "has title"@en ,
        "tem título"@pt ,
        "trägt den Titel"@de ,
        "έχει τίτλο"@el ,
        "имеет заголовок"@ru ,
        "有题名"@zh .


###  http://www.cidoc-crm.org/cidoc-crm/P102i_is_title_of
<http://www.cidoc-crm.org/cidoc-crm/P102i_is_title_of> rdf:type owl:ObjectProperty ;
    rdfs:subPropertyOf <http://www.cidoc-crm.org/cidoc-crm/P1i_identifies> ;
    rdfs:domain <http://www.cidoc-crm.org/cidoc-crm/E35_Title> ;
    rdfs:range <http://www.cidoc-crm.org/cidoc-crm/E71_Human-Made_Thing> ;
    rdfs:isDefinedBy <http://www.cidoc-crm.org/cidoc-crm/> ;
    rdfs:label "est le titre de"@fr ,
        "is title of"@en ,
        "ist der Titel von"@de ,
        "é título de"@pt ,
        "είναι τίτλος του/της"@el ,
        "является заголовком для"@ru ,
        "题名是"@zh .


###  http://www.cidoc-crm.org/cidoc-crm/P10_falls_within
<http://www.cidoc-crm.org/cidoc-crm/P10_falls_within> rdf:type owl:ObjectProperty .


###  http://www.cidoc-crm.org/cidoc-crm/P10i_contains
<http://www.cidoc-crm.org/cidoc-crm/P10i_contains> rdf:type owl:ObjectProperty .


###  http://www.cidoc-crm.org/cidoc-crm/P11_had_participant
<http://www.cidoc-crm.org/cidoc-crm/P11_had_participant> rdf:type owl:ObjectProperty ;
    rdfs:subPropertyOf <http://www.cidoc-crm.org/cidoc-crm/P12_occurred_in_the_presence_of> ;
    rdfs:domain <http://www.cidoc-crm.org/cidoc-crm/E5_Event> ;
    rdfs:range <http://www.cidoc-crm.org/cidoc-crm/E39_Actor> ;
    rdfs:comment "This property describes the participation of one or more actors in an event."@en ;
    rdfs:isDefinedBy <http://www.cidoc-crm.org/cidoc-crm/> ;
    <http://purl.org/vocab/vann/example> """

        ### Example of an actor participating in an activity.
        
        :event a crm:E5_Event ;
            crm:P11_had_participant :agent .
        
        :agent a crm:E39_Actor .

    """@en ;
    <http://www.w3.org/2003/06/sw-vocab-status/ns#term_status> <http://purl.org/linked-data/registry#statusStable> ;
    <http://www.linkedmodel.org/schema/vaem#rationale> "This property is used to represent the participation of some person or organization to an activity, such as the creation of a CHO, or its digital acquisition."@en ;
    rdfs:label "a eu pour actant participant"@fr ,
        "had participant"@en ,
        "hatte Teilnehmer"@de ,
        "tem participante"@pt ,
        "είχε συμμέτοχο"@el ,
        "имел участника"@ru ,
        "有参与者"@zh .


###  http://www.cidoc-crm.org/cidoc-crm/P11i_participated_in
<http://www.cidoc-crm.org/cidoc-crm/P11i_participated_in> rdf:type owl:ObjectProperty ;
    rdfs:subPropertyOf <http://www.cidoc-crm.org/cidoc-crm/P12i_was_present_at> ;
    owl:inverseOf <http://www.cidoc-crm.org/cidoc-crm/P11_had_participant> ;
    rdfs:domain <http://www.cidoc-crm.org/cidoc-crm/E39_Actor> ;
    rdfs:range <http://www.cidoc-crm.org/cidoc-crm/E5_Event> ;
    rdfs:isDefinedBy <http://www.cidoc-crm.org/cidoc-crm/> ;
    rdfs:label "a participé à"@fr ,
        "nahm Teil an"@de ,
        "participa em"@pt ,
        "participated in"@en ,
        "συμμετείχε σε"@el ,
        "участвовал в"@ru ,
        "参与"@zh .


###  http://www.cidoc-crm.org/cidoc-crm/P125_used_object_of_type
<http://www.cidoc-crm.org/cidoc-crm/P125_used_object_of_type> rdf:type owl:ObjectProperty .


###  http://www.cidoc-crm.org/cidoc-crm/P129_is_about
<http://www.cidoc-crm.org/cidoc-crm/P129_is_about> rdf:type owl:ObjectProperty ;
    rdfs:subPropertyOf <http://www.cidoc-crm.org/cidoc-crm/P67_refers_to> ;
    rdfs:domain <http://www.cidoc-crm.org/cidoc-crm/E89_Propositional_Object> ;
    rdfs:range <http://www.cidoc-crm.org/cidoc-crm/E1_CRM_Entity> ;
    rdfs:comment "This property documents that an expression has some entity as its topic."@en ;
    rdfs:isDefinedBy <http://www.cidoc-crm.org/cidoc-crm/> ;
    <http://purl.org/vocab/vann/example> """

        ### Example of an expression having a topic.
        
        :expression a lrmoo:F2_Expression ;
            crm:P129_is_about :subject .

    """@en ;
    <http://www.w3.org/2003/06/sw-vocab-status/ns#term_status> <http://purl.org/linked-data/registry#statusStable> ;
    <http://www.linkedmodel.org/schema/vaem#rationale> "This property is used to represent topics of CHOs at their Expression level."@en ;
    rdfs:label "a pour sujet"@fr ,
        "handelt über"@de ,
        "is about"@en ,
        "é sobre"@pt ,
        "έχει ως θέμα"@el ,
        "касается"@ru ,
        "有关"@zh .


###  http://www.cidoc-crm.org/cidoc-crm/P129i_is_subject_of
<http://www.cidoc-crm.org/cidoc-crm/P129i_is_subject_of> rdf:type owl:ObjectProperty ;
    rdfs:subPropertyOf <http://www.cidoc-crm.org/cidoc-crm/P67i_is_referred_to_by> ;
    owl:inverseOf <http://www.cidoc-crm.org/cidoc-crm/P129_is_about> ;
    rdfs:domain <http://www.cidoc-crm.org/cidoc-crm/E1_CRM_Entity> ;
    rdfs:range <http://www.cidoc-crm.org/cidoc-crm/E89_Propositional_Object> ;
    rdfs:isDefinedBy <http://www.cidoc-crm.org/cidoc-crm/> ;
    rdfs:label "est le sujet de"@fr ,
        "is subject of"@en ,
        "wird behandelt in"@de ,
        "é assunto de"@pt ,
        "είναι θέμα του/της"@el ,
        "является предметом для"@ru ,
        "是主题"@zh .


###  http://www.cidoc-crm.org/cidoc-crm/P12_occurred_in_the_presence_of
<http://www.cidoc-crm.org/cidoc-crm/P12_occurred_in_the_presence_of> rdf:type owl:ObjectProperty ;
    rdfs:domain <http://www.cidoc-crm.org/cidoc-crm/E5_Event> ;
    rdfs:range <http://www.cidoc-crm.org/cidoc-crm/E77_Persistent_Item> ;
    rdfs:comment "This property describes the presence of an entity during an event, without implying any specific role."@en ;
    rdfs:isDefinedBy <http://www.cidoc-crm.org/cidoc-crm/> ;
    <http://purl.org/vocab/vann/example> """

        ### Example of a curation activity involving a collection.
        
        :curation-activity a crm:E7_Activity ;
            crm:P12_occurred_in_the_presence_of :collection .
        
        :collection a crm:E24_Physical_Human-Made_Thing .

    """@en ;
    <http://www.w3.org/2003/06/sw-vocab-status/ns#term_status> <http://purl.org/linked-data/registry#statusStable> ;
    <http://www.linkedmodel.org/schema/vaem#rationale> "This property is used to represent the fact that a curation activity involves a collection a CHO is part of."@en ;
    rdfs:label "a eu lieu en présence de"@fr ,
        "fand statt im Beisein von"@de ,
        "occurred in the presence of"@en ,
        "ocorreu na presença de"@pt ,
        "συνέβη παρουσία του/της"@el ,
        "появился в присутствии"@ru ,
        "已出现"@zh .


###  http://www.cidoc-crm.org/cidoc-crm/P12i_was_present_at
<http://www.cidoc-crm.org/cidoc-crm/P12i_was_present_at> rdf:type owl:ObjectProperty ;
    owl:inverseOf <http://www.cidoc-crm.org/cidoc-crm/P12_occurred_in_the_presence_of> ;
    rdfs:domain <http://www.cidoc-crm.org/cidoc-crm/E77_Persistent_Item> ;
    rdfs:range <http://www.cidoc-crm.org/cidoc-crm/E5_Event> ;
    rdfs:isDefinedBy <http://www.cidoc-crm.org/cidoc-crm/> ;
    rdfs:label "a été présent à"@fr ,
        "estava presente no"@pt ,
        "war anwesend bei"@de ,
        "was present at"@en ,
        "ήταν παρών/παρούσα/παρόν σε"@el ,
        "присутствовал при"@ru ,
        "出现在"@zh .


###  http://www.cidoc-crm.org/cidoc-crm/P14_carried_out_by
<http://www.cidoc-crm.org/cidoc-crm/P14_carried_out_by> rdf:type owl:ObjectProperty ;
    rdfs:subPropertyOf <http://www.cidoc-crm.org/cidoc-crm/P11_had_participant> ;
    owl:inverseOf <http://www.cidoc-crm.org/cidoc-crm/P14i_performed> ;
    rdfs:domain <http://www.cidoc-crm.org/cidoc-crm/E7_Activity> ;
    rdfs:range <http://www.cidoc-crm.org/cidoc-crm/E39_Actor> ;
    rdfs:comment "This property describes the active, accountable participation of an actor during an activity."@en ;
    rdfs:isDefinedBy <http://www.cidoc-crm.org/cidoc-crm/> ;
    <http://purl.org/vocab/vann/example> """

        ### Example of a person carrying out an acquisition activity.
        
        :acquisition a crmdig:D2_Digitization_Process ;
            crm:P14_carried_out_by :researcher .
        
        :researcher a crm:E21_Person .

    """@en ;
    <http://www.w3.org/2003/06/sw-vocab-status/ns#term_status> <http://purl.org/linked-data/registry#statusStable> ;
    <http://www.linkedmodel.org/schema/vaem#rationale> "This property is used to represent the direct responsibility of a person carrying out an activity, such as the acquisition of a CHO, its curation, its creation, etc."@en ;
    rdfs:label "a été effectué par"@fr ,
        "carried out by"@en ,
        "realizada por"@pt ,
        "wurde ausgeführt von"@de ,
        "πραγματοποιήθηκε από"@el ,
        "выполнялся"@ru ,
        "执行者是"@zh .


###  http://www.cidoc-crm.org/cidoc-crm/P14i_performed
<http://www.cidoc-crm.org/cidoc-crm/P14i_performed> rdf:type owl:ObjectProperty ;
    rdfs:subPropertyOf <http://www.cidoc-crm.org/cidoc-crm/P11i_participated_in> ;
    rdfs:domain <http://www.cidoc-crm.org/cidoc-crm/E39_Actor> ;
    rdfs:range <http://www.cidoc-crm.org/cidoc-crm/E7_Activity> ;
    rdfs:isDefinedBy <http://www.cidoc-crm.org/cidoc-crm/> ;
    rdfs:label "a effectué"@fr ,
        "executou"@pt ,
        "führte aus"@de ,
        "performed"@en ,
        "πραγματοποίησε"@el ,
        "выполнял"@ru ,
        "执行"@zh .


###  http://www.cidoc-crm.org/cidoc-crm/P15_was_influenced_by
<http://www.cidoc-crm.org/cidoc-crm/P15_was_influenced_by> rdf:type owl:ObjectProperty .


###  http://www.cidoc-crm.org/cidoc-crm/P15i_influenced
<http://www.cidoc-crm.org/cidoc-crm/P15i_influenced> rdf:type owl:ObjectProperty .


###  http://www.cidoc-crm.org/cidoc-crm/P16_used_specific_object
<http://www.cidoc-crm.org/cidoc-crm/P16_used_specific_object> rdf:type owl:ObjectProperty ;
    rdfs:subPropertyOf <http://www.cidoc-crm.org/cidoc-crm/P12_occurred_in_the_presence_of> ,
                        <http://www.cidoc-crm.org/cidoc-crm/P15_was_influenced_by> ;
    owl:inverseOf <http://www.cidoc-crm.org/cidoc-crm/P16i_was_used_for> ;
    rdfs:domain <http://www.cidoc-crm.org/cidoc-crm/E7_Activity> ;
    rdfs:range <http://www.cidoc-crm.org/cidoc-crm/E70_Thing> ;
    rdfs:comment "This property describes the use of a tool for performing an activity."@en ;
    rdfs:isDefinedBy <http://www.cidoc-crm.org/cidoc-crm/> ;
    <http://purl.org/vocab/vann/example> """

        ### Example of a CHO being involved in a curation activity.
        
        :curation-activity a crm:E7_Activity ;
            crm:P16_used_specific_object :item .
        
        :item a lrmoo:F1_Item .

    """@en ;
    <http://www.w3.org/2003/06/sw-vocab-status/ns#term_status> <http://purl.org/linked-data/registry#statusStable> ;
    <http://www.linkedmodel.org/schema/vaem#rationale> "This property is used to represent the fact that a certain tool is used to carry out an activity, such as a LRM Item entity during a curation activity, or a digital scanner during an acquisition activity."@en ;
    rdfs:label "a mobilisé l’objet spécifique"@fr ,
        "benutzte das bestimmte Objekt"@de ,
        "used specific object"@en ,
        "usou objeto específico"@pt ,
        "χρησιμοποίησε αντικείμενο"@el ,
        "использовал особый объект"@ru ,
        "使用特定对象"@zh .


###  http://www.cidoc-crm.org/cidoc-crm/P16i_was_used_for
<http://www.cidoc-crm.org/cidoc-crm/P16i_was_used_for> rdf:type owl:ObjectProperty ;
    rdfs:subPropertyOf <http://www.cidoc-crm.org/cidoc-crm/P12i_was_present_at> ,
        <http://www.cidoc-crm.org/cidoc-crm/P15i_influenced> ;
    rdfs:domain <http://www.cidoc-crm.org/cidoc-crm/E70_Thing> ;
    rdfs:range <http://www.cidoc-crm.org/cidoc-crm/E7_Activity> ;
    rdfs:isDefinedBy <http://www.cidoc-crm.org/cidoc-crm/> ;
    rdfs:label "a été mobilisé pour"@fr ,
        "foi usado por"@pt ,
        "was used for"@en ,
        "wurde benutzt für"@de ,
        "χρησιμοποιήθηκε για"@el ,
        "был использован для"@ru ,
        "用于"@zh .


###  http://www.cidoc-crm.org/cidoc-crm/P1_is_identified_by
<http://www.cidoc-crm.org/cidoc-crm/P1_is_identified_by> rdf:type owl:ObjectProperty .


###  http://www.cidoc-crm.org/cidoc-crm/P1i_identifies
<http://www.cidoc-crm.org/cidoc-crm/P1i_identifies> rdf:type owl:ObjectProperty .


###  http://www.cidoc-crm.org/cidoc-crm/P2_has_type
<http://www.cidoc-crm.org/cidoc-crm/P2_has_type> rdf:type owl:ObjectProperty ;
    rdfs:domain <http://www.cidoc-crm.org/cidoc-crm/E1_CRM_Entity> ;
    rdfs:range <http://www.cidoc-crm.org/cidoc-crm/E55_Type> ;
    rdfs:comment "This property allows typing of an entity through the use of an external knowledge organization system, such as a thesaurus or a controlled vocabulary."@en ;
    rdfs:isDefinedBy <http://www.cidoc-crm.org/cidoc-crm/> ;
    <http://purl.org/vocab/vann/example> """

        ### Example of a title having "original title" (aat:300417204) as its type.
        
        ex:32-work-title-01 a crm:E35_Title ;
            crm:P2_has_type aat:300417204 ;
            crm:P190_has_symbolic_content "Essere umano ermafrodita"@it .

    """@en ;
    <http://www.w3.org/2003/06/sw-vocab-status/ns#term_status> <http://purl.org/linked-data/registry#statusStable> ;
    <http://www.linkedmodel.org/schema/vaem#rationale> "This property is used to represent the type of an entity through a flexible, generalised modelling mechanism. This property turns the burden of typifying entities (and thus managing the related individuals) on any external controlled vocabulary that is compatible with RDF representations, such as the Getty's Art and Architecture Thesaurus (AAT)."@en ;
    rdfs:label "a pour type"@fr ,
        "has type"@en ,
        "hat den Typus"@de ,
        "é do tipo"@pt ,
        "έχει τύπο"@el ,
        "имеет тип"@ru ,
        "有类型"@zh .


###  http://www.cidoc-crm.org/cidoc-crm/P32_used_general_technique
<http://www.cidoc-crm.org/cidoc-crm/P32_used_general_technique> rdf:type owl:ObjectProperty ;
    rdfs:subPropertyOf <http://www.cidoc-crm.org/cidoc-crm/P125_used_object_of_type> ;
    owl:inverseOf <http://www.cidoc-crm.org/cidoc-crm/P32i_was_technique_of> ;
    rdfs:domain <http://www.cidoc-crm.org/cidoc-crm/E7_Activity> ;
    rdfs:range <http://www.cidoc-crm.org/cidoc-crm/E55_Type> ;
    rdfs:comment "This property identifies the technique or method that was employed during an activity."@en ;
    rdfs:isDefinedBy <http://www.cidoc-crm.org/cidoc-crm/> ;
    <http://purl.org/vocab/vann/example> """

        ### Example of an activity (expression creation) employing a "drawing technique" (aat:300054196).
        
        ex:32-expression-creation a lrmoo:F28_Expression_Creation ;
            crm:P32_used_general_technique aat:300054196 .

    """@en ;
    <http://www.w3.org/2003/06/sw-vocab-status/ns#term_status> <http://purl.org/linked-data/registry#statusStable> ;
    <http://www.linkedmodel.org/schema/vaem#rationale> "This property is used to represent the technique employed during an activity, and especially during the creation of CHOs and DCHOs. This property turns the burden of defining techniques (and thus the related individuals) on any external controlled vocabulary that is compatible with RDF representations, such as the Getty's Art and Architecture Thesaurus (AAT)."@en ;    
    rdfs:label "a mobilisé comme technique générale"@fr ,
        "benutzte das allgemeine Verfahren"@de ,
        "used general technique"@en ,
        "usou técnica geral"@pt ,
        "χρησιμοποίησε γενική τεχνική"@el ,
        "использовал общую технику"@ru ,
        "使用通用技术"@zh .


###  http://www.cidoc-crm.org/cidoc-crm/P32i_was_technique_of
<http://www.cidoc-crm.org/cidoc-crm/P32i_was_technique_of> rdf:type owl:ObjectProperty .


###  http://www.cidoc-crm.org/cidoc-crm/P39_measured
<http://www.cidoc-crm.org/cidoc-crm/P39_measured> rdf:type owl:ObjectProperty .


###  http://www.cidoc-crm.org/cidoc-crm/P39i_was_measured_by
<http://www.cidoc-crm.org/cidoc-crm/P39i_was_measured_by> rdf:type owl:ObjectProperty .


###  http://www.cidoc-crm.org/cidoc-crm/P46_is_composed_of
<http://www.cidoc-crm.org/cidoc-crm/P46_is_composed_of> rdf:type owl:ObjectProperty ;
    rdfs:domain <http://www.cidoc-crm.org/cidoc-crm/E18_Physical_Thing> ;
    rdfs:range <http://www.cidoc-crm.org/cidoc-crm/E18_Physical_Thing> ;
    rdfs:comment "This property associates a physical entity with another physical entity that forms part of it."@en ;
    rdfs:isDefinedBy <http://www.cidoc-crm.org/cidoc-crm/> ;
    <http://www.w3.org/2003/06/sw-vocab-status/ns#term_status> <http://purl.org/linked-data/registry#statusStable> ;
    <http://www.linkedmodel.org/schema/vaem#rationale> "This property is used to represent the fact that a CHO at the Item level can be composed of other CHOs at the Item level."@en ;    
    rdfs:label "est composé de"@fr ,
        "is composed of"@en ,
        "ist zusammengesetzt aus"@de ,
        "é composto de"@pt ,
        "αποτελείται από"@el ,
        "составлен из"@ru ,
        "组成成分是"@zh .


###  http://www.cidoc-crm.org/cidoc-crm/P46i_forms_part_of
<http://www.cidoc-crm.org/cidoc-crm/P46i_forms_part_of> rdf:type owl:ObjectProperty ;
    owl:inverseOf <http://www.cidoc-crm.org/cidoc-crm/P46_is_composed_of> ;
    rdfs:domain <http://www.cidoc-crm.org/cidoc-crm/E18_Physical_Thing> ;
    rdfs:range <http://www.cidoc-crm.org/cidoc-crm/E18_Physical_Thing> ;
    rdfs:isDefinedBy <http://www.cidoc-crm.org/cidoc-crm/> ;
    rdfs:label "bildet Teil von"@de ,
        "fait partie de"@fr ,
        "faz parte de"@pt ,
        "forms part of"@en ,
        "αποτελεί μέρος του/της"@el ,
        "формирует часть"@ru ,
        "构成部分"@zh .


###  http://www.cidoc-crm.org/cidoc-crm/P1_is_identified_by
<http://www.cidoc-crm.org/cidoc-crm/P1_is_identified_by> rdf:type owl:ObjectProperty ;
    rdfs:label "is identified by"@en,
        "wird bezeichnet als"@de,
        "αναγνωρίζεται ως"@el,
        "est identifié par"@fr,
        "é identificado por"@pt,
        "идентифицируется посредством"@ru,
        "被标识为"@zh ;
    rdfs:comment "This property describes the naming or identification of any real-world item by a name or any other identifier."@en ;
    <http://purl.org/vocab/vann/example> """

        ### Example of a CHO being identified by three identifiers: an accession number (aat:300312355),
        ### a book number (aat:300445021) and a shelfmark (aat:300404704).
        
        ex:32-item a lrmoo:F5_Item ;
            crm:P1_is_identified_by ex:32-item-identifier-01 ,
                ex:32-item-identifier-02 ,
                ex:32-item-identifier-03 .

        ex:32-item-identifier-01 a crm:E42_Identifier ;
            crm:P2_has_type aat:300312355 ;
            crm:P190_has_symbolic_content "32"^^rdfs:Literal .

        ex:32-item-identifier-02 a crm:E42_Identifier ;
            crm:P2_has_type aat:300445021 ;
            crm:P190_has_symbolic_content "5"^^rdfs:Literal .

        ex:32-item-identifier-03 a crm:E42_Identifier ;
            crm:P2_has_type aat:300404704 ;
            crm:P190_has_symbolic_content "Ms. Aldrovandi, Tavole di animali, vol. 5, carta 86"^^rdfs:Literal .

    """@en ;
    <http://www.w3.org/2003/06/sw-vocab-status/ns#term_status> <http://purl.org/linked-data/registry#statusStable> ;
    <http://www.linkedmodel.org/schema/vaem#rationale> "This property is used to represent the identification of CHOs as a reified relation between the CHO and its identifiers, each characterised by a series of attributes."@en ;        
    rdfs:domain crm:E1_CRM_Entity ;
    rdfs:range crm:E41_Appellation ;
    owl:inverseOf crm:P1i_identifies ;
    rdfs:isDefinedBy <http://www.cidoc-crm.org/cidoc-crm/> .


###  http://www.cidoc-crm.org/cidoc-crm/P1i_identifies
<http://www.cidoc-crm.org/cidoc-crm/P1i_identifies> rdf:type owl:ObjectProperty ;
    rdfs:label "identifies"@en,
        "bezeichnet"@de,
        "είναι αναγνωριστικό"@el,
        "identifie"@fr,
        "identifica"@pt,
        "идентифицирует"@ru,
        "标识"@zh ;
    rdfs:domain crm:E41_Appellation ;
    rdfs:range crm:E1_CRM_Entity ;
    owl:inverseOf crm:P1_is_identified_by ;
    rdfs:isDefinedBy <http://www.cidoc-crm.org/cidoc-crm/> .


###  http://www.cidoc-crm.org/cidoc-crm/P4_has_time-span
<http://www.cidoc-crm.org/cidoc-crm/P4_has_time-span> rdf:type owl:ObjectProperty ;
    owl:inverseOf <http://www.cidoc-crm.org/cidoc-crm/P4i_is_time-span_of> ;
    rdfs:domain <http://www.cidoc-crm.org/cidoc-crm/E2_Temporal_Entity> ;
    rdfs:range <http://www.cidoc-crm.org/cidoc-crm/E52_Time-Span> ;
    rdfs:comment "This property associates a phenomenon with the time span during which that phenomenon was on-going."@en ;
    rdfs:isDefinedBy <http://www.cidoc-crm.org/cidoc-crm/> ;
    <http://purl.org/vocab/vann/example> """

        ### Example of an activity (expression creation) happening in the 16th century (a time span between the 
        ### first day of 1500 and the last day of 1599).
        
        ex:32-expression-creation a lrmoo:F28_Expression_Creation ;
            crm:P4_has_time-span ex:1500-1599 .
        
        ex:1500-1599 a crm:E52_Time-Span ;
            crm:P82a_begin_of_the_begin "1500-01-01T00:00:00Z"^^xsd:dateTime ;
            crm:P82b_end_of_the_end "1599-12-31T23:59:59Z"^^xsd:dateTime .

    """@en ;
    <http://www.w3.org/2003/06/sw-vocab-status/ns#term_status> <http://purl.org/linked-data/registry#statusStable> ;
    <http://www.linkedmodel.org/schema/vaem#rationale> "This property is used to represent the fact that an activity happens within a time span, defined by precise starting and ending date times."@en ;        
    rdfs:label "a pour intervalle temporel"@fr ,
        "has time-span"@en ,
        "hat Zeitspanne"@de ,
        "tem período de tempo"@pt ,
        "βρισκόταν σε εξέλιξη"@el ,
        "имеет временной отрезок"@ru ,
        "发生时段是"@zh .


###  http://www.cidoc-crm.org/cidoc-crm/P4i_is_time-span_of
<http://www.cidoc-crm.org/cidoc-crm/P4i_is_time-span_of> rdf:type owl:ObjectProperty ;
    rdfs:domain <http://www.cidoc-crm.org/cidoc-crm/E52_Time-Span> ;
    rdfs:range <http://www.cidoc-crm.org/cidoc-crm/E2_Temporal_Entity> ;
    rdfs:isDefinedBy <http://www.cidoc-crm.org/cidoc-crm/> ;
    rdfs:label "est l’intervalle temporel de"@fr ,
        "is time-span of"@en ,
        "ist Zeitspanne von"@de ,
        "é o período de tempo de"@pt ,
        "είναι χρονικό διάστημα του/της"@el ,
        "является временным отрезком для"@ru ,
        "是时段"@zh .


###  http://www.cidoc-crm.org/cidoc-crm/P62_depicts
<http://www.cidoc-crm.org/cidoc-crm/P62_depicts> rdf:type owl:ObjectProperty ;
    rdfs:domain <http://www.cidoc-crm.org/cidoc-crm/E24_Physical_Human-Made_Thing> ;
    rdfs:range <http://www.cidoc-crm.org/cidoc-crm/E1_CRM_Entity> ;
    rdfs:comment "This property identifies some entity that is depicted by a physical object."@en ;
    rdfs:isDefinedBy <http://www.cidoc-crm.org/cidoc-crm/> ;
    <http://www.w3.org/2003/06/sw-vocab-status/ns#term_status> <http://purl.org/linked-data/registry#statusStable> ;
    <http://www.linkedmodel.org/schema/vaem#rationale> "This property is used to represent the fact that a CHO at the Item level can depict the content (the Expression) of another CHO."@en ;        
    rdfs:label "bildet ab"@de ,
        "depicts"@en ,
        "illustre"@fr ,
        "retrata"@pt ,
        "απεικονίζει"@el ,
        "описывает"@ru ,
        "描绘了"@zh .


###  http://www.cidoc-crm.org/cidoc-crm/P62i_is_depicted_by
<http://www.cidoc-crm.org/cidoc-crm/P62i_is_depicted_by> rdf:type owl:ObjectProperty ;
    owl:inverseOf <http://www.cidoc-crm.org/cidoc-crm/P62_depicts> ;
    rdfs:domain <http://www.cidoc-crm.org/cidoc-crm/E1_CRM_Entity> ;
    rdfs:range <http://www.cidoc-crm.org/cidoc-crm/E24_Physical_Human-Made_Thing> ;
    rdfs:isDefinedBy <http://www.cidoc-crm.org/cidoc-crm/> ;
    rdfs:label "est illustré par"@fr ,
        "is depicted by"@en ,
        "wird abgebildet durch"@de ,
        "é retratada por"@pt ,
        "απεικονίζεται σε"@el ,
        "описан посредством"@ru ,
        "被描绘"@zh .


###  http://www.cidoc-crm.org/cidoc-crm/P67_refers_to
<http://www.cidoc-crm.org/cidoc-crm/P67_refers_to> rdf:type owl:ObjectProperty ;
    rdfs:domain <http://www.cidoc-crm.org/cidoc-crm/E89_Propositional_Object> ;
    rdfs:range <http://www.cidoc-crm.org/cidoc-crm/E1_CRM_Entity> ;
    rdfs:comment "This property documents that a propositional object refers to some entity."@en ;
    rdfs:isDefinedBy <http://www.cidoc-crm.org/cidoc-crm/> ;
    <http://purl.org/vocab/vann/example> """

        ### Example of a license statement (a crm:E73_Information_Object with type aat:300435434) referring to
        ### a CHO at the Manifestation level.
        
        ex:32-manifestation-license a crm:E73_Information_Object ;
            crm:P2_has_type aat:300435434 ;
            crm:P67_refers_to ex:32-manifestation .

    """@en ;
    <http://www.w3.org/2003/06/sw-vocab-status/ns#term_status> <http://purl.org/linked-data/registry#statusStable> ;
    <http://www.linkedmodel.org/schema/vaem#rationale> "This property is used to represent the relation between a license or copyright statement (modelled as a crm:E73_Information_Object with type aat:300435434) and the CHO it is attached to."@en ;        
    rdfs:label "referencia"@pt ,
        "refers to"@en ,
        "renvoie à"@fr ,
        "verweist auf"@de ,
        "αναφέρεται σε"@el ,
        "ссылается на"@ru ,
        "涉及"@zh .


###  http://www.cidoc-crm.org/cidoc-crm/P67i_is_referred_to_by
<http://www.cidoc-crm.org/cidoc-crm/P67i_is_referred_to_by> rdf:type owl:ObjectProperty ;
    owl:inverseOf <http://www.cidoc-crm.org/cidoc-crm/P67_refers_to> ;
    rdfs:domain <http://www.cidoc-crm.org/cidoc-crm/E1_CRM_Entity> ;
    rdfs:range <http://www.cidoc-crm.org/cidoc-crm/E89_Propositional_Object> ;
    rdfs:isDefinedBy <http://www.cidoc-crm.org/cidoc-crm/> ;
    rdfs:label "fait l'objet d'un renvoi par"@fr ,
        "is referred to by"@en ,
        "wird angeführt von"@de ,
        "é referenciado por"@pt ,
        "αναφέρεται από"@el ,
        "имеет ссылку на себя от"@ru ,
        "被涉及"@zh .


###  http://www.cidoc-crm.org/cidoc-crm/P70_documents
<http://www.cidoc-crm.org/cidoc-crm/P70_documents> rdf:type owl:ObjectProperty ;
    rdfs:subPropertyOf <http://www.cidoc-crm.org/cidoc-crm/P67_refers_to> ;
    rdfs:domain <http://www.cidoc-crm.org/cidoc-crm/E31_Document> ;
    rdfs:range <http://www.cidoc-crm.org/cidoc-crm/E1_CRM_Entity> ;
    rdfs:comment "This property refers to the fact that a document describes some entity."@en ;
    rdfs:isDefinedBy <http://www.cidoc-crm.org/cidoc-crm/> ;
    <http://purl.org/vocab/vann/example> """

        ### Example of an external web page documenting a license statement referring to
        ### a CHO at the Manifestation level.
        
        ex:32-manifestation-license a crm:E73_Information_Object ;
            crm:P2_has_type aat:300435434 ;
            crm:P67_refers_to ex:32-manifestation ;
            crm:P70i_is_documented_in <http://rightsstatements.org/vocab/InC/1.0/> .

    """@en ;
    <http://www.w3.org/2003/06/sw-vocab-status/ns#term_status> <http://purl.org/linked-data/registry#statusStable> ;
    <http://www.linkedmodel.org/schema/vaem#rationale> "This property is used to represent the relation between a license or copyright statement (modelled as a crm:E73_Information_Object with type aat:300435434) and the external document (e.g. a Web page) that describes its legal implications, either in a technical or non-technical way."@en ;
    rdfs:label "belegt"@de ,
        "documenta"@pt ,
        "documente"@fr ,
        "documents"@en ,
        "τεκμηριώνει"@el ,
        "документирует"@ru ,
        "记录了"@zh .


###  http://www.cidoc-crm.org/cidoc-crm/P70i_is_documented_in
<http://www.cidoc-crm.org/cidoc-crm/P70i_is_documented_in> rdf:type owl:ObjectProperty ;
    rdfs:subPropertyOf <http://www.cidoc-crm.org/cidoc-crm/P67i_is_referred_to_by> ;
    owl:inverseOf <http://www.cidoc-crm.org/cidoc-crm/P70_documents> ;
    rdfs:domain <http://www.cidoc-crm.org/cidoc-crm/E1_CRM_Entity> ;
    rdfs:range <http://www.cidoc-crm.org/cidoc-crm/E31_Document> ;
    rdfs:isDefinedBy <http://www.cidoc-crm.org/cidoc-crm/> ;
    rdfs:label "est documenté dans"@fr ,
        "is documented in"@en ,
        "wird belegt in"@de ,
        "é documentado em"@pt ,
        "τεκμηριώνεται σε"@el ,
        "документирован в"@ru ,
        "记录在"@zh .


###  http://www.cidoc-crm.org/cidoc-crm/P74_has_current_or_former_residence
<http://www.cidoc-crm.org/cidoc-crm/P74_has_current_or_former_residence> rdf:type owl:ObjectProperty ;
    owl:inverseOf <http://www.cidoc-crm.org/cidoc-crm/P74i_is_current_or_former_residence_of> ;
    rdfs:domain <http://www.cidoc-crm.org/cidoc-crm/E39_Actor> ;
    rdfs:range <http://www.cidoc-crm.org/cidoc-crm/E53_Place> ;
    rdfs:comment "This property describes the current or former place of residence of an actor."@en ;
    rdfs:isDefinedBy <http://www.cidoc-crm.org/cidoc-crm/> ;
    <http://www.w3.org/2003/06/sw-vocab-status/ns#term_status> <http://purl.org/linked-data/registry#statusStable> ;
    <http://www.linkedmodel.org/schema/vaem#rationale> "This property is used to represent the fact that a person or an organisation resides in a certain place."@en ;
    rdfs:label "a pour résidence actuelle ou antérieure"@fr ,
        "has current or former residence"@en ,
        "hat derzeitigen oder früheren Sitz"@de ,
        "reside ou residiu em"@pt ,
        "έχει ή είχε κατοικία"@el ,
        "имеет текущее или бывшее местожительства"@ru ,
        "有当前或曾经居住地"@zh .


###  http://www.cidoc-crm.org/cidoc-crm/P74i_is_current_or_former_residence_of
<http://www.cidoc-crm.org/cidoc-crm/P74i_is_current_or_former_residence_of> rdf:type owl:ObjectProperty ;
    rdfs:domain <http://www.cidoc-crm.org/cidoc-crm/E53_Place> ;
    rdfs:range <http://www.cidoc-crm.org/cidoc-crm/E39_Actor> ;
    rdfs:isDefinedBy <http://www.cidoc-crm.org/cidoc-crm/> ;
    rdfs:label "est la résidence actuelle ou antérieure de"@fr ,
        "is current or former residence of"@en ,
        "ist derzeitiger oder früherer Sitz von"@de ,
        "é ou foi residência de"@pt ,
        "είναι ή ήταν κατοικία του/της"@el ,
        "является текущим или бывшим местом жительства для"@ru ,
        "是当前或曾经居住地"@zh .


###  http://www.cidoc-crm.org/cidoc-crm/P94_has_created
<http://www.cidoc-crm.org/cidoc-crm/P94_has_created> rdf:type owl:ObjectProperty .


###  http://www.cidoc-crm.org/cidoc-crm/P94i_was_created_by
<http://www.cidoc-crm.org/cidoc-crm/P94i_was_created_by> rdf:type owl:ObjectProperty .


###  http://www.cidoc-crm.org/cidoc-crm/P9_consists_of
<http://www.cidoc-crm.org/cidoc-crm/P9_consists_of> rdf:type owl:ObjectProperty ;
    rdfs:subPropertyOf <http://www.cidoc-crm.org/cidoc-crm/P10i_contains> ;
    owl:inverseOf <http://www.cidoc-crm.org/cidoc-crm/P9i_forms_part_of> ;
    rdfs:domain <http://www.cidoc-crm.org/cidoc-crm/E4_Period> ;
    rdfs:range <http://www.cidoc-crm.org/cidoc-crm/E4_Period> ;
    rdfs:comment "This property associates a period of time with another period of time it contains."@en ;
    rdfs:isDefinedBy <http://www.cidoc-crm.org/cidoc-crm/> ;
    <http://purl.org/vocab/vann/example> """

        ### Example of an activity (Expression Creation) consisting of another creation activity (aat:300404387).

        ex:32-expression-creation a lrmoo:F28_Expression_Creation ;
            crm:P9_consists_of ex:32-expression-creation-activity-01 .

        ex:32-expression-creation-activity-01 a crm:E7_Activity ;
            crm:P2_has_type aat:300404387 ;
            crm:P14_carried_out_by ex:ulisse-aldrovandi .

    """@en ;
    <http://www.w3.org/2003/06/sw-vocab-status/ns#term_status> <http://purl.org/linked-data/registry#statusStable> ;
    <http://www.linkedmodel.org/schema/vaem#rationale> "This property is used to represent the fact that the creation of a CHO often consists of a set of smaller activities involving different people, techniques, and other aspects that cannot be related to a single entity."@en ;    
    rdfs:label "comprend"@fr ,
        "consiste de"@pt ,
        "consists of"@en ,
        "setzt sich zusammen aus"@de ,
        "αποτελείται από"@el ,
        "состоит из"@ru ,
        "包括"@zh .


###  http://www.cidoc-crm.org/cidoc-crm/P9i_forms_part_of
<http://www.cidoc-crm.org/cidoc-crm/P9i_forms_part_of> rdf:type owl:ObjectProperty ;
    rdfs:subPropertyOf <http://www.cidoc-crm.org/cidoc-crm/P10_falls_within> ;
    rdfs:domain <http://www.cidoc-crm.org/cidoc-crm/E4_Period> ;
    rdfs:range <http://www.cidoc-crm.org/cidoc-crm/E4_Period> ;
    rdfs:isDefinedBy <http://www.cidoc-crm.org/cidoc-crm/> ;
    rdfs:label "bildet Teil von"@de ,
        "fait partie de"@fr ,
        "faz parte de"@pt ,
        "forms part of"@en ,
        "αποτελεί μέρος του/της"@el ,
        "формирует часть"@ru ,
        "组成部分"@zh .


###  http://www.ics.forth.gr/isl/CRMdig/L10_had_input
<http://www.ics.forth.gr/isl/CRMdig/L10_had_input> rdf:type owl:ObjectProperty ;
    rdfs:subPropertyOf <http://www.cidoc-crm.org/cidoc-crm/P16_used_specific_object> ;
    owl:inverseOf <http://www.ics.forth.gr/isl/CRMdig/L10i_was_input_of> ;
    rdfs:domain <http://www.ics.forth.gr/isl/CRMdig/D7_Digital_Machine_Event> ;
    rdfs:range <http://www.ics.forth.gr/isl/CRMdig/D1_Digital_Object> ;
    rdfs:comment "This property associates an activity in a digitization workflow with a digital object used as input for that activity."@en ;
    rdfs:isDefinedBy <http://www.ics.forth.gr/isl/CRMdig/> ;
    <http://purl.org/vocab/vann/example> """

        ### Example of a processing activity (a crmdig:D10_Software_Execution with type aat:300054636) using a 
        ### DCHO (the raw 3D model acquired in the previous step).

        ex:32-processing a crmdig:D10_Software_Execution ;
            crm:P2_has_type aat:300054636 ;
            crmdig:L10_had_input ex:32-model-00 .

    """@en ;
    <http://www.w3.org/2003/06/sw-vocab-status/ns#term_status> <http://purl.org/linked-data/registry#statusStable> ;
    <http://www.linkedmodel.org/schema/vaem#rationale> "This property is used to represent the fact that a digitisation activity uses some DCHO as input for producing another DCHO as an output."@en ;        
    rdfs:label "has input"@en .


###  http://www.ics.forth.gr/isl/CRMdig/L10i_was_input_of
<http://www.ics.forth.gr/isl/CRMdig/L10i_was_input_of> rdf:type owl:ObjectProperty ;
    rdfs:subPropertyOf <http://www.cidoc-crm.org/cidoc-crm/P16i_was_used_for> ;
    rdfs:domain <http://www.ics.forth.gr/isl/CRMdig/D1_Digital_Object> ;
    rdfs:range <http://www.ics.forth.gr/isl/CRMdig/D7_Digital_Machine_Event> ;
    rdfs:isDefinedBy <http://www.ics.forth.gr/isl/CRMdig/> ;
    rdfs:label "was input of"@en .


###  http://www.ics.forth.gr/isl/CRMdig/L11_had_output
<http://www.ics.forth.gr/isl/CRMdig/L11_had_output> rdf:type owl:ObjectProperty ;
    rdfs:subPropertyOf <http://www.cidoc-crm.org/cidoc-crm/P94_has_created> ;
    rdfs:domain <http://www.ics.forth.gr/isl/CRMdig/D7_Digital_Machine_Event> ;
    rdfs:range <http://www.ics.forth.gr/isl/CRMdig/D1_Digital_Object> ;
    rdfs:comment "This property associates an activity in a digitization workflow with a digital object produced as a result of that activity."@en ;
    rdfs:isDefinedBy <http://www.ics.forth.gr/isl/CRMdig/> ;
    <http://purl.org/vocab/vann/example> """

        ### Example of a processing activity (a crmdig:D10_Software_Execution with type aat:300054636) producing a 
        ### DCHO (the processed 3D model) as an output.

        ex:32-processing a crmdig:D10_Software_Execution ;
            crm:P2_has_type aat:300054636 ;
            crmdig:L11_had_output ex:32-model-01 .

    """@en ;
    <http://www.w3.org/2003/06/sw-vocab-status/ns#term_status> <http://purl.org/linked-data/registry#statusStable> ;
    <http://www.linkedmodel.org/schema/vaem#rationale> "This property is used to represent the fact that a digitisation activity produces some DCHO as an output starting from another DCHO used as its input."@en ;
    rdfs:label "has output"@en .


###  http://www.ics.forth.gr/isl/CRMdig/L11i_was_output_of
<http://www.ics.forth.gr/isl/CRMdig/L11i_was_output_of> rdf:type owl:ObjectProperty ;
    rdfs:subPropertyOf <http://www.cidoc-crm.org/cidoc-crm/P94i_was_created_by> ;
    owl:inverseOf <http://www.ics.forth.gr/isl/CRMdig/L11_had_output> ;
    rdfs:domain <http://www.ics.forth.gr/isl/CRMdig/D1_Digital_Object> ;
    rdfs:range <http://www.ics.forth.gr/isl/CRMdig/D7_Digital_Machine_Event> ;
    rdfs:isDefinedBy <http://www.ics.forth.gr/isl/CRMdig/> ;
    rdfs:label "was output of"@en .


###  http://www.ics.forth.gr/isl/CRMdig/L1_digitized
<http://www.ics.forth.gr/isl/CRMdig/L1_digitized> rdf:type owl:ObjectProperty ;
    rdfs:subPropertyOf <http://www.cidoc-crm.org/cidoc-crm/P39_measured> ;
    rdfs:domain <http://www.ics.forth.gr/isl/CRMdig/D2_Digitization_Process> ;
    rdfs:range <http://www.cidoc-crm.org/cidoc-crm/E18_Physical_Thing> ;
    rdfs:comment "This property associates a digitization process with the cultural heritage object that is being digitized."@en ;
    rdfs:isDefinedBy <http://www.ics.forth.gr/isl/CRMdig/> ;
    <http://purl.org/vocab/vann/example> """

        ### Example of an acquisition activity digitising a CHO at the Item level to produce a DCHO 
        ### (the raw 3D model) as an output.

        ex:32-acquisition a crmdig:D2_Digitization_Process ;
            crmdig:L1_digitized ex:32-item ;
            crmdig:L11_had_output ex:32-model-00 .

    """@en ;
    <http://www.w3.org/2003/06/sw-vocab-status/ns#term_status> <http://purl.org/linked-data/registry#statusStable> ;
    <http://www.linkedmodel.org/schema/vaem#rationale> "This property is used to represent the fact that an acquisition activity digitises some CHO to produce a DCHO as an output."@en ;
    rdfs:label "digitized"@en .


###  http://www.ics.forth.gr/isl/CRMdig/L1i_was_digitized_by
<http://www.ics.forth.gr/isl/CRMdig/L1i_was_digitized_by> rdf:type owl:ObjectProperty ;
    rdfs:subPropertyOf <http://www.cidoc-crm.org/cidoc-crm/P39i_was_measured_by> ;
    owl:inverseOf <http://www.ics.forth.gr/isl/CRMdig/L1_digitized> ;
    rdfs:domain <http://www.cidoc-crm.org/cidoc-crm/E18_Physical_Thing> ;
    rdfs:range <http://www.ics.forth.gr/isl/CRMdig/D2_Digitization_Process> ;
    rdfs:isDefinedBy <http://www.ics.forth.gr/isl/CRMdig/> ;
    rdfs:label "was digitized by"@en .


###  http://www.ics.forth.gr/isl/CRMdig/L23_used_software_or_firmware
<http://www.ics.forth.gr/isl/CRMdig/L23_used_software_or_firmware> rdf:type owl:ObjectProperty ;
    rdfs:subPropertyOf <http://www.cidoc-crm.org/cidoc-crm/P16_used_specific_object> ;
    rdfs:domain <http://www.ics.forth.gr/isl/CRMdig/D7_Digital_Machine_Event> ;
    rdfs:range <http://www.ics.forth.gr/isl/CRMdig/D14_Software> ;
    rdfs:comment "This property associates a digitization activity with the software that was used during that activity."@en ;
    rdfs:isDefinedBy <http://www.ics.forth.gr/isl/CRMdig/> ;
    <http://purl.org/vocab/vann/example> """

        ### Example of a processing activity using 3D Zephyr for producing its output 

        ex:32-processing a crmdig:D10_Software_Execution ;
            crm:P2_has_type aat:300054636 ;
            crmdig:L10_had_input ex:32-model-00 ;
            crmdig:L11_had_output ex:32-model-01 ;
            crmdig:L23_used_software_or_firmware ex:3df-zephyr .

    """@en ;
    <http://www.w3.org/2003/06/sw-vocab-status/ns#term_status> <http://purl.org/linked-data/registry#statusStable> ;
    <http://www.linkedmodel.org/schema/vaem#rationale> "This property is used to represent the fact that during a digitisation activity one or more software are used to produce its output."@en ;
    rdfs:label "used software or firmware"@en .


#################################################################
#    Data properties
#################################################################

###  http://www.cidoc-crm.org/cidoc-crm/P190_has_symbolic_content
<http://www.cidoc-crm.org/cidoc-crm/P190_has_symbolic_content> rdf:type owl:DatatypeProperty ;
    rdfs:subPropertyOf <http://www.cidoc-crm.org/cidoc-crm/P3_has_note> ;
    rdfs:domain <http://www.cidoc-crm.org/cidoc-crm/E90_Symbolic_Object> ;
    rdfs:range rdfs:Literal ;
    rdfs:comment "This property associates a symbolic object with a textual representation of its content."@en ;
    rdfs:isDefinedBy <http://www.cidoc-crm.org/cidoc-crm/> ;
    <http://purl.org/vocab/vann/example> """

        ### Example of the textual content of a title 

        ex:32-work-title-01 a crm:E35_Title ;
            crm:P190_has_symbolic_content "Essere umano ermafrodita"@it .

    """@en ;
    <http://www.w3.org/2003/06/sw-vocab-status/ns#term_status> <http://purl.org/linked-data/registry#statusStable> ;
    <http://www.linkedmodel.org/schema/vaem#rationale> "This property is used to represent the textual content of entities such as titles and identifiers."@en ;    
    rdfs:label "a pour contenu symbolique"@fr ,
                "has symbolic content"@en .


###  http://www.cidoc-crm.org/cidoc-crm/P3_has_note
<http://www.cidoc-crm.org/cidoc-crm/P3_has_note> rdf:type owl:DatatypeProperty ;
    rdfs:domain <http://www.cidoc-crm.org/cidoc-crm/E1_CRM_Entity> ;
    rdfs:range rdfs:Literal ;
    rdfs:comment "This property contains the textual description of an entity."@en ;
    rdfs:isDefinedBy <http://www.cidoc-crm.org/cidoc-crm/> ;
    <http://purl.org/vocab/vann/example> """

        ### Example of the textual description of a CHO at the Item level

        ex:32-item a lrmoo:F5_Item ;
            crm:P3_has_note '''
                Essere umano ermafrodita 
                Human hermaphrodite (Monstrum humanum hermaphroditicum) 
                sec. XVI 
                16th century 
                BUB, 
                Ms. Aldrovandi, Tavole di animali, vol. 5, carta 86
            '''^^rdfs:Literal .

    """@en ;
    <http://www.w3.org/2003/06/sw-vocab-status/ns#term_status> <http://purl.org/linked-data/registry#statusStable> ;
    <http://www.linkedmodel.org/schema/vaem#rationale> "This property is used to represent the textual description of a CHO at the Item level (thus intended as an exemplar of the exhibition)."@en ;        
    rdfs:label "a pour note"@fr ,
        "has note"@en ,
        "hat Anmerkung"@de ,
        "tem nota"@pt ,
        "έχει επεξήγηση"@el ,
        "имеет примечание"@ru ,
        "有注释"@zh .


###  http://www.cidoc-crm.org/cidoc-crm/P82_at_some_time_within
<http://www.cidoc-crm.org/cidoc-crm/P82_at_some_time_within> rdf:type owl:DatatypeProperty ;
    rdfs:domain <http://www.cidoc-crm.org/cidoc-crm/E52_Time-Span> ;
    rdfs:range rdfs:Literal ;
    rdfs:comment "This property describes the maximum period of time within which a time span falls."@en ;
    rdfs:isDefinedBy <http://www.cidoc-crm.org/cidoc-crm/> ;
    <http://www.w3.org/2003/06/sw-vocab-status/ns#term_status> <http://purl.org/linked-data/registry#statusStable> ;
    <http://www.linkedmodel.org/schema/vaem#rationale> "This property is used to represent the instances of fuzzy temporal descriptions of time spans (e.g. when a time span has no precise starting or ending date times)."@en ;        
    rdfs:label "a eu lieu durant"@fr ,
        "abrange no máximo"@pt ,
        "at some time within"@en ,
        "irgendwann innerhalb von"@de ,
        "κάποτε εντός"@el ,
        "некоторое время в течение"@ru ,
        "最长范围是"@zh .


###  http://www.cidoc-crm.org/cidoc-crm/P82a_begin_of_the_begin
<http://www.cidoc-crm.org/cidoc-crm/P82a_begin_of_the_begin> rdf:type owl:DatatypeProperty ;
    rdfs:subPropertyOf <http://www.cidoc-crm.org/cidoc-crm/P82_at_some_time_within> ;
    rdfs:domain <http://www.cidoc-crm.org/cidoc-crm/E52_Time-Span> ;
    rdfs:range xsd:dateTime ;
    rdfs:comment "This property describes the precise beginning date and time of a time span."@en ;
    rdfs:isDefinedBy <http://www.cidoc-crm.org/cidoc-crm/> ;
    <http://purl.org/vocab/vann/example> """

        ### Example of a time span having a beginning date time

        ex:1500-1599 a crm:E52_Time-Span ;
            crm:P82a_begin_of_the_begin "1500-01-01T00:00:00Z"^^xsd:dateTime .

    """@en ;
    <http://www.w3.org/2003/06/sw-vocab-status/ns#term_status> <http://purl.org/linked-data/registry#statusStable> ;
    <http://www.linkedmodel.org/schema/vaem#rationale> "This property is used to represent the precise beginning date time of a time span."@en ;        
    rdfs:label "Anfang des Anfangs"@de ,
        "begin of the begin"@en ,
        "começar do início"@pt ,
        "début du début"@fr ,
        "αρχή της αρχής"@el ,
        "начать с начала"@ru .


###  http://www.cidoc-crm.org/cidoc-crm/P82b_end_of_the_end
<http://www.cidoc-crm.org/cidoc-crm/P82b_end_of_the_end> rdf:type owl:DatatypeProperty ;
    rdfs:subPropertyOf <http://www.cidoc-crm.org/cidoc-crm/P82_at_some_time_within> ;
    rdfs:domain <http://www.cidoc-crm.org/cidoc-crm/E52_Time-Span> ;
    rdfs:range xsd:dateTime ;
    rdfs:comment "This property describes the precise ending date and time of a time span."@en ;
    rdfs:isDefinedBy <http://www.cidoc-crm.org/cidoc-crm/> ;
    <http://purl.org/vocab/vann/example> """

        ### Example of a time span having a ending date time

        ex:1500-1599 a crm:E52_Time-Span ;
            crm:P82b_end_of_the_end "1599-12-31T23:59:59Z"^^xsd:dateTime .

    """@en ;
    <http://www.w3.org/2003/06/sw-vocab-status/ns#term_status> <http://purl.org/linked-data/registry#statusStable> ;
    <http://www.linkedmodel.org/schema/vaem#rationale> "This property is used to represent the precise ending date time of a time span."@en ;        
    rdfs:label "Ende vom Ende"@de ,
                "end of the end"@en ,
                "fim do fim"@pt ,
                "fin de la fin"@fr ,
                "τέλος του τέλους"@el ,
                "конец конец"@ru .


#################################################################
#    Classes
#################################################################


###  http://iflastandards.info/ns/lrm/lrmoo/F1_Work
<http://iflastandards.info/ns/lrm/lrmoo/F1_Work> rdf:type owl:Class ;
    rdfs:label "Work"@en ;
    rdfs:comment "The essence or conceptualisation of an endeavor."@en ;
    rdfs:subClassOf crm:E89_Propositional_Object ;
    <http://purl.org/vocab/vann/example> """

        ### Example of a CHO at the Work level, characterised by two titles and realised in an Expression

        ex:32-work a lrmoo:F1_Work ;
            crm:P102_has_title ex:32-work-title-01 ,
                ex:32-work-title-02 ;
            lrmoo:R3_is_realised_in ex:32-expression .

    """@en ;
    <http://www.w3.org/2003/06/sw-vocab-status/ns#term_status> <http://purl.org/linked-data/registry#statusStable> ;
    <http://www.linkedmodel.org/schema/vaem#rationale> "This class represents the Work level of conceptualisation as instructed by the LRM conceptual model. The Work represents the essence of a CHO, as it was thought out during its conception in the mind of its creator(s)."@en ;        
    rdfs:isDefinedBy <http://iflastandards.info/ns/lrm/lrmoo/> .


###  http://iflastandards.info/ns/lrm/lrmoo/F28_Expression_Creation
<http://iflastandards.info/ns/lrm/lrmoo/F28_Expression_Creation> rdf:type owl:Class ;
    rdfs:subClassOf <http://www.cidoc-crm.org/cidoc-crm/E12_Production> ,
                    <http://www.cidoc-crm.org/cidoc-crm/E65_Creation> ;
    rdfs:comment "An activity that represents the creation of an expression."@en ;
    rdfs:isDefinedBy <http://iflastandards.info/ns/lrm/lrmoo/> ;
    <http://purl.org/vocab/vann/example> """

        ### Example of an Expression Creation. It consists of a smaller activity; it is carried out through a drawing
        ### technique; it happens during the XVI century; and it generates both the Expression of the CHO (its content) and
        ### its realisation (the Work).

        ex:32-expression-creation a lrmoo:F28_Expression_Creation ;
            crm:P9_consists_of ex:32-expression-creation-activity-01 ;
            crm:P32_used_general_technique aat:300054196 ;
            lrmoo:R19_created_a_realisation_of ex:32-work ;
            lrmoo:R17_created ex:32-expression ;
            crm:P4_has_time-span ex:1500-1599 .

    """@en ;
    <http://www.w3.org/2003/06/sw-vocab-status/ns#term_status> <http://purl.org/linked-data/registry#statusStable> ;
    <http://www.linkedmodel.org/schema/vaem#rationale> "This class represents the creation of the CHO at both the Work and Expression levels."@en ;
    rdfs:label "Expression Creation"@en .


###  http://iflastandards.info/ns/lrm/lrmoo/F2_Expression
<http://iflastandards.info/ns/lrm/lrmoo/F2_Expression> rdf:type owl:Class ;
    rdfs:subClassOf <http://www.cidoc-crm.org/cidoc-crm/E73_Information_Object> ;
    rdfs:comment "The realisation of a work, referring to the intellectual content of a cultural heritage object."@en ;
    rdfs:isDefinedBy <http://iflastandards.info/ns/lrm/lrmoo/> ;
    <http://purl.org/vocab/vann/example> """

        ### Example of a CHO at the Expression level, characterised by a subject and embodied in a Manifestation

        ex:32-expression a lrmoo:F2_Expression ;
            crm:P129_is_about ex:ermafrodita ;
            lrmoo:R4i_is_embodied_in ex:32-manifestation .

    """@en ;
    <http://www.w3.org/2003/06/sw-vocab-status/ns#term_status> <http://purl.org/linked-data/registry#statusStable> ;
    <http://www.linkedmodel.org/schema/vaem#rationale> "This class represents the Expression level of conceptualisation as instructed by the LRM conceptual model. The Expression represents the content of a CHO, intended as the specific intellectual or artistic form that a Work takes each time it is realised."@en ;
    rdfs:label "Expression"@en .


###  http://iflastandards.info/ns/lrm/lrmoo/F3_Manifestation
<http://iflastandards.info/ns/lrm/lrmoo/F3_Manifestation> rdf:type owl:Class ;
    rdfs:label "Manifestation"@en ;
    rdfs:comment "The rendering of one or more expressions. It is defined by both the overall content and the form of its presentation. The substance of manifestation is not only signs, but also the manner in which they are presented to be consumed by users, including the kind of media adopted."@en ;
    rdfs:subClassOf crm:E73_Information_Object ;
    <http://purl.org/vocab/vann/example> """

        ### Example of a CHO at the Manifestation level, characterised by a type and exemplified in an Item

        ex:32-manifestation a lrmoo:F3_Manifestation ;
            crm:P2_has_type aat:300028569 ;
            lrmoo:R7i_is_exemplified_by ex:32-item .

    """@en ;
    <http://www.w3.org/2003/06/sw-vocab-status/ns#term_status> <http://purl.org/linked-data/registry#statusStable> ;
    <http://www.linkedmodel.org/schema/vaem#rationale> "This class represents the Manifestation level of conceptualisation as instructed by the LRM conceptual model. The Manifestation represents the format of a CHO, intended as the result from the capture of one or more Expressions onto a carrier or set of carriers."@en ;
    rdfs:isDefinedBy <http://iflastandards.info/ns/lrm/lrmoo/> .


lrmoo:F5_Item 
    a owl:Class ;
    rdfs:label "Item"@en ;
    rdfs:comment "This class comprises physical objects that were produced by a process involving a given manifestation."@en ;
    rdfs:subClassOf crm:E24_Physical_Human-Made_Thing ;
    <http://purl.org/vocab/vann/example> """

        ### Example of a CHO at the Item level, characterised by three identifiers and a description

        ex:32-item a lrmoo:F5_Item ;
            crm:P1_is_identified_by ex:32-item-identifier-01 ,
                ex:32-item-identifier-02 ,
                ex:32-item-identifier-03 ;
            crm:P3_has_note '''
                Essere umano ermafrodita 
                Human hermaphrodite (Monstrum humanum hermaphroditicum) 
                sec. XVI 
                16th century 
                BUB, 
                Ms. Aldrovandi, Tavole di animali, vol. 5, carta 86
                '''^^rdfs:Literal .

    """@en ;
    <http://www.w3.org/2003/06/sw-vocab-status/ns#term_status> <http://purl.org/linked-data/registry#statusStable> ;
    <http://www.linkedmodel.org/schema/vaem#rationale> "This class represents the Item level of conceptualisation as instructed by the LRM conceptual model. The Item represents the single exemplar of a CHO, intended as an object physically localised."@en ;
    rdfs:isDefinedBy <http://iflastandards.info/ns/lrm/lrmoo/> .


###  http://vocab.getty.edu/aat/Concept
<http://vocab.getty.edu/aat/Concept> rdf:type owl:Class .


###  http://www.cidoc-crm.org/cidoc-crm/E12_Production
<http://www.cidoc-crm.org/cidoc-crm/E12_Production> rdf:type owl:Class .


###  http://www.cidoc-crm.org/cidoc-crm/E18_Physical_Thing
<http://www.cidoc-crm.org/cidoc-crm/E18_Physical_Thing> rdf:type owl:Class .


###  http://www.cidoc-crm.org/cidoc-crm/E1_CRM_Entity
<http://www.cidoc-crm.org/cidoc-crm/E1_CRM_Entity> rdf:type owl:Class .


###  http://www.cidoc-crm.org/cidoc-crm/E20_Biological_Object
<http://www.cidoc-crm.org/cidoc-crm/E20_Biological_Object> rdf:type owl:Class .


###  http://www.cidoc-crm.org/cidoc-crm/E21_Person
<http://www.cidoc-crm.org/cidoc-crm/E21_Person> rdf:type owl:Class ;
    rdfs:subClassOf <http://www.cidoc-crm.org/cidoc-crm/E20_Biological_Object> ,
                    <http://www.cidoc-crm.org/cidoc-crm/E39_Actor> ;
    rdfs:comment "An individual person."@en ;
    <http://www.w3.org/2003/06/sw-vocab-status/ns#term_status> <http://purl.org/linked-data/registry#statusStable> ;
    <http://www.linkedmodel.org/schema/vaem#rationale> "This class represents a person, usually involved in some sort of activity."@en ;
    rdfs:isDefinedBy <http://www.cidoc-crm.org/cidoc-crm/> ;
    rdfs:label "Person"@de ,
            "Person"@en ,
            "Personne"@fr ,
            "Pessoa"@pt ,
            "Πρόσωπο"@el ,
            "Личность"@ru ,
            "人物"@zh .


###  http://www.cidoc-crm.org/cidoc-crm/E22_Man-Made_Object
<http://www.cidoc-crm.org/cidoc-crm/E22_Man-Made_Object> rdf:type owl:Class .


###  http://www.cidoc-crm.org/cidoc-crm/E24_Physical_Human-Made_Thing
<http://www.cidoc-crm.org/cidoc-crm/E24_Physical_Human-Made_Thing> rdf:type owl:Class ;
    rdfs:subClassOf <http://www.cidoc-crm.org/cidoc-crm/E18_Physical_Thing> ,
        <http://www.cidoc-crm.org/cidoc-crm/E71_Human-Made_Thing> ;
    rdfs:comment "A persistent physical item of any size that is purposely created by human activity."@en ;
    rdfs:isDefinedBy <http://www.cidoc-crm.org/cidoc-crm/> ;
    <http://www.w3.org/2003/06/sw-vocab-status/ns#term_status> <http://purl.org/linked-data/registry#statusStable> ;
    <http://www.linkedmodel.org/schema/vaem#rationale> "This class is used in conjunction with crm:P2_has_type and aat:300025976 to represent the concept of collection."@en ;
    rdfs:label "Chose matérielle élaborée par l’humain"@fr ,
        "Physical Human-Made Thing"@en .


###  http://www.cidoc-crm.org/cidoc-crm/E28_Conceptual_Object
<http://www.cidoc-crm.org/cidoc-crm/E28_Conceptual_Object> rdf:type owl:Class .


###  http://www.cidoc-crm.org/cidoc-crm/E2_Temporal_Entity
<http://www.cidoc-crm.org/cidoc-crm/E2_Temporal_Entity> rdf:type owl:Class .


###  http://www.cidoc-crm.org/cidoc-crm/E31_Document
<http://www.cidoc-crm.org/cidoc-crm/E31_Document> rdf:type owl:Class ;
    rdfs:subClassOf <http://www.cidoc-crm.org/cidoc-crm/E73_Information_Object> ;
    rdfs:comment "An information object that makes propositions about reality."@en ;
    rdfs:isDefinedBy <http://www.cidoc-crm.org/cidoc-crm/> ;
    <http://www.w3.org/2003/06/sw-vocab-status/ns#term_status> <http://purl.org/linked-data/registry#statusStable> ;
    <http://www.linkedmodel.org/schema/vaem#rationale> "This class is implicitly used in conjunction with crm:P70i_is_documented_in to represent external resources (e.g. copyright statements, authority records, etc.)."@en ;
    rdfs:label "Document"@en ,
        "Document"@fr ,
        "Documento"@pt ,
        "Dokument"@de ,
        "Τεκμήριο"@el ,
        "Документ"@ru ,
        "文献"@zh .


###  http://www.cidoc-crm.org/cidoc-crm/E33_Linguistic_Object
<http://www.cidoc-crm.org/cidoc-crm/E33_Linguistic_Object> rdf:type owl:Class .


###  http://www.cidoc-crm.org/cidoc-crm/E35_Title
<http://www.cidoc-crm.org/cidoc-crm/E35_Title> rdf:type owl:Class ;
    rdfs:subClassOf <http://www.cidoc-crm.org/cidoc-crm/E33_Linguistic_Object> ,
        <http://www.cidoc-crm.org/cidoc-crm/E41_Appellation> ;
    rdfs:comment "A textual string that functions as a title for a work."@en ;
    rdfs:isDefinedBy <http://www.cidoc-crm.org/cidoc-crm/> ;
    <http://purl.org/vocab/vann/example> """

        ### Example of a title, characterised by a type and a textual content

        ex:32-work-title-01 a crm:E35_Title ;
            crm:P2_has_type aat:300417204 ;
            crm:P190_has_symbolic_content "Essere umano ermafrodita"@it .

    """@en ;
    <http://www.w3.org/2003/06/sw-vocab-status/ns#term_status> <http://purl.org/linked-data/registry#statusStable> ;
    <http://www.linkedmodel.org/schema/vaem#rationale> "This class represents a title given to the CHO at the Work level."@en ;
    rdfs:label "Titel"@de ,
        "Title"@en ,
        "Titre"@fr ,
        "Título"@pt ,
        "Τίτλος"@el ,
        "Заголовок"@ru ,
        "题名"@zh .


###  http://www.cidoc-crm.org/cidoc-crm/E39_Actor
<http://www.cidoc-crm.org/cidoc-crm/E39_Actor> rdf:type owl:Class ;
    rdfs:subClassOf <http://www.cidoc-crm.org/cidoc-crm/E77_Persistent_Item> ;
    rdfs:comment "An individual person or a group of people, with the potential to perform intentional and accountable actions."@en ;
    rdfs:isDefinedBy <http://www.cidoc-crm.org/cidoc-crm/> ;
    <http://www.w3.org/2003/06/sw-vocab-status/ns#term_status> <http://purl.org/linked-data/registry#statusStable> ;
    <http://www.linkedmodel.org/schema/vaem#rationale> "This class represents a generic entity with an agency, which can be either a person or an organisation."@en ;
    rdfs:label "Actant"@fr ,
        "Actor"@en ,
        "Agente"@pt ,
        "Akteur"@de ,
        "Δράστης"@el ,
        "Агент"@ru ,
        "参与者"@zh .


###  http://www.cidoc-crm.org/cidoc-crm/E41_Appellation
<http://www.cidoc-crm.org/cidoc-crm/E41_Appellation> rdf:type owl:Class .


###  http://www.cidoc-crm.org/cidoc-crm/E42_Identifier
<http://www.cidoc-crm.org/cidoc-crm/E42_Identifier> rdf:type owl:Class ;
    rdfs:subClassOf <http://www.cidoc-crm.org/cidoc-crm/E41_Appellation> ;
    rdfs:comment "A textual string assigned to a cultural heritage object in order to identify it uniquely within a given context."@en ;
    rdfs:isDefinedBy <http://www.cidoc-crm.org/cidoc-crm/> ;
    <http://purl.org/vocab/vann/example> """

        ### Example of an identifier, characterised by a type and a textual content

        ex:32-item-identifier-01 a crm:E42_Identifier ;
            crm:P2_has_type aat:300312355 ;
            crm:P190_has_symbolic_content "32"^^rdfs:Literal .

    """@en ;
    <http://www.w3.org/2003/06/sw-vocab-status/ns#term_status> <http://purl.org/linked-data/registry#statusStable> ;
    <http://www.linkedmodel.org/schema/vaem#rationale> "This class represents a identifier given to the CHO at the Item level."@en ;
    rdfs:label "Identifiant"@fr ,
        "Identificador de Objeto"@pt ,
        "Identifier"@en ,
        "Kennung"@de ,
        "Κωδικός Αναγνώρισης"@el ,
        "Идентификатор Объекта"@ru ,
        "标识符"@zh .


###  http://www.cidoc-crm.org/cidoc-crm/E4_Period
<http://www.cidoc-crm.org/cidoc-crm/E4_Period> rdf:type owl:Class .


###  http://www.cidoc-crm.org/cidoc-crm/E52_Time-Span
<http://www.cidoc-crm.org/cidoc-crm/E52_Time-Span> rdf:type owl:Class ;
    rdfs:subClassOf <http://www.cidoc-crm.org/cidoc-crm/E1_CRM_Entity> ;
    rdfs:comment "An abstract temporal extent having a beginning, an end and a duration."@en ;
    rdfs:isDefinedBy <http://www.cidoc-crm.org/cidoc-crm/> ;
    <http://purl.org/vocab/vann/example> """

        ### Example of a time span, characterised by a starting date time and an ending date time

        ex:1500-1599 a crm:E52_Time-Span ;
            crm:P82a_begin_of_the_begin "1500-01-01T00:00:00Z"^^xsd:dateTime ;
            crm:P82b_end_of_the_end "1599-12-31T23:59:59Z"^^xsd:dateTime .

    """@en ;
    <http://www.w3.org/2003/06/sw-vocab-status/ns#term_status> <http://purl.org/linked-data/registry#statusStable> ;
    <http://www.linkedmodel.org/schema/vaem#rationale> "This class represents a period of time defined within a starting date time and an ending date time. Both dates are declared in the following form 'YYYY-MM-DDThh:mm:ss', as instructed by the XML Schema Definition (XSD)."@en ;
    rdfs:label "Intervalle temporel"@fr ,
        "Período de Tempo"@pt ,
        "Time-Span"@en ,
        "Zeitspanne"@de ,
        "Χρονικό Διάστημα"@el ,
        "Интервал Времени"@ru ,
        "时段"@zh .


###  http://www.cidoc-crm.org/cidoc-crm/E53_Place
<http://www.cidoc-crm.org/cidoc-crm/E53_Place> rdf:type owl:Class ;
    rdfs:subClassOf <http://www.cidoc-crm.org/cidoc-crm/E1_CRM_Entity> ;
    rdfs:comment "A geographical location."@en ;
    rdfs:isDefinedBy <http://www.cidoc-crm.org/cidoc-crm/> ;
    <http://www.w3.org/2003/06/sw-vocab-status/ns#term_status> <http://purl.org/linked-data/registry#statusStable> ;
    <http://www.linkedmodel.org/schema/vaem#rationale> "This class represents a geograhical location, usually indicating the current residence of some actor."@en ;
    rdfs:label "Lieu"@fr ,
        "Local"@pt ,
        "Ort"@de ,
        "Place"@en ,
        "Τόπος"@el ,
        "Место"@ru ,
        "地点"@zh .


###  http://www.cidoc-crm.org/cidoc-crm/E54_Dimension
<http://www.cidoc-crm.org/cidoc-crm/E54_Dimension> rdf:type owl:Class .


###  http://www.cidoc-crm.org/cidoc-crm/E55_Type
<http://www.cidoc-crm.org/cidoc-crm/E55_Type> rdf:type owl:Class ;
    rdfs:subClassOf <http://www.cidoc-crm.org/cidoc-crm/E28_Conceptual_Object> ;
    rdfs:comment "A categorical concept denoted by terms from thesauri and controlled vocabularies used to characterize and classify other entities."@en ;
    rdfs:isDefinedBy <http://www.cidoc-crm.org/cidoc-crm/> ;
    <http://www.w3.org/2003/06/sw-vocab-status/ns#term_status> <http://purl.org/linked-data/registry#statusStable> ;
    <http://www.linkedmodel.org/schema/vaem#rationale> "This class is indirectly used in conjunction with crm:P2_has_type as a typification mechanism that can be applied to a variety of cases (e.g. activities, CHOs, techniques, etc.). This mechanism allows one to rely on existing and well-established external vocabularies, such as the Getty's Art and Architecture Thesaurus (AAT), to do the heavy lifting in modelling named individuals."@en ;
    rdfs:label "Tipo"@pt ,
        "Type"@en ,
        "Type"@fr ,
        "Typus"@de ,
        "Τύπος"@el ,
        "Тип"@ru ,
        "类型"@zh .


###  http://www.cidoc-crm.org/cidoc-crm/E5_Event
<http://www.cidoc-crm.org/cidoc-crm/E5_Event> rdf:type owl:Class .


###  http://www.cidoc-crm.org/cidoc-crm/E65_Creation
<http://www.cidoc-crm.org/cidoc-crm/E65_Creation> rdf:type owl:Class .


###  http://www.cidoc-crm.org/cidoc-crm/E70_Thing
<http://www.cidoc-crm.org/cidoc-crm/E70_Thing> rdf:type owl:Class .


###  http://www.cidoc-crm.org/cidoc-crm/E71_Human-Made_Thing
<http://www.cidoc-crm.org/cidoc-crm/E71_Human-Made_Thing> rdf:type owl:Class .


###  http://www.cidoc-crm.org/cidoc-crm/E73_Information_Object
<http://www.cidoc-crm.org/cidoc-crm/E73_Information_Object> rdf:type owl:Class ;
    rdfs:subClassOf <http://www.cidoc-crm.org/cidoc-crm/E89_Propositional_Object> ,
        <http://www.cidoc-crm.org/cidoc-crm/E90_Symbolic_Object> ;
    rdfs:comment "An immaterial item that has an objectively recognizable structure and is documented as a single unit."@en ;
    rdfs:isDefinedBy <http://www.cidoc-crm.org/cidoc-crm/> ;
    <http://purl.org/vocab/vann/example> """

        ### Example of two Information Objects, one representing a copyright statement and 
        ### the other representing a subject of a CHO at the Expression level

        ex:32-manifestation-license a crm:E73_Information_Object ;
            crm:P2_has_type aat:300435434 ;
            crm:P67_refers_to ex:32-manifestation ;
            crm:P70i_is_documented_in <http://rightsstatements.org/vocab/InC/1.0/> .

        ex:ermafrodita a crm:E73_Information_Object ;
            crm:P2_has_type aat:300404126 .

    """@en ;
    <http://www.w3.org/2003/06/sw-vocab-status/ns#term_status> <http://purl.org/linked-data/registry#statusStable> ;
    <http://www.linkedmodel.org/schema/vaem#rationale> "This class consists in a generic abstract construct that can be used in conjunction with crm:P2_has_type to represent conceptual entities like rights statements and CHOs subjects."@en ;    
    rdfs:label "Information Object"@en ,
        "Informationsgegenstand"@de ,
        "Objet informationnel"@fr ,
        "Objeto de Informação"@pt ,
        "Πληροφοριακό Αντικείμενο"@el ,
        "Информационный Объект"@ru ,
        "信息对象"@zh .


###  http://www.cidoc-crm.org/cidoc-crm/E74_Group
<http://www.cidoc-crm.org/cidoc-crm/E74_Group> rdf:type owl:Class ;
    rdfs:subClassOf <http://www.cidoc-crm.org/cidoc-crm/E39_Actor> ;
    rdfs:comment "A unified group of people."@en ;
    rdfs:isDefinedBy <http://www.cidoc-crm.org/cidoc-crm/> ;
    <http://www.w3.org/2003/06/sw-vocab-status/ns#term_status> <http://purl.org/linked-data/registry#statusStable> ;
    <http://www.linkedmodel.org/schema/vaem#rationale> "This class represents organisations and other entities made up by groups of actors."@en ;    
    rdfs:label "Group"@en ,
        "Groupe"@fr ,
        "Grupo"@pt ,
        "Menschliche Gruppe"@de ,
        "Ομάδα"@el ,
        "Группа"@ru ,
        "团体"@zh . 


###  http://www.cidoc-crm.org/cidoc-crm/E77_Persistent_Item
<http://www.cidoc-crm.org/cidoc-crm/E77_Persistent_Item> rdf:type owl:Class .


###  http://www.cidoc-crm.org/cidoc-crm/E7_Activity
<http://www.cidoc-crm.org/cidoc-crm/E7_Activity> rdf:type owl:Class ;
    rdfs:subClassOf <http://www.cidoc-crm.org/cidoc-crm/E5_Event> ;
    rdfs:comment "An action intentionally carried out by one or more actors."@en ;
    rdfs:isDefinedBy <http://www.cidoc-crm.org/cidoc-crm/> ;
    <http://purl.org/vocab/vann/example> """

        ### Example of activity consisting in the curation (aat:300054277) of a 
        ### CHO at the Item level, carried out by a cultural organization (BUB)

        ex:32-item-curation a crm:E7_Activity ;
            crm:P2_has_type aat:300054277 ;
            crm:P16_used_specific_object ex:32-item ;
            crm:P14_carried_out_by ex:bub .

    """@en ;
    <http://www.w3.org/2003/06/sw-vocab-status/ns#term_status> <http://purl.org/linked-data/registry#statusStable> ;
    <http://www.linkedmodel.org/schema/vaem#rationale> "This class consists in a generic action carried out by one or more actors. An activity should at least be typified (through the combination of crm:P2_has_type and AAT) and assigned to its respective actors, although its properties may vary depending on the type of activity."@en ;    
    rdfs:label "Activity"@en ,
        "Activité"@fr ,
        "Atividade"@pt ,
        "Handlung"@de ,
        "Δράση"@el ,
        "Деятельность"@ru ,
        "活动"@zh .


###  http://www.cidoc-crm.org/cidoc-crm/E89_Propositional_Object
<http://www.cidoc-crm.org/cidoc-crm/E89_Propositional_Object> rdf:type owl:Class .


###  http://www.cidoc-crm.org/cidoc-crm/E90_Symbolic_Object
<http://www.cidoc-crm.org/cidoc-crm/E90_Symbolic_Object> rdf:type owl:Class .


###  http://www.ics.forth.gr/isl/CRMdig/D10_Software_Execution
<http://www.ics.forth.gr/isl/CRMdig/D10_Software_Execution> rdf:type owl:Class ;
    rdfs:subClassOf <http://www.ics.forth.gr/isl/CRMdig/D7_Digital_Machine_Event> ;
    rdfs:comment "An activity in which a digital device runs a software program on a digital object."@en ;
    rdfs:isDefinedBy <http://www.ics.forth.gr/isl/CRMdig/> ;
    <http://purl.org/vocab/vann/example> """

        ### Example of software activity consisting in the processing (aat:300054636) of the 
        ### DCHO produced by the previous acquisition activity, carried out by an expert
        ### (ex:alice-bordignon) during a defined time-span (ex:32-processing-timespan) using a 
        ### certain tool (ex:3df-zephyr).

        ex:32-processing a crmdig:D10_Software_Execution ;
            crm:P2_has_type aat:300054636 ;
            crmdig:L10_had_input ex:32-model-00 ;
            crmdig:L11_had_output ex:32-model-01 ;
            crm:P4_has_time-span ex:32-processing-timespan ;
            crm:P11_had_participant ex:unibo-ficlit ;
            crm:P14_carried_out_by ex:alice-bordignon ;
            crmdig:L23_used_software_or_firmware ex:3df-zephyr .

    """@en ;
    <http://www.w3.org/2003/06/sw-vocab-status/ns#term_status> <http://purl.org/linked-data/registry#statusStable> ;
    <http://www.linkedmodel.org/schema/vaem#rationale> "This class consists in a digitisation activity that follows the digital acquisition of a CHO. A software activity should at least be typified (through the combination of crm:P2_has_type and AAT), be assigned to its respective actors, have defined both its input and its output, have a time-span, and have the tool(s) used to carry it out."@en ;        
    rdfs:label "Software Execution"@en .


###  http://www.ics.forth.gr/isl/CRMdig/D11_Digital_Measurement_Event
<http://www.ics.forth.gr/isl/CRMdig/D11_Digital_Measurement_Event> rdf:type owl:Class .


###  http://www.ics.forth.gr/isl/CRMdig/D14_Software
<http://www.ics.forth.gr/isl/CRMdig/D14_Software> rdf:type owl:Class ;
    rdfs:subClassOf <http://www.ics.forth.gr/isl/CRMdig/D1_Digital_Object> ;
    rdfs:comment "A computer program."@en ;
    rdfs:isDefinedBy <http://www.ics.forth.gr/isl/CRMdig/> ;
    <http://purl.org/vocab/vann/example> """

        ### Example of a graphics software (aat:300426696)

        ex:3df-zephyr a crmdig:D14_Software ;
            crm:P2_has_type aat:300426696 .

    """@en ;
    <http://www.w3.org/2003/06/sw-vocab-status/ns#term_status> <http://purl.org/linked-data/registry#statusStable> ;
    <http://www.linkedmodel.org/schema/vaem#rationale> "This class is used to represent the software used to carry out software activities during the digitisation process."@en ;        
    rdfs:label "Software"@en .


###  http://www.ics.forth.gr/isl/CRMdig/D1_Digital_Object
<http://www.ics.forth.gr/isl/CRMdig/D1_Digital_Object> rdf:type owl:Class .


###  http://www.ics.forth.gr/isl/CRMdig/D2_Digitization_Process
<http://www.ics.forth.gr/isl/CRMdig/D2_Digitization_Process> rdf:type owl:Class ;
    rdfs:subClassOf <http://www.ics.forth.gr/isl/CRMdig/D11_Digital_Measurement_Event> ;
    rdfs:comment "An activity that results in the production of data objects functioning as digital representations of physical entities."@en ;
    rdfs:isDefinedBy <http://www.ics.forth.gr/isl/CRMdig/> ;
    <http://purl.org/vocab/vann/example> """

        ### Example of an acquisition activity that digitises a CHO at
        ### the Item level (ex:32-item) and produces a DCHO as a result 
        ### (ex:32-model-00), being carried out by an expert (ex:alice-bordignon)
        ### during a given time-span (ex:32-acquisition-timespan), using a
        ### certain technique such as photogrammetry (aat:300391312) with the
        ### help of a given tool (ex:panasonic-dmc-lx100).

        ex:32-acquisition a crmdig:D2_Digitization_Process ;
            crmdig:L1_digitized ex:32-item ;
            crmdig:L11_had_output ex:32-model-00 ;
            crm:P4_has_time-span ex:32-acquisition-timespan ;
            crm:P11_had_participant ex:unibo-ficlit ;
            crm:P14_carried_out_by ex:alice-bordignon ;
            crm:P32_used_general_technique aat:300391312 ;
            crm:P16_used_specific_object ex:panasonic-dmc-lx100 .

    """@en ;
    <http://www.w3.org/2003/06/sw-vocab-status/ns#term_status> <http://purl.org/linked-data/registry#statusStable> ;
    <http://www.linkedmodel.org/schema/vaem#rationale> "This class is used to represent the acquisition activity that kickstarts the digitisation process. An acquisition activity should at least be associated with the CHO it digitises and its output (the raw DCHO), as well as its time-span, the actors involved in it, and both the technique and the tool(s) used to carry it out."@en ;        
    rdfs:label "Digitization Process"@en .


###  http://www.ics.forth.gr/isl/CRMdig/D7_Digital_Machine_Event
<http://www.ics.forth.gr/isl/CRMdig/D7_Digital_Machine_Event> rdf:type owl:Class .


###  http://www.ics.forth.gr/isl/CRMdig/D8_Digital_Device
<http://www.ics.forth.gr/isl/CRMdig/D8_Digital_Device> rdf:type owl:Class ;
    rdfs:subClassOf <http://www.cidoc-crm.org/cidoc-crm/E22_Man-Made_Object> ;
    rdfs:comment "A technical tool that is used to process or produce digital objects."@en ;
    rdfs:isDefinedBy <http://www.ics.forth.gr/isl/CRMdig/> ;
    <http://purl.org/vocab/vann/example> """

        ### Example of a digital camera (aat:300266792)

        ex:panasonic-dmc-lx100 a crmdig:D8_Digital_Device ;
            crm:P2_has_type aat:300266792 .

    """@en ;
    <http://www.w3.org/2003/06/sw-vocab-status/ns#term_status> <http://purl.org/linked-data/registry#statusStable> ;
    <http://www.linkedmodel.org/schema/vaem#rationale> "This class is used to represent the tools used to carry out acquisition activities. A digital device should at least be typified through the combination of crm:P2_has_type and AAT."@en ;        
    rdfs:label "Digital Device"@en .


###  http://www.ics.forth.gr/isl/CRMdig/D9_Data_Object
<http://www.ics.forth.gr/isl/CRMdig/D9_Data_Object> rdf:type owl:Class ;
    rdfs:subClassOf <http://www.cidoc-crm.org/cidoc-crm/E54_Dimension> ,
        <http://www.ics.forth.gr/isl/CRMdig/D1_Digital_Object> ;
    rdfs:comment "A digital object that is the direct result of an activity in a digitization workflow."@en ;
    rdfs:isDefinedBy <http://www.ics.forth.gr/isl/CRMdig/> ;
    <http://www.w3.org/2003/06/sw-vocab-status/ns#term_status> <http://purl.org/linked-data/registry#statusStable> ;
    <http://www.linkedmodel.org/schema/vaem#rationale> "This class is used to represent the DCHO produced at the end of each digitisation activity."@en ;
    rdfs:label "Data Object"@en .


#################################################################
#    Individuals
#################################################################

###  http://vocab.getty.edu/aat/300054277
<http://vocab.getty.edu/aat/300054277> rdf:type owl:NamedIndividual ,
        <http://vocab.getty.edu/aat/Concept> ;
    <http://purl.org/dc/elements/1.1/identifier> "300054277" ;
    rdfs:comment "Superintending or managing the collections, exhibitions, research activities, and personnel of a museum, art gallery, zoo, or other place of exhibit; also, the superintending or managing of a single collection."@en ;
    rdfs:isDefinedBy <http://vocab.getty.edu/aat/> ;
    rdfs:label "curating"@en ;
    <http://www.w3.org/2004/02/skos/core#inScheme> <http://vocab.getty.edu/aat/> .


###  http://vocab.getty.edu/aat/300025976
<http://vocab.getty.edu/aat/300025976> rdf:type owl:NamedIndividual ,
        <http://vocab.getty.edu/aat/Concept> ;
    <http://purl.org/dc/elements/1.1/identifier> "300025976" ;
    rdfs:comment "Accumulated groups of objects or materials having a focal characteristic and that have been brought together by an individual or organization."@en ;
    rdfs:isDefinedBy <http://vocab.getty.edu/aat/> ;
    rdfs:label "collections (object groupings)"@en ;
    <http://www.w3.org/2004/02/skos/core#inScheme> <http://vocab.getty.edu/aat/> .


###  http://vocab.getty.edu/aat/300404126
<http://vocab.getty.edu/aat/300404126> rdf:type owl:NamedIndividual ,
        <http://vocab.getty.edu/aat/Concept> ;
    <http://purl.org/dc/elements/1.1/identifier> "300404126" ;
    rdfs:comment "In the visual arts, oral works, music, performing arts, and literature, the topics, themes, or other visual, oral, or written content of the work. It includes what the work is of or about."@en ;
    rdfs:isDefinedBy <http://vocab.getty.edu/aat/> ;
    rdfs:label "subjects (content of works)"@en ;
    <http://www.w3.org/2004/02/skos/core#inScheme> <http://vocab.getty.edu/aat/> .


###  http://vocab.getty.edu/aat/300011172
<http://vocab.getty.edu/aat/300011172> rdf:type owl:NamedIndividual ,
        <http://vocab.getty.edu/aat/Concept> ;
    <http://purl.org/dc/elements/1.1/identifier> "300011172" ;
    rdfs:comment "Works comprising precious or semiprecious stones or other materials such as amber or pearl, cut, polished, or otherwise dressed for ornamental purposes to be used in jewelry, seals, or amulets."@en ;
    rdfs:isDefinedBy <http://vocab.getty.edu/aat/> ;
    rdfs:label "gems (worked stones)"@en ;
    <http://www.w3.org/2004/02/skos/core#inScheme> <http://vocab.getty.edu/aat/> .


###  http://vocab.getty.edu/aat/300022488
<http://vocab.getty.edu/aat/300022488> rdf:type owl:NamedIndividual ,
            <http://vocab.getty.edu/aat/Concept> ;
    <http://purl.org/dc/elements/1.1/identifier> "300022488" ;
    rdfs:comment "Instruments for drawing circles and measuring the distance between two points."@en ;
    rdfs:isDefinedBy <http://vocab.getty.edu/aat/> ;
    rdfs:label "compasses (drawing instruments)"@en ;
    <http://www.w3.org/2004/02/skos/core#inScheme> <http://vocab.getty.edu/aat/> .


###  http://vocab.getty.edu/aat/300024594
<http://vocab.getty.edu/aat/300024594> rdf:type owl:NamedIndividual ,
            <http://vocab.getty.edu/aat/Concept> ;
    <http://purl.org/dc/elements/1.1/identifier> "300024594" ;
    rdfs:comment "Optical instruments consisting of a lens or combination of lenses that allow the viewing of objects that are too small to be seen with the naked, unaided eye."@en ;
    rdfs:isDefinedBy <http://vocab.getty.edu/aat/> ;
    rdfs:label "microscopes"@en ;
    <http://www.w3.org/2004/02/skos/core#inScheme> <http://vocab.getty.edu/aat/> .


###  http://vocab.getty.edu/aat/300024814
<http://vocab.getty.edu/aat/300024814> rdf:type owl:NamedIndividual ,
            <http://vocab.getty.edu/aat/Concept> ;
    <http://purl.org/dc/elements/1.1/identifier> "300024814" ;
    rdfs:comment "Hollow forms in which castings or pressings are made; used with many materials, including clay, metal, glass, and paper."@en ;
    rdfs:isDefinedBy <http://vocab.getty.edu/aat/> ;
    rdfs:label "molds (shaping equipment)"@en ;
    <http://www.w3.org/2004/02/skos/core#inScheme> <http://vocab.getty.edu/aat/> .


###  http://vocab.getty.edu/aat/300024928
<http://vocab.getty.edu/aat/300024928> rdf:type owl:NamedIndividual ,
            <http://vocab.getty.edu/aat/Concept> ;
    <http://purl.org/dc/elements/1.1/identifier> "300024928" ;
    rdfs:comment "Tool handles, such as those of axes, hatchets, or hammers."@en ;
    rdfs:isDefinedBy <http://vocab.getty.edu/aat/> ;
    rdfs:label "helves"@en ;
    <http://www.w3.org/2004/02/skos/core#inScheme> <http://vocab.getty.edu/aat/> .


###  http://vocab.getty.edu/aat/300027349
<http://vocab.getty.edu/aat/300027349> rdf:type owl:NamedIndividual ,
            <http://vocab.getty.edu/aat/Concept> ;
    <http://purl.org/dc/elements/1.1/identifier> "300027349" ;
    rdfs:comment "A conceptual grouping of visual arts works, literary works, or performance art created in succession by the same author, artist, or studio and intended by the creator(s) to be seen together."@en ;
    rdfs:isDefinedBy <http://vocab.getty.edu/aat/> ;
    rdfs:label "series (object groupings)"@en ;
    <http://www.w3.org/2004/02/skos/core#inScheme> <http://vocab.getty.edu/aat/> .


###  http://vocab.getty.edu/aat/300028051
<http://vocab.getty.edu/aat/300028051> rdf:type owl:NamedIndividual ,
            <http://vocab.getty.edu/aat/Concept> ;
    <http://purl.org/dc/elements/1.1/identifier> "300028051" ;
    rdfs:comment "Items comprising a collection of leaves of paper, parchment, wood, stiffened textile, ivory, metal tablets, or other flat material, that are blank, written on, or printed, and are strung or bound together."@en ;
    rdfs:isDefinedBy <http://vocab.getty.edu/aat/> ;
    rdfs:label "books"@en ;
    <http://www.w3.org/2004/02/skos/core#inScheme> <http://vocab.getty.edu/aat/> .


###  http://vocab.getty.edu/aat/300028094
<http://vocab.getty.edu/aat/300028094> rdf:type owl:NamedIndividual ,
            <http://vocab.getty.edu/aat/Concept> ;
    <http://purl.org/dc/elements/1.1/identifier> "300028094" ;
    rdfs:comment "Refers to graphic or photogrammetric representations of the Earth's surface or a part of it, including physical features and political boundaries."@en ;
    rdfs:isDefinedBy <http://vocab.getty.edu/aat/> ;
    rdfs:label "maps (documents)"@en ;
    <http://www.w3.org/2004/02/skos/core#inScheme> <http://vocab.getty.edu/aat/> .


###  http://vocab.getty.edu/aat/300028309
<http://vocab.getty.edu/aat/300028309> rdf:type owl:NamedIndividual ,
            <http://vocab.getty.edu/aat/Concept> ;
    <http://purl.org/dc/elements/1.1/identifier> "300028309" ;
    rdfs:comment "Maps designed and used primarily for plotting courses and traveling on water in a ship or other vessel or in an aircraft or spacecraft."@en ;
    rdfs:isDefinedBy <http://vocab.getty.edu/aat/> ;
    rdfs:label "navigation charts"@en ;
    <http://www.w3.org/2004/02/skos/core#inScheme> <http://vocab.getty.edu/aat/> .


###  http://vocab.getty.edu/aat/300028569
<http://vocab.getty.edu/aat/300028569> rdf:type owl:NamedIndividual ,
            <http://vocab.getty.edu/aat/Concept> ;
    <http://purl.org/dc/elements/1.1/identifier> "300028569" ;
    rdfs:comment "Handwritten documents, particularly books and other documents created before the invention of the printing press."@en ;
    rdfs:isDefinedBy <http://vocab.getty.edu/aat/> ;
    rdfs:label "manuscripts (documents)"@en ;
    <http://www.w3.org/2004/02/skos/core#inScheme> <http://vocab.getty.edu/aat/> .


###  http://vocab.getty.edu/aat/300028682
<http://vocab.getty.edu/aat/300028682> rdf:type owl:NamedIndividual ,
            <http://vocab.getty.edu/aat/Concept> ;
    <http://purl.org/dc/elements/1.1/identifier> "300028682" ;
    rdfs:comment "Manifestations of motion pictures, stored electronically, in any media or digitized format."@en ;
    rdfs:isDefinedBy <http://vocab.getty.edu/aat/> ;
    rdfs:label "video recordings (physical artifacts)"@en ;
    <http://www.w3.org/2004/02/skos/core#inScheme> <http://vocab.getty.edu/aat/> .


###  http://vocab.getty.edu/aat/300033618
<http://vocab.getty.edu/aat/300033618> rdf:type owl:NamedIndividual ,
            <http://vocab.getty.edu/aat/Concept> ;
    <http://purl.org/dc/elements/1.1/identifier> "300033618" ;
    rdfs:comment "Unique works in which images are formed primarily by the direct application of pigments suspended in oil, water, egg yolk, molten wax, or other liquid, arranged in masses of color, onto a general surface."@en ;
    rdfs:isDefinedBy <http://vocab.getty.edu/aat/> ;
    rdfs:label "paintings (visual works)"@en ;
    <http://www.w3.org/2004/02/skos/core#inScheme> <http://vocab.getty.edu/aat/> .


###  http://vocab.getty.edu/aat/300015045
<http://vocab.getty.edu/aat/300015045> rdf:type owl:NamedIndividual ,
            <http://vocab.getty.edu/aat/Concept> ;
    <http://purl.org/dc/elements/1.1/identifier> "300015045" ;
    rdfs:comment "Transparent aqueous based paint produced by mixing ground pigments with water and, generally, gum arabic."@en ;
    rdfs:isDefinedBy <http://vocab.getty.edu/aat/> ;
    rdfs:label "watercolor (paint)"@en ;
    <http://www.w3.org/2004/02/skos/core#inScheme> <http://vocab.getty.edu/aat/> .


###  http://vocab.getty.edu/aat/300178684
<http://vocab.getty.edu/aat/300178684> rdf:type owl:NamedIndividual ,
            <http://vocab.getty.edu/aat/Concept> ;
    <http://purl.org/dc/elements/1.1/identifier> "300178684" ;
    rdfs:comment "The art or practice of producing creative works in oil paint, which is pigment suspended in vegetal drying oils."@en ;
    rdfs:isDefinedBy <http://vocab.getty.edu/aat/> ;
    rdfs:label "oil painting (technique)"@en ;
    <http://www.w3.org/2004/02/skos/core#inScheme> <http://vocab.getty.edu/aat/> .


###  http://vocab.getty.edu/aat/300053319
<http://vocab.getty.edu/aat/300053319> rdf:type owl:NamedIndividual ,
            <http://vocab.getty.edu/aat/Concept> ;
    <http://purl.org/dc/elements/1.1/identifier> "300053319" ;
    rdfs:comment "Various means of reproducing identical copies of graphic matter in a fixed form, by which an image, pictorial or textual, is transferred, usually to paper or cloth."@en ;
    rdfs:isDefinedBy <http://vocab.getty.edu/aat/> ;
    rdfs:label "printing (process)"@en ;
    <http://www.w3.org/2004/02/skos/core#inScheme> <http://vocab.getty.edu/aat/> .


###  http://vocab.getty.edu/aat/300037592
<http://vocab.getty.edu/aat/300037592> rdf:type owl:NamedIndividual ,
            <http://vocab.getty.edu/aat/Concept> ;
    <http://purl.org/dc/elements/1.1/identifier> "300037592" ;
    rdfs:comment "Lighting devices having a vessel to contain fuel used as a source of illumination, such as grease or oil."@en ;
    rdfs:isDefinedBy <http://vocab.getty.edu/aat/> ;
    rdfs:label "lamps (lighting devices)"@en ;
    <http://www.w3.org/2004/02/skos/core#inScheme> <http://vocab.getty.edu/aat/> .


###  http://vocab.getty.edu/aat/300041273
<http://vocab.getty.edu/aat/300041273> rdf:type owl:NamedIndividual ,
            <http://vocab.getty.edu/aat/Concept> ;
    <http://purl.org/dc/elements/1.1/identifier> "300041273" ;
    rdfs:comment "Pictorial works produced by transferring images by means of a matrix such as a plate, block, or screen, using any of various printing processes."@en ;
    rdfs:isDefinedBy <http://vocab.getty.edu/aat/> ;
    rdfs:label "prints (visual works)"@en ;
    <http://www.w3.org/2004/02/skos/core#inScheme> <http://vocab.getty.edu/aat/> .


###  http://vocab.getty.edu/aat/300041340
<http://vocab.getty.edu/aat/300041340> rdf:type owl:NamedIndividual ,
            <http://vocab.getty.edu/aat/Concept> ;
    <http://purl.org/dc/elements/1.1/identifier> "300041340" ;
    rdfs:comment "Prints on paper incorporating impressions of a reverse design created on a printing plate, usually copper, into which the design has been incised (engraved) using burins or gravers."@en ;
    rdfs:isDefinedBy <http://vocab.getty.edu/aat/> ;
    rdfs:label "engravings (prints)"@en ;
    <http://www.w3.org/2004/02/skos/core#inScheme> <http://vocab.getty.edu/aat/> .


###  http://vocab.getty.edu/aat/300041405
<http://vocab.getty.edu/aat/300041405> rdf:type owl:NamedIndividual ,
            <http://vocab.getty.edu/aat/Concept> ;
    <http://purl.org/dc/elements/1.1/identifier> "300041405" ;
    rdfs:comment "Prints made using the process of woodcut, which is a relief process in which the design is cut into and printed from the plank side of a wood block."@en ;
    rdfs:isDefinedBy <http://vocab.getty.edu/aat/> ;
    rdfs:label "woodcuts (prints)"@en ;
    <http://www.w3.org/2004/02/skos/core#inScheme> <http://vocab.getty.edu/aat/> .


###  http://vocab.getty.edu/aat/300041933
<http://vocab.getty.edu/aat/300041933> rdf:type owl:NamedIndividual ,
            <http://vocab.getty.edu/aat/Concept> ;
    <http://purl.org/dc/elements/1.1/identifier> "300041933" ;
    rdfs:comment "Shaken idiophones made in a variety of forms worldwide, in which one or more objects strike against each other or against the inside or outside of another object."@en ;
    rdfs:isDefinedBy <http://vocab.getty.edu/aat/> ;
    rdfs:label "rattles (indirectly struck idiophones)"@en ;
    <http://www.w3.org/2004/02/skos/core#inScheme> <http://vocab.getty.edu/aat/> .


###  http://vocab.getty.edu/aat/300045627
<http://vocab.getty.edu/aat/300045627> rdf:type owl:NamedIndividual ,
            <http://vocab.getty.edu/aat/Concept> ;
    <http://purl.org/dc/elements/1.1/identifier> "300045627" ;
    rdfs:comment "Vessels having a neck and mouth considerably narrower than the body, used for packaging and containing liquid and dry preparations."@en ;
    rdfs:isDefinedBy <http://vocab.getty.edu/aat/> ;
    rdfs:label "bottles"@en ;
    <http://www.w3.org/2004/02/skos/core#inScheme> <http://vocab.getty.edu/aat/> .


###  http://vocab.getty.edu/aat/300046001
<http://vocab.getty.edu/aat/300046001> rdf:type owl:NamedIndividual ,
            <http://vocab.getty.edu/aat/Concept> ;
    <http://purl.org/dc/elements/1.1/identifier> "300046001" ;
    rdfs:comment "Ornaments worn around the neck, usually in the form of chains or strands of beads, pearls, stones, or decorative or precious materials, and often including a suspended ornamental pendant."@en ;
    rdfs:isDefinedBy <http://vocab.getty.edu/aat/> ;
    rdfs:label "necklaces"@en ;
    <http://www.w3.org/2004/02/skos/core#inScheme> <http://vocab.getty.edu/aat/> .


###  http://vocab.getty.edu/aat/300046025
<http://vocab.getty.edu/aat/300046025> rdf:type owl:NamedIndividual ,
            <http://vocab.getty.edu/aat/Concept> ;
    <http://purl.org/dc/elements/1.1/identifier> "300046025" ;
    rdfs:comment "Small pieces of metal, usually gold, silver, or bronze and bearing a relief design on one or both sides and having a commemorative purpose."@en ;
    rdfs:isDefinedBy <http://vocab.getty.edu/aat/> ;
    rdfs:label "medals"@en ;
    <http://www.w3.org/2004/02/skos/core#inScheme> <http://vocab.getty.edu/aat/> .


###  http://vocab.getty.edu/aat/300047600
<http://vocab.getty.edu/aat/300047600> rdf:type owl:NamedIndividual ,
            <http://vocab.getty.edu/aat/Concept> ;
    <http://purl.org/dc/elements/1.1/identifier> "300047600" ;
    rdfs:comment "Sculpture in the round, usually but not always depicting humans, animals, mythical beings, or small figure groups."@en ;
    rdfs:isDefinedBy <http://vocab.getty.edu/aat/> ;
    rdfs:label "statues"@en ;
    <http://www.w3.org/2004/02/skos/core#inScheme> <http://vocab.getty.edu/aat/> .


###  http://vocab.getty.edu/aat/300047753
<http://vocab.getty.edu/aat/300047753> rdf:type owl:NamedIndividual ,
            <http://vocab.getty.edu/aat/Concept> ;
    <http://purl.org/dc/elements/1.1/identifier> "300047753" ;
    rdfs:comment "Refers to scaled or lifesize representations of objects, structures, beings, or other subjects, usually three-dimensional."@en ;
    rdfs:isDefinedBy <http://vocab.getty.edu/aat/> ;
    rdfs:label "models (representations)"@en ;
    <http://www.w3.org/2004/02/skos/core#inScheme> <http://vocab.getty.edu/aat/> .


###  http://vocab.getty.edu/aat/300047762
<http://vocab.getty.edu/aat/300047762> rdf:type owl:NamedIndividual ,
            <http://vocab.getty.edu/aat/Concept> ;
    <http://purl.org/dc/elements/1.1/identifier> "300047762" ;
    rdfs:comment "Works in which three-dimensional objects, often figural sculpture, in the foreground blend with a realistic painted background."@en ;
    rdfs:isDefinedBy <http://vocab.getty.edu/aat/> ;
    rdfs:label "dioramas"@en ;
    <http://www.w3.org/2004/02/skos/core#inScheme> <http://vocab.getty.edu/aat/> .


###  http://vocab.getty.edu/aat/300053225
<http://vocab.getty.edu/aat/300053225> rdf:type owl:NamedIndividual ,
            <http://vocab.getty.edu/aat/Concept> ;
    <http://purl.org/dc/elements/1.1/identifier> "300053225" ;
    rdfs:comment "The intaglio process in which the design is incised into a printing plate, usually a flat copper plate, with the aid of a graver or burin."@en ;
    rdfs:isDefinedBy <http://vocab.getty.edu/aat/> ;
    rdfs:label "engraving (printing process)"@en ;
    <http://www.w3.org/2004/02/skos/core#inScheme> <http://vocab.getty.edu/aat/> .


###  http://vocab.getty.edu/aat/300053357
<http://vocab.getty.edu/aat/300053357> rdf:type owl:NamedIndividual ,
            <http://vocab.getty.edu/aat/Concept> ;
    <http://purl.org/dc/elements/1.1/identifier> "300053357" ;
    rdfs:comment "Mural painting technique in which dry pigments are ground with water then brushed onto wet or partially dry lime plaster."@en ;
    rdfs:isDefinedBy <http://vocab.getty.edu/aat/> ;
    rdfs:label "fresco painting (technique)"@en ;
    <http://www.w3.org/2004/02/skos/core#inScheme> <http://vocab.getty.edu/aat/> .


###  http://vocab.getty.edu/aat/300053363
<http://vocab.getty.edu/aat/300053363> rdf:type owl:NamedIndividual ,
            <http://vocab.getty.edu/aat/Concept> ;
    <http://purl.org/dc/elements/1.1/identifier> "300053363" ;
    rdfs:comment "Watercolor painting done in transparent washes of color as distinguished from the opaque method using gouache."@en ;
    rdfs:isDefinedBy <http://vocab.getty.edu/aat/> ;
    rdfs:label "aquarelle (technique)"@en ;
    <http://www.w3.org/2004/02/skos/core#inScheme> <http://vocab.getty.edu/aat/> .


###  http://vocab.getty.edu/aat/300053580
<http://vocab.getty.edu/aat/300053580> rdf:type owl:NamedIndividual ,
            <http://vocab.getty.edu/aat/Concept> ;
    <http://purl.org/dc/elements/1.1/identifier> "300053580" ;
    rdfs:comment "Refers to the technique of making measurements by using photography. It usually refers to this technique as applied to mapmaking, measuring site elements, and surveying."@en ;
    rdfs:isDefinedBy <http://vocab.getty.edu/aat/> ;
    rdfs:label "photogrammetry"@en ;
    <http://www.w3.org/2004/02/skos/core#inScheme> <http://vocab.getty.edu/aat/> .


###  http://vocab.getty.edu/aat/300053628
<http://vocab.getty.edu/aat/300053628> rdf:type owl:NamedIndividual ,
            <http://vocab.getty.edu/aat/Concept> ;
    <http://purl.org/dc/elements/1.1/identifier> "300053628" ;
    rdfs:comment "Preparing lifelike representations of animals by stuffing the skin or molding it around a model of the specimen."@en ;
    rdfs:isDefinedBy <http://vocab.getty.edu/aat/> ;
    rdfs:label "taxidermy"@en ;
    <http://www.w3.org/2004/02/skos/core#inScheme> <http://vocab.getty.edu/aat/> .


###  http://vocab.getty.edu/aat/300053758
<http://vocab.getty.edu/aat/300053758> rdf:type owl:NamedIndividual ,
            <http://vocab.getty.edu/aat/Concept> ;
    <http://purl.org/dc/elements/1.1/identifier> "300053758" ;
    rdfs:comment "Making free or nearly free of liquids."@en ;
    rdfs:isDefinedBy <http://vocab.getty.edu/aat/> ;
    rdfs:label "drying"@en ;
    <http://www.w3.org/2004/02/skos/core#inScheme> <http://vocab.getty.edu/aat/> .


###  http://vocab.getty.edu/aat/300053852
<http://vocab.getty.edu/aat/300053852> rdf:type owl:NamedIndividual ,
            <http://vocab.getty.edu/aat/Concept> ;
    <http://purl.org/dc/elements/1.1/identifier> "300053852" ;
    rdfs:comment "Decorative wood process in which the design or pattern is made by assembling small pieces of veneer in various shapes."@en ;
    rdfs:isDefinedBy <http://vocab.getty.edu/aat/> ;
    rdfs:label "intarsia (process)"@en ;
    <http://www.w3.org/2004/02/skos/core#inScheme> <http://vocab.getty.edu/aat/> .


###  http://vocab.getty.edu/aat/300054196
<http://vocab.getty.edu/aat/300054196> rdf:type owl:NamedIndividual ,
            <http://vocab.getty.edu/aat/Concept> ;
    <http://purl.org/dc/elements/1.1/identifier> "300054196" ;
    rdfs:comment "Producing visible forms primarily by delineation, usually by the direct application of material or instrument to the surface of the support."@en ;
    rdfs:isDefinedBy <http://vocab.getty.edu/aat/> ;
    rdfs:label "drawing (image-making)"@en ;
    <http://www.w3.org/2004/02/skos/core#inScheme> <http://vocab.getty.edu/aat/> .


###  http://vocab.getty.edu/aat/300054200
<http://vocab.getty.edu/aat/300054200> rdf:type owl:NamedIndividual ,
            <http://vocab.getty.edu/aat/Concept> ;
    <http://purl.org/dc/elements/1.1/identifier> "300054200" ;
    rdfs:comment "The art or process of providing drawings or other pictures intended to elucidate a description, story, or other written material, usually in a book or periodical."@en ;
    rdfs:isDefinedBy <http://vocab.getty.edu/aat/> ;
    rdfs:label "illustration (process)"@en ;
    <http://www.w3.org/2004/02/skos/core#inScheme> <http://vocab.getty.edu/aat/> .


###  http://vocab.getty.edu/aat/300054636
<http://vocab.getty.edu/aat/300054636> rdf:type owl:NamedIndividual ,
            <http://vocab.getty.edu/aat/Concept> ;
    <http://purl.org/dc/elements/1.1/identifier> "300054636" ;
    rdfs:comment "Creating and manipulating data in machine-readable form by means of computers, including inputting, storage, conversion, editing, and printing."@en ;
    rdfs:isDefinedBy <http://vocab.getty.edu/aat/> ;
    rdfs:label "data processing"@en ;
    <http://www.w3.org/2004/02/skos/core#inScheme> <http://vocab.getty.edu/aat/> .


###  http://vocab.getty.edu/aat/300054638
<http://vocab.getty.edu/aat/300054638> rdf:type owl:NamedIndividual ,
            <http://vocab.getty.edu/aat/Concept> ;
    <http://purl.org/dc/elements/1.1/identifier> "300054638" ;
    rdfs:comment "The process or function of gathering and recording information, especially to record facts or characteristics or to establish evidence or testimony."@en ;
    rdfs:isDefinedBy <http://vocab.getty.edu/aat/> ;
    rdfs:label "documentation (activity)"@en ;
    <http://www.w3.org/2004/02/skos/core#inScheme> <http://vocab.getty.edu/aat/> .


###  http://vocab.getty.edu/aat/300054686
<http://vocab.getty.edu/aat/300054686> rdf:type owl:NamedIndividual ,
            <http://vocab.getty.edu/aat/Concept> ;
    <http://purl.org/dc/elements/1.1/identifier> "300054686" ;
    rdfs:comment "The actions, functions, or event of issuing printed, taped, or otherwise reproduced records of knowledge or visual works in any medium for sale or distribution to the public."@en ;
    rdfs:isDefinedBy <http://vocab.getty.edu/aat/> ;
    rdfs:label "publishing"@en ;
    <http://www.w3.org/2004/02/skos/core#inScheme> <http://vocab.getty.edu/aat/> .


###  http://vocab.getty.edu/aat/300404387
<http://vocab.getty.edu/aat/300404387> rdf:type owl:NamedIndividual ,
            <http://vocab.getty.edu/aat/Concept> ;
    <http://purl.org/dc/elements/1.1/identifier> "300404387" ;
    rdfs:comment "The activities surrounding the production or conception of a work, particularly a work of visual art, literary art, or performing arts."@en ;
    rdfs:isDefinedBy <http://vocab.getty.edu/aat/> ;
    rdfs:label "creating (artistic activity)"@en ;
    <http://www.w3.org/2004/02/skos/core#inScheme> <http://vocab.getty.edu/aat/> .


###  http://vocab.getty.edu/aat/300055021
<http://vocab.getty.edu/aat/300055021> rdf:type owl:NamedIndividual ,
            <http://vocab.getty.edu/aat/Concept> ;
    <http://purl.org/dc/elements/1.1/identifier> "300055021" ;
    rdfs:comment "Books printed before 1501."@en ;
    rdfs:isDefinedBy <http://vocab.getty.edu/aat/> ;
    rdfs:label "incunabula (books)"@en ;
    <http://www.w3.org/2004/02/skos/core#inScheme> <http://vocab.getty.edu/aat/> .


###  http://vocab.getty.edu/aat/300069831
<http://vocab.getty.edu/aat/300069831> rdf:type owl:NamedIndividual ,
            <http://vocab.getty.edu/aat/Concept> ;
    <http://purl.org/dc/elements/1.1/identifier> "300069831" ;
    rdfs:comment "The activity of comprehending, analyzing, and expressing written or spoken material in a different language from the original."@en ;
    rdfs:isDefinedBy <http://vocab.getty.edu/aat/> ;
    rdfs:label "translation (function)"@en ;
    <http://www.w3.org/2004/02/skos/core#inScheme> <http://vocab.getty.edu/aat/> .


###  http://vocab.getty.edu/aat/300077565
<http://vocab.getty.edu/aat/300077565> rdf:type owl:NamedIndividual ,
            <http://vocab.getty.edu/aat/Concept> ;
    <http://purl.org/dc/elements/1.1/identifier> "300077565" ;
    rdfs:comment "The action or process of making something ready for use or service or of getting ready for some occasion, test, or duty."@en ;
    rdfs:isDefinedBy <http://vocab.getty.edu/aat/> ;
    rdfs:label "preparing"@en ;
    <http://www.w3.org/2004/02/skos/core#inScheme> <http://vocab.getty.edu/aat/> .


###  http://vocab.getty.edu/aat/300117127
<http://vocab.getty.edu/aat/300117127> rdf:type owl:NamedIndividual ,
            <http://vocab.getty.edu/aat/Concept> ;
    <http://purl.org/dc/elements/1.1/identifier> "300117127" ;
    rdfs:comment "Generally, objects or other things made or modified by humans, typically manually portable products of human workmanship, such as tools, utensils, objects for personal adornment, or art."@en ;
    rdfs:isDefinedBy <http://vocab.getty.edu/aat/> ;
    rdfs:label "artifacts (object genre)"@en ;
    <http://www.w3.org/2004/02/skos/core#inScheme> <http://vocab.getty.edu/aat/> .


###  http://vocab.getty.edu/aat/300122241
<http://vocab.getty.edu/aat/300122241> rdf:type owl:NamedIndividual ,
            <http://vocab.getty.edu/aat/Concept> ;
    <http://purl.org/dc/elements/1.1/identifier> "300122241" ;
    rdfs:comment "Articles or physical resources used to array, dress up, rig out, equip, or otherwise provide with what is requisite for efficient action by a person or animal or for a thing."@en ;
    rdfs:isDefinedBy <http://vocab.getty.edu/aat/> ;
    rdfs:label "equipment"@en ;
    <http://www.w3.org/2004/02/skos/core#inScheme> <http://vocab.getty.edu/aat/> .


###  http://vocab.getty.edu/aat/300132254
<http://vocab.getty.edu/aat/300132254> rdf:type owl:NamedIndividual ,
            <http://vocab.getty.edu/aat/Concept> ;
    <http://purl.org/dc/elements/1.1/identifier> "300132254" ;
    rdfs:comment "Vessels of varying shape and size but which are usually taller than they are wide, varying greatly in actual form and use."@en ;
    rdfs:isDefinedBy <http://vocab.getty.edu/aat/> ;
    rdfs:label "vases"@en ;
    <http://www.w3.org/2004/02/skos/core#inScheme> <http://vocab.getty.edu/aat/> .


###  http://vocab.getty.edu/aat/300137376
<http://vocab.getty.edu/aat/300137376> rdf:type owl:NamedIndividual ,
            <http://vocab.getty.edu/aat/Concept> ;
    <http://purl.org/dc/elements/1.1/identifier> "300137376" ;
    rdfs:comment "Medieval marine charts, used before compasses, and for Medieval navigation manuals, illustrated with charts and showing the location of ports and other navigational information."@en ;
    rdfs:isDefinedBy <http://vocab.getty.edu/aat/> ;
    rdfs:label "portolanos"@en ;
    <http://www.w3.org/2004/02/skos/core#inScheme> <http://vocab.getty.edu/aat/> .


###  http://vocab.getty.edu/aat/300138684
<http://vocab.getty.edu/aat/300138684> rdf:type owl:NamedIndividual ,
            <http://vocab.getty.edu/aat/Concept> ;
    <http://purl.org/dc/elements/1.1/identifier> "300138684" ;
    rdfs:comment "A method of decorating surfaces with patterns or pictures composed of small, regularly-shaped pieces of colored durable material, such as stone or glass."@en ;
    rdfs:isDefinedBy <http://vocab.getty.edu/aat/> ;
    rdfs:label "mosaic (process)"@en ;
    <http://www.w3.org/2004/02/skos/core#inScheme> <http://vocab.getty.edu/aat/> .


###  http://vocab.getty.edu/aat/300138758
<http://vocab.getty.edu/aat/300138758> rdf:type owl:NamedIndividual ,
            <http://vocab.getty.edu/aat/Concept> ;
    <http://purl.org/dc/elements/1.1/identifier> "300138758" ;
    rdfs:comment "Refers to coverings for all or part of the face, usually with openings for the eyes and sometimes the mouth."@en ;
    rdfs:isDefinedBy <http://vocab.getty.edu/aat/> ;
    rdfs:label "masks (costume)"@en ;
    <http://www.w3.org/2004/02/skos/core#inScheme> <http://vocab.getty.edu/aat/> .


###  http://vocab.getty.edu/aat/300155365
<http://vocab.getty.edu/aat/300155365> rdf:type owl:NamedIndividual ,
            <http://vocab.getty.edu/aat/Concept> ;
    <http://purl.org/dc/elements/1.1/identifier> "300155365" ;
    rdfs:comment "Publishing text or images in electronic machine-readable formats."@en ;
    rdfs:isDefinedBy <http://vocab.getty.edu/aat/> ;
    rdfs:label "electronic publishing"@en ;
    <http://www.w3.org/2004/02/skos/core#inScheme> <http://vocab.getty.edu/aat/> .


###  http://vocab.getty.edu/aat/300178926
<http://vocab.getty.edu/aat/300178926> rdf:type owl:NamedIndividual ,
            <http://vocab.getty.edu/aat/Concept> ;
    <http://purl.org/dc/elements/1.1/identifier> "300178926" ;
    rdfs:comment "Printing from raised and inked type, distinguished from lithographic or intaglio printing, particularly in the context of book and other text printing."@en ;
    rdfs:isDefinedBy <http://vocab.getty.edu/aat/> ;
    rdfs:label "letterpress printing"@en ;
    <http://www.w3.org/2004/02/skos/core#inScheme> <http://vocab.getty.edu/aat/> .


###  http://vocab.getty.edu/aat/300184300
<http://vocab.getty.edu/aat/300184300> rdf:type owl:NamedIndividual ,
            <http://vocab.getty.edu/aat/Concept> ;
    <http://purl.org/dc/elements/1.1/identifier> "300184300" ;
    rdfs:comment "Refers to series of visual works depicting events and unified by a common topic, not necessarily a sequence in a single story line."@en ;
    rdfs:isDefinedBy <http://vocab.getty.edu/aat/> ;
    rdfs:label "narrative cycles"@en ;
    <http://www.w3.org/2004/02/skos/core#inScheme> <http://vocab.getty.edu/aat/> .


###  http://vocab.getty.edu/aat/300189634
<http://vocab.getty.edu/aat/300189634> rdf:type owl:NamedIndividual ,
            <http://vocab.getty.edu/aat/Concept> ;
    <http://purl.org/dc/elements/1.1/identifier> "300189634" ;
    rdfs:comment "Groups of prints related in theme or technique and usually issued together."@en ;
    rdfs:isDefinedBy <http://vocab.getty.edu/aat/> ;
    rdfs:label "suites (print groupings)"@en ;
    <http://www.w3.org/2004/02/skos/core#inScheme> <http://vocab.getty.edu/aat/> .


###  http://vocab.getty.edu/aat/300191086
<http://vocab.getty.edu/aat/300191086> rdf:type owl:NamedIndividual ,
            <http://vocab.getty.edu/aat/Concept> ;
    <http://purl.org/dc/elements/1.1/identifier> "300191086" ;
    rdfs:comment "Works of art, architecture, and any objects that occupy space, are perceived by the sense of sight, and are created or arranged, rather than naturally occurring."@en ;
    rdfs:isDefinedBy <http://vocab.getty.edu/aat/> ;
    rdfs:label "visual works (works)"@en ;
    <http://www.w3.org/2004/02/skos/core#inScheme> <http://vocab.getty.edu/aat/> .


###  http://vocab.getty.edu/aat/300224200
<http://vocab.getty.edu/aat/300224200> rdf:type owl:NamedIndividual ,
            <http://vocab.getty.edu/aat/Concept> ;
    <http://purl.org/dc/elements/1.1/identifier> "300224200" ;
    rdfs:comment "Ancient manuscripts generally taking the form of the modern book: bound leaves of paper or parchment with information inscribed on both faces, attached at a center fold."@en ;
    rdfs:isDefinedBy <http://vocab.getty.edu/aat/> ;
    rdfs:label "codices (bound manuscripts)"@en ;
    <http://www.w3.org/2004/02/skos/core#inScheme> <http://vocab.getty.edu/aat/> .


###  http://vocab.getty.edu/aat/300226836
<http://vocab.getty.edu/aat/300226836> rdf:type owl:NamedIndividual ,
            <http://vocab.getty.edu/aat/Concept> ;
    <http://purl.org/dc/elements/1.1/identifier> "300226836" ;
    rdfs:comment "Sets or ensembles of visual works."@en ;
    rdfs:isDefinedBy <http://vocab.getty.edu/aat/> ;
    rdfs:label "visual works groupings"@en ;
    <http://www.w3.org/2004/02/skos/core#inScheme> <http://vocab.getty.edu/aat/> .


###  http://vocab.getty.edu/aat/300235576
<http://vocab.getty.edu/aat/300235576> rdf:type owl:NamedIndividual ,
            <http://vocab.getty.edu/aat/Concept> ;
    <http://purl.org/dc/elements/1.1/identifier> "300235576" ;
    rdfs:comment "A specimen is an individual instance that represents a class. A good specimen shows the character of the thing or material, useful for close study and permitting exact identification."@en ;
    rdfs:isDefinedBy <http://vocab.getty.edu/aat/> ;
    rdfs:label "specimens"@en ;
    <http://www.w3.org/2004/02/skos/core#inScheme> <http://vocab.getty.edu/aat/> .


###  http://vocab.getty.edu/aat/300252927
<http://vocab.getty.edu/aat/300252927> rdf:type owl:NamedIndividual ,
            <http://vocab.getty.edu/aat/Concept> ;
    <http://purl.org/dc/elements/1.1/identifier> "300252927" ;
    rdfs:comment "The forming of letters and words by hand rather than by printing; may be used to designate a particular and distinctive form, style, or method of writing by hand."@en ;
    rdfs:isDefinedBy <http://vocab.getty.edu/aat/> ;
    rdfs:label "handwriting"@en ;
    <http://www.w3.org/2004/02/skos/core#inScheme> <http://vocab.getty.edu/aat/> .


###  http://vocab.getty.edu/aat/300264383
<http://vocab.getty.edu/aat/300264383> rdf:type owl:NamedIndividual ,
            <http://vocab.getty.edu/aat/Concept> ;
    <http://purl.org/dc/elements/1.1/identifier> "300264383" ;
    rdfs:comment "Refers to the process or branch of fine art concerned with creating sculpture, which are three-dimensional works."@en ;
    rdfs:isDefinedBy <http://vocab.getty.edu/aat/> ;
    rdfs:label "sculpting"@en ;
    <http://www.w3.org/2004/02/skos/core#inScheme> <http://vocab.getty.edu/aat/> .


###  http://vocab.getty.edu/aat/300265248
<http://vocab.getty.edu/aat/300265248> rdf:type owl:NamedIndividual ,
            <http://vocab.getty.edu/aat/Concept> ;
    <http://purl.org/dc/elements/1.1/identifier> "300265248" ;
    rdfs:comment "Any technique for forming or shaping wax into sculptural shapes, either for casting purposes or as a final work."@en ;
    rdfs:isDefinedBy <http://vocab.getty.edu/aat/> ;
    rdfs:label "wax-modeling"@en ;
    <http://www.w3.org/2004/02/skos/core#inScheme> <http://vocab.getty.edu/aat/> .


###  http://vocab.getty.edu/aat/300265483
<http://vocab.getty.edu/aat/300265483> rdf:type owl:NamedIndividual ,
            <http://vocab.getty.edu/aat/Concept> ;
    <http://purl.org/dc/elements/1.1/identifier> "300265483" ;
    rdfs:comment "Handwritten manuscripts that have been decorated with gold or silver, brilliant colors, designs, or miniature pictures."@en ;
    rdfs:isDefinedBy <http://vocab.getty.edu/aat/> ;
    rdfs:label "illuminated manuscripts"@en ;
    <http://www.w3.org/2004/02/skos/core#inScheme> <http://vocab.getty.edu/aat/> .


###  http://vocab.getty.edu/aat/300265632
<http://vocab.getty.edu/aat/300265632> rdf:type owl:NamedIndividual ,
            <http://vocab.getty.edu/aat/Concept> ;
    <http://purl.org/dc/elements/1.1/identifier> "300265632" ;
    rdfs:comment "Objects comprising sheets of paper, vellum, papyrus, or another material that are bound together. Volumes may include printed books, manuscripts, sketchbooks, or albums."@en ;
    rdfs:isDefinedBy <http://vocab.getty.edu/aat/> ;
    rdfs:label "volumes (documents by form)"@en ;
    <http://www.w3.org/2004/02/skos/core#inScheme> <http://vocab.getty.edu/aat/> .


###  http://vocab.getty.edu/aat/300266792
<http://vocab.getty.edu/aat/300266792> rdf:type owl:NamedIndividual ,
            <http://vocab.getty.edu/aat/Concept> ;
    <http://purl.org/dc/elements/1.1/identifier> "300266792" ;
    rdfs:comment "Cameras capable of acquiring still or motion pictures via an electronic sensor and storing them as digital information on a memory device."@en ;
    rdfs:isDefinedBy <http://vocab.getty.edu/aat/> ;
    rdfs:label "digital cameras"@en ;
    <http://www.w3.org/2004/02/skos/core#inScheme> <http://vocab.getty.edu/aat/> .


###  http://vocab.getty.edu/aat/300312355
<http://vocab.getty.edu/aat/300312355> rdf:type owl:NamedIndividual ,
            <http://vocab.getty.edu/aat/Concept> ;
    <http://purl.org/dc/elements/1.1/identifier> "300312355" ;
    rdfs:comment "Numeric, alphanumeric, or other identifying codes assigned when an art object, book, or other item enters the collection of a museum, library, or other repository."@en ;
    rdfs:isDefinedBy <http://vocab.getty.edu/aat/> ;
    rdfs:label "accession numbers"@en ;
    <http://www.w3.org/2004/02/skos/core#inScheme> <http://vocab.getty.edu/aat/> .


###  http://vocab.getty.edu/aat/300343820
<http://vocab.getty.edu/aat/300343820> rdf:type owl:NamedIndividual ,
            <http://vocab.getty.edu/aat/Concept> ;
    <http://purl.org/dc/elements/1.1/identifier> "300343820" ;
    rdfs:comment "The process and technique of creating two-dimensional decoration on pottery by using paint made of metallic oxides or other pigments held in suspension in slip or another medium."@en ;
    rdfs:isDefinedBy <http://vocab.getty.edu/aat/> ;
    rdfs:label "vase painting (image-making)"@en ;
    <http://www.w3.org/2004/02/skos/core#inScheme> <http://vocab.getty.edu/aat/> .


###  http://vocab.getty.edu/aat/300386427
<http://vocab.getty.edu/aat/300386427> rdf:type owl:NamedIndividual ,
            <http://vocab.getty.edu/aat/Concept> ;
    <http://purl.org/dc/elements/1.1/identifier> "300386427" ;
    rdfs:comment "Reduction of data needed for storage or transmission. Data is reduced in volume by means of encoding information to require fewer bits to be stored than the original."@en ;
    rdfs:isDefinedBy <http://vocab.getty.edu/aat/> ;
    rdfs:label "data compression"@en ;
    <http://www.w3.org/2004/02/skos/core#inScheme> <http://vocab.getty.edu/aat/> .


###  http://vocab.getty.edu/aat/300391312
<http://vocab.getty.edu/aat/300391312> rdf:type owl:NamedIndividual ,
            <http://vocab.getty.edu/aat/Concept> ;
    <http://purl.org/dc/elements/1.1/identifier> "300391312" ;
    rdfs:comment "Scanning technique that involves a pattern of lines projected onto a 3-D object and the subsequent mathematical measurement of the deformations caused by the geometry of the object."@en ;
    rdfs:isDefinedBy <http://vocab.getty.edu/aat/> ;
    rdfs:label "structured light scanning"@en ;
    <http://www.w3.org/2004/02/skos/core#inScheme> <http://vocab.getty.edu/aat/> .


###  http://vocab.getty.edu/aat/300391447
<http://vocab.getty.edu/aat/300391447> rdf:type owl:NamedIndividual ,
            <http://vocab.getty.edu/aat/Concept> ;
    <http://purl.org/dc/elements/1.1/identifier> "300391447" ;
    rdfs:comment "Computer software technique for rendering virtual models of surfaces in three-dimensions."@en ;
    rdfs:isDefinedBy <http://vocab.getty.edu/aat/> ;
    rdfs:label "digital surface modeling"@en ;
    <http://www.w3.org/2004/02/skos/core#inScheme> <http://vocab.getty.edu/aat/> .


###  http://vocab.getty.edu/aat/300403970
<http://vocab.getty.edu/aat/300403970> rdf:type owl:NamedIndividual ,
            <http://vocab.getty.edu/aat/Concept> ;
    <http://purl.org/dc/elements/1.1/identifier> "300403970" ;
    rdfs:comment "Manuscript volumes comprising two or more works, whether referring to only the content combined or to the combination of physically separate leafs or gatherings that are sewn or tipped in"@en ;
    rdfs:isDefinedBy <http://vocab.getty.edu/aat/> ;
    rdfs:label "compilation manuscripts"@en ;
    <http://www.w3.org/2004/02/skos/core#inScheme> <http://vocab.getty.edu/aat/> .


###  http://vocab.getty.edu/aat/300404386
<http://vocab.getty.edu/aat/300404386> rdf:type owl:NamedIndividual ,
            <http://vocab.getty.edu/aat/Concept> ;
    <http://purl.org/dc/elements/1.1/identifier> "300404386" ;
    rdfs:comment "Events or activities of finding out or becoming aware of something that had been lost, forgotten, or previously unknown. Includes the finding of archaeological objects, lost buildings, places."@en ;
    rdfs:isDefinedBy <http://vocab.getty.edu/aat/> ;
    rdfs:label "discoveries"@en ;
    <http://www.w3.org/2004/02/skos/core#inScheme> <http://vocab.getty.edu/aat/> .


###  http://vocab.getty.edu/aat/300404704
<http://vocab.getty.edu/aat/300404704> rdf:type owl:NamedIndividual ,
            <http://vocab.getty.edu/aat/Concept> ;
    <http://purl.org/dc/elements/1.1/identifier> "300404704" ;
    rdfs:comment "Identifying numeric or alpha codes found, usually on the spine, of a manuscript, book or other volume, giving the location where the item can be found in the library."@en ;
    rdfs:isDefinedBy <http://vocab.getty.edu/aat/> ;
    rdfs:label "shelf marks"@en ;
    <http://www.w3.org/2004/02/skos/core#inScheme> <http://vocab.getty.edu/aat/> .


###  http://vocab.getty.edu/aat/300417204
<http://vocab.getty.edu/aat/300417204> rdf:type owl:NamedIndividual ,
            <http://vocab.getty.edu/aat/Concept> ;
    <http://purl.org/dc/elements/1.1/identifier> "300417204" ;
    rdfs:comment "Titles or names that were originally assigned to a work or assigned soon after its creation. It may refer to a former title or to a title that has been translated."@en ;
    rdfs:isDefinedBy <http://vocab.getty.edu/aat/> ;
    rdfs:label "original titles"@en ;
    <http://www.w3.org/2004/02/skos/core#inScheme> <http://vocab.getty.edu/aat/> .


###  http://vocab.getty.edu/aat/300417207
<http://vocab.getty.edu/aat/300417207> rdf:type owl:NamedIndividual ,
            <http://vocab.getty.edu/aat/Concept> ;
    <http://purl.org/dc/elements/1.1/identifier> "300417207" ;
    rdfs:comment "For art cataloging, titles or names by which the work has been known in exhibitions, particularly when different from titles by which the work is normally known."@en ;
    rdfs:isDefinedBy <http://vocab.getty.edu/aat/> ;
    rdfs:label "exhibition titles (work titles)"@en ;
    <http://www.w3.org/2004/02/skos/core#inScheme> <http://vocab.getty.edu/aat/> .


###  http://vocab.getty.edu/aat/300417260
<http://vocab.getty.edu/aat/300417260> rdf:type owl:NamedIndividual ,
            <http://vocab.getty.edu/aat/Concept> ;
    <http://purl.org/dc/elements/1.1/identifier> "300417260" ;
    rdfs:comment "The process or function of copying material or data to a computer drive, the cloud, or otherwise to a safe, more permanent location."@en ;
    rdfs:isDefinedBy <http://vocab.getty.edu/aat/> ;
    rdfs:label "saving (information handling)"@en ;
    <http://www.w3.org/2004/02/skos/core#inScheme> <http://vocab.getty.edu/aat/> .


###  http://vocab.getty.edu/aat/300417639
<http://vocab.getty.edu/aat/300417639> rdf:type owl:NamedIndividual ,
            <http://vocab.getty.edu/aat/Concept> ;
    <http://purl.org/dc/elements/1.1/identifier> "300417639" ;
    rdfs:comment "Method of acquiring property by request from the creator or producer."@en ;
    rdfs:isDefinedBy <http://vocab.getty.edu/aat/> ;
    rdfs:label "commission (method of acquisition)"@en ;
    <http://www.w3.org/2004/02/skos/core#inScheme> <http://vocab.getty.edu/aat/> .


###  http://vocab.getty.edu/aat/300420536
<http://vocab.getty.edu/aat/300420536> rdf:type owl:NamedIndividual ,
            <http://vocab.getty.edu/aat/Concept> ;
    <http://purl.org/dc/elements/1.1/identifier> "300420536" ;
    rdfs:comment "A category of handheld tools or weapons characterized by a sharp-edged blade attached to a handle, typically made of wood or metal."@en ;
    rdfs:isDefinedBy <http://vocab.getty.edu/aat/> ;
    rdfs:label "axe weapons"@en ;
    <http://www.w3.org/2004/02/skos/core#inScheme> <http://vocab.getty.edu/aat/> .


###  http://vocab.getty.edu/aat/300422994
<http://vocab.getty.edu/aat/300422994> rdf:type owl:NamedIndividual ,
            <http://vocab.getty.edu/aat/Concept> ;
    <http://purl.org/dc/elements/1.1/identifier> "300422994" ;
    rdfs:comment "A small decorative item, often made of metal or other materials, that is attached to a necklace or bracelet."@en ;
    rdfs:isDefinedBy <http://vocab.getty.edu/aat/> ;
    rdfs:label "charm pendant"@en ;
    <http://www.w3.org/2004/02/skos/core#inScheme> <http://vocab.getty.edu/aat/> .


###  http://vocab.getty.edu/aat/300425064
<http://vocab.getty.edu/aat/300425064> rdf:type owl:NamedIndividual ,
            <http://vocab.getty.edu/aat/Concept> ;
    <http://purl.org/dc/elements/1.1/identifier> "300425064" ;
    rdfs:comment "Machines for the production of electrical discharge at high voltage."@en ;
    rdfs:isDefinedBy <http://vocab.getty.edu/aat/> ;
    rdfs:label "electrostatic generators"@en ;
    <http://www.w3.org/2004/02/skos/core#inScheme> <http://vocab.getty.edu/aat/> .


###  http://vocab.getty.edu/aat/300426696
<http://vocab.getty.edu/aat/300426696> rdf:type owl:NamedIndividual ,
            <http://vocab.getty.edu/aat/Concept> ;
    <http://purl.org/dc/elements/1.1/identifier> "300426696" ;
    rdfs:comment "Software used to create computer graphics, or edit and otherwise manipulate existing graphics."@en ;
    rdfs:isDefinedBy <http://vocab.getty.edu/aat/> ;
    rdfs:label "graphics software"@en ;
    <http://www.w3.org/2004/02/skos/core#inScheme> <http://vocab.getty.edu/aat/> .


###  http://vocab.getty.edu/aat/300429747
<http://vocab.getty.edu/aat/300429747> rdf:type owl:NamedIndividual ,
            <http://vocab.getty.edu/aat/Concept> ;
    <http://purl.org/dc/elements/1.1/identifier> "300429747" ;
    rdfs:comment "A device that captures images or text documents and converts them into digital data that can be processed by a computer. These scanners use optical technology to scan physical documents or images and create digital representations of them."@en ;
    rdfs:isDefinedBy <http://vocab.getty.edu/aat/> ;
    rdfs:label "optical scanner"@en ;
    <http://www.w3.org/2004/02/skos/core#inScheme> <http://vocab.getty.edu/aat/> .


###  http://vocab.getty.edu/aat/300433476
<http://vocab.getty.edu/aat/300433476> rdf:type owl:NamedIndividual ,
            <http://vocab.getty.edu/aat/Concept> ;
    <http://purl.org/dc/elements/1.1/identifier> "300433476" ;
    rdfs:comment "Instruments used to discharge a capacitor, which is a device capable of storing energy within an electrostatic field."@en ;
    rdfs:isDefinedBy <http://vocab.getty.edu/aat/> ;
    rdfs:label "spark arresters"@en ;
    <http://www.w3.org/2004/02/skos/core#inScheme> <http://vocab.getty.edu/aat/> .


###  http://vocab.getty.edu/aat/300435434
<http://vocab.getty.edu/aat/300435434> rdf:type owl:NamedIndividual ,
            <http://vocab.getty.edu/aat/Concept> ;
    <http://purl.org/dc/elements/1.1/identifier> "300435434" ;
    rdfs:comment "A formal statement of the copyright or licensing of a work, and/or any restrictions placed on it."@en ;
    rdfs:isDefinedBy <http://vocab.getty.edu/aat/> ;
    rdfs:label "copyright/licensing statement"@en ;
    <http://www.w3.org/2004/02/skos/core#inScheme> <http://vocab.getty.edu/aat/> .


###  http://vocab.getty.edu/aat/300440768
<http://vocab.getty.edu/aat/300440768> rdf:type owl:NamedIndividual ,
            <http://vocab.getty.edu/aat/Concept> ;
    <http://purl.org/dc/elements/1.1/identifier> "300440768" ;
    rdfs:comment "Systematically arranged collections of pressed plant specimens that have been gathered in situ, then dried and pressed onto sheets of archival paper so that major morphological characteristics are preserved."@en ;
    rdfs:isDefinedBy <http://vocab.getty.edu/aat/> ;
    rdfs:label "herbaria (documents)"@en ;
    <http://www.w3.org/2004/02/skos/core#inScheme> <http://vocab.getty.edu/aat/> .


###  http://vocab.getty.edu/aat/300445021
<http://vocab.getty.edu/aat/300445021> rdf:type owl:NamedIndividual ,
            <http://vocab.getty.edu/aat/Concept> ;
    <http://purl.org/dc/elements/1.1/identifier> "300445021" ;
    rdfs:comment "Numbers used to identify an individual publication within a classification or location in a library."@en ;
    rdfs:isDefinedBy <http://vocab.getty.edu/aat/> ;
    rdfs:label "book numbers"@en ;
    <http://www.w3.org/2004/02/skos/core#inScheme> <http://vocab.getty.edu/aat/> .


###  Generated by the OWL API (version 5.1.18) https://github.com/owlcs/owlapi/
